<?xml version="1.0" encoding="UTF-8"?>

<section xml:id="sec_fourth-examplesB" xmlns:xi="http://www.w3.org/2001/XInclude">
  <title>Examples B</title>
 
 <example>
  <statement>
    <p>
      Solve <me>
        2x^{2}y'' -xy' +(x^{2}+1)y =0.
      </me>
    </p>
  </statement>
  <solution>
    <p>
      <men xml:id="eqn-powers_ex1">
        2x^{2}y'' -xy' +(x^{2}+1)y =0	
      </men>
      This equation has a regular singularity at <m>x=0</m>. Hence we assume the solution in the form 
      <men xml:id="eqn-powers_ex2">
        y = \sum\limits_{\lambda =0}^{\infty}a_{\lambda}x^{\lambda+k} 
      </men>
      or,
      <me>
        y' = \sum\limits_{\lambda =0}^{\infty}a_{\lambda}(\lambda+k)x^{\lambda+k-1}
      </me>
      and 
      <me>
        y'' = \sum\limits_{\lambda =0}^{\infty}a_{\lambda}(\lambda+k)(\lambda+k-1)x^{\lambda+k-2}
      </me>
      Substituting these values in eqn. <xref ref="eqn-powers_ex1"/>, we get - 
      <me>
        2x^{2}\sum\limits_{\lambda =0}^{\infty}a_{\lambda}(\lambda+k)(\lambda+k-1)x^{\lambda+k-2}-x\sum\limits_{\lambda =0}^{\infty}a_{\lambda}(\lambda+k)x^{\lambda+k-1}
      </me>
      <me>
         +(x^{2}+1)\sum\limits_{\lambda =0}^{\infty}a_{\lambda}x^{\lambda+k} =0
      </me>
      or,
      <me>
        \sum\limits_{\lambda =0}^{\infty}a_{\lambda}\left[2(\lambda+k)(\lambda+k-1)x^{\lambda+k-1}-(\lambda+k)x^{\lambda+k}+x^{\lambda+k}\right]
      </me>
      <me>
        +\sum\limits_{\lambda =0}^{\infty}a_{\lambda}x^{\lambda+k+2} =0
      </me>
      or,
      <me>
        \sum\limits_{\lambda =0}^{\infty}a_{\lambda}\left[(\lambda+k)\{2(\lambda+k-1)-1\}+1\right]x^{\lambda+k}
      </me>
      <me>
        +\sum\limits_{\lambda =0}^{\infty}a_{\lambda}x^{\lambda+k+2} =0
      </me>
      or, 
      <men xml:id="eqn-powers_ex3">
        \sum\limits_{\lambda =0}^{\infty}a_{\lambda}\left[(\lambda+k)(2\lambda+2k-3)+1\right]x^{\lambda+k}+\sum\limits_{\lambda =0}^{\infty}a_{\lambda}x^{\lambda+k+2} =0 
      </men>
      Equating the coefficient of lowest power of <m>x</m> (i.e., 
      the coefficient of <m>x^{k}</m>) to zero. We get the indicial equation.
      <me>
        a_{o}\left[k(2k-3)+1\right] =0
      </me>
      or,
      <me>
        2k^{2}-3k+1 =0 \quad \text{Since,}\quad a_{o}\neq 0.
      </me>
      or,
      <me>
         2k^{2}-2k-k+1 =0
      </me>
      or,
      <me>
        (2k-1)(k-1)=0  \hspace{1cm} \Rightarrow k=1,\frac{1}{2}
      </me>
      and the difference of roots is not an integer.
    </p>
    <p>
      Equating the coefficient of next higher power of <m>x</m> (i.e., <m>x^{k+1}</m>) to zero, we get 
      <me>
        a_{1}\left[(k+1)(2k+2-3)+1\right] =0
      </me>
      or,
      <me>
        a_{1}\left[(k+1)(2k-1)+1\right] =0
      </me>
      or,
      <me>
        a_{1}\left[2k^{2}-k+2k-1+1\right] =0
      </me>
      or,
      <me>
       a_{1}\left[2k^{2}+k\right] =0
      </me>
      or,
      <me>
        a_{1}\left[2k+1\right]k =0
      </me>
      for <m>k=1</m>,
      <me>
        (2k+1)k \neq =0, \quad \text{hence,} \quad a_{1}=0
      </me>
      for <m>k=\frac{1}{2}</m>
      <me>
       (2k+1)k \neq =0, \quad \text{hence,} \quad a_{1}=0 
      </me>
       i.e., the series solution does not contain the coefficient <m>a_{1}</m>.
      </p>
      <p>
        Again, equating the coefficient of general power of <m>x</m> (i.e., <m>x^{\lambda+k+2}</m>) to zero, 
        we get the recursion relation.
        <me>
          \sum a_{\lambda+2}\left[(\lambda+k+2)\{2k+2(\lambda+2)-3\}+1\right]+\sum a_{\lambda}=0
        </me>
        <men xml:id="eqn-powers_ex4">
          \therefore  a_{\lambda+2} =-\frac{a_{\lambda}}{\left[(k+\lambda+2)\{2k+2\lambda+1\}+1\right]} 
        </men>
        for <m>k=1</m> 
        <me>
          a_{\lambda+2} =-\frac{a_{\lambda}}{\left[(\lambda+3)(2\lambda+3)+1\right]}  
        </me>
        [from equation <xref ref="eqn-powers_ex4"/>]
        or,
        <me>
          a_{2}=-\frac{a_{o}}{(3\cdot 3+1)}=-\frac{a_{o}}{10};\quad a_{4}=-\frac{a_{2}}{(5\cdot 7+1)}=\frac{a_{o}}{36\cdot 10}=\frac{a_{o}}{360};
        </me>
        and so on. Or,
        <me>
          y_{1}=x\left[a_{o}+a_{1}x+a_{2}x^{2}+a_{3}x^{3}+a_{4}x^{4}+\cdots\right] 
        </me>
        <men xml:id="eqn-powers_ex5">
          \therefore y_{1}= a_{o}x\left[1-\frac{x^{2}}{10}+\frac{x^{4}}{360}-\cdots\right]
        </men>
         for <m>k=\frac{1}{2}</m>,
        <me>
          a_{\lambda+2} =-\frac{a_{\lambda}}{\left[(\lambda+\frac{5}{2})(2\lambda+2)+1\right]}  
        </me>
        [from eqn. <xref ref="eqn-powers_ex4"/>]
        or,
        <me>
          a_{2}=-\frac{a_{o}}{(\frac{5}{2}\cdot 2+1)}=-\frac{a_{o}}{6};
        </me>
        <me>
          a_{4}=-\frac{a_{2}}{(\frac{9}{2}\cdot 6+1)}=\frac{a_{o}}{6\cdot 28}=\frac{a_{o}}{168}; 
        </me>
        and so on.  From eqn. <xref ref="eqn-powers_ex2"/>, we have 
        <me>
          y_{2}=x^{\frac{1}{2}}\left[a_{o}+a_{1}x+a_{2}x^{2}+a_{3}x^{3}+a_{4}x^{4}+\cdots\right] 
        </me>
       <men xml:id="eqn-powers_ex6">
         \therefore, y_{2}= a_{o}x^{\frac{1}{2}}\left[1-\frac{x^{2}}{6}+\frac{x^{4}}{168}-\cdots\right] 
       </men>
       The complete solution of eqn. <xref ref="eqn-powers_ex1"/> is 
       <me>
        y=C_{1}y_{1}+C_{2}y_{2}
       </me>
       <me>
        =Ax\left[1-\frac{x^{2}}{10}+\frac{x^{4}}{360}-\cdots\right]+Bx^{\frac{1}{2}}\left[1-\frac{x^{2}}{6}+\frac{x^{4}}{168}-\cdots\right] 
       </me>
        </p>
  </solution>
 </example>

    <example>
      <statement>
        <p>
           Solve <me>
            xy''+y' +x^{2}y=0
           </me>
            </p>
      </statement>
      <solution>
        <p>
          <men xml:id="eqn-powers_eq8">
            xy''+y'+x^{2}y=0 
          </men>
          The equation has <m>x=0</m> is a regular singular point.
          Let  
          <men xml:id="eqn-powers_eq9">
            y=\sum\limits_{\lambda=0}^{\infty}a_{\lambda}x^{\lambda+k}
          </men>
           be the solution of eqn. <xref ref="eqn-powers_eq8"/>.  
           Since eqn. <xref ref="eqn-powers_eq9"/> satisfies the eqn. <xref ref="eqn-powers_eq8"/> we have 
           <me>
            x\sum a_{\lambda}(\lambda+k)(\lambda+k-1)x^{\lambda+k-2}
           </me> 
           <me>
            +\sum a_{\lambda}(\lambda+k)x^{\lambda+k-1} +x^{2}\sum a_{\lambda}x^{\lambda+k} =0
           </me>
           
           or,
           <me>
            \sum a_{\lambda}(\lambda+k)(\lambda+k-1)x^{\lambda+k-1}+\sum a_{\lambda}(\lambda+k)x^{\lambda+k-1}+\sum a_{\lambda}x^{\lambda+k+2} =0
           </me>
           or,
           <me>
            \sum a_{\lambda}\left[(\lambda+k)(\lambda+k-1) +(\lambda+k)\right]x^{\lambda+k-1}+\sum a_{\lambda}x^{\lambda+k+2} =0
           </me>
           or,
           <men xml:id="eqn-powers_eq10">
            \sum a_{\lambda}(\lambda+k)^{2}x^{\lambda+k-1} +\sum a_{\lambda}x^{\lambda+k+2} =0      
           </men>
           Equating the coefficient of lowest power of <m>x</m>  (i.e., <m>x^{k-1} </m>) to zero, we get - 
           <me>
            a_{o}(k^{2})=0 \hspace{1cm} \because \quad a_{o}\neq  0  \quad \Rightarrow k=0,0. 
           </me>
           Equating the coefficient of <m> x^{k}</m> to zero, we get -
           <me>
            a_{1}(k+1)^{2}=0 
           </me>
           for <m>k=0,</m>
           <me>
            (k+1)^{2} \neq 0,\quad 
           </me>
           hence, <m>a_{1}=  0.</m> 
           Again, equating the coefficient of <m>x^{k+1}</m> to zero, we get -
           <me>
            a_{2}(k+2)^{2}=0 \quad \Rightarrow a_{2}=  0. 
           </me>
          [<m>\because \quad (k+2)^{2} \neq 0</m> at <m>k=0</m>.] 
          Equating the coefficient of <m>x^{\lambda+k+2}</m> to zero, we get - 
          <me>
            a_{\lambda+3}(\lambda+k+3)^{2}+a_{\lambda}=0
          </me>
          or, 
         <men xml:id="eqn-powers_eq11">
         a_{\lambda+3} =-\frac{a_{\lambda}}{(\lambda+k+3)^{2}}  
         </men>
         for <m>\lambda =0,</m> 
         <me>
           a_{3}=-\frac{a_{o}}{(m+3)^{2}},
         </me>
         for <m>\lambda =1,</m>  
         <me>
           a_{4}=-\frac{a_{1}}{(m+4)^{2}}=0,
         </me>
         also, <m>a_{7}=0,\quad a_{10}=0,</m> 
          for <m>\lambda =2,</m> 
          <me>
             a_{5}=-\frac{a_{2}}{(m+5)^{2}}=0,
          </me>
          also, <m>a_{8}=0,\quad  a_{11}=0,</m> 
          for <m>\lambda =3,</m>  
          <me>
            a_{6}=-\frac{a_{3}}{(m+6)^{2}}=\frac{a_{o}}{(m+3)^{2}(m+6)^{2}},
          </me>
          similarly, 
          <me>
            a_{9}=-\frac{a_{6}}{(m+9)^{2}}=-\frac{a_{o}}{(m+3)^{2}(m+6)^{2}(m+9)^{2}},
          </me>
           and so on.         
        </p>
        <p>
          Hence, from eqn. <xref ref="eqn-powers_eq9"/>, we get -
          <me>
             y=a_{o}x^{m}\left[1-\frac{x^{3}}{(m+3)^{2}}+\frac{x^{6}}{(m+3)^{2}(m+6)^{2}} \right.
          </me>
          
          <men xml:id="eqn-powers_eq12">
            \left. -\frac{x^{9}}{(m+3)^{2}(m+6)^{2}(m+9)^{2}}+\cdots\right] 
          </men>
          To get the first solution, let <m>m=0</m> in eqn. <xref ref="eqn-powers_eq12"/>, 
          <men xml:id="eqn-powers_eq13">
            y_{1}=a_{o}\left[1-\frac{x^{3}}{3^{2}}+\frac{x^{6}}{3^{2}\cdot 6^{2}}-\frac{x^{9}}{3^{2}\cdot 6^{2}\cdot 9^{2}}+\cdots\right]
          </men>
          To get the second independent solution, differentiate eqn. <xref ref="eqn-powers_eq12"/> w.r.t. 
          'm', we get -
          <fn>
          Let 
          <me>
            \theta =a_{o}x^{m}
          </me>
          then.
          <me>
            \log\theta = \log a_{o}+m\log x 
          </me>
          or,
          <me>
           \frac{1}{\theta}\partial\theta =0+\log x\partial m  
          </me>
          <me>
            \therefore \frac{\partial\theta}{\partial m } = \theta\log x. 
          </me>
          </fn>
          </p>
          <p>
            <me>
               \frac{\partial y}{\partial m} =a_{o}x^{m}\log x\left[1-\frac{x^{3}}{(m+3)^{2}}+\frac{x^{6}}{(m+3)^{2}(m+6)^{2}}-\cdots\right]
            </me>
            <me>
              +a_{o}x^{m}\left[\frac{2x^{3}}{(m+3)^{3}}-\frac{2x^{6}}{(m+3)^{3}(m+6)^{2}}-\frac{2x^{6}}{(m+3)^{2}(m+6)^{3}}+\cdots\right]
            </me>
            <me>
              \therefore y_{2}=\left(\frac{\partial y}{\partial m}\right)_{m=0}= a_{o}\log x \left[1-\frac{x^{3}}{3^{2}}+\frac{x^{6}}{3^{2}\cdot 6^{2}}-\cdots\right]
            </me>
            
            <men xml:id="eqn-powers_eq14">
               +a_{o}\left[\frac{2x^{3}}{3^{3}}-\frac{2x^{6}}{3^{3}\cdot 6^{2}}-\frac{2x^{6}}{3^{2}\cdot 6^{3}}+\cdots\right]     
            </men>
            Hence the general solution is given by
            <me>
               y=C_{1}y_{1}+C_{2}y_{2}=a_{o}C_{1}\left[1-\frac{x^{3}}{3^{2}}+\frac{x^{6}}{3^{2}\cdot 6^{2}}-\cdots\right]
            </me>
            <me>
             +a_{o}C_{2}\log x\left[1-\frac{x^{3}}{3^{2}}+\frac{x^{6}}{3^{2}\cdot 6^{2}}-\cdots\right] 
            </me>
            <me>
              +a_{o}C_{2}\left[\frac{2x^{3}}{3^{3}}-\frac{2x^{6}}{3^{2}\cdot 6^{2}}(\frac{1}{3}+\frac{1}{6})-\frac{2x^{6}}{3^{2}\cdot 6^{2}\cdot 9^{2}}(\frac{1}{3}+\frac{1}{6}+\frac{1}{9})+\cdots\right]
            </me>
            <me>
               \therefore y =\left(C_{1}+C_{2}\log x\right)a_{o}\left[1-\frac{x^{3}}{3^{2}}+\frac{x^{6}}{3^{2}\cdot 6^{2}}-\cdots\right]
            </me>
             <men xml:id="eqn-powers_eq15">
             +2a_{o}C_{2}\left[\frac{x^{3}}{3^{3}}-\frac{x^{6}}{3^{5}\cdot 2^{2}}(1+\frac{1}{2})+\cdots\right]  
            </men>
            </p>
      </solution>
    </example>

    <example>
      <statement>
        <p>
          Solve <me>
            x^{2}y''+xy'+(x^{2}-1)y=0.
          </me>
        </p>
      </statement>
      <solution>
        <p>
          <men xml:id="eqn-powers_eq16">
            x^{2}y''+xy'+(x^{2}-1)y=0 
          </men>
          Let
          <men xml:id="eqn-powers_eq17">
             y=\sum\limits_{\lambda =0}^{\infty}a_{\lambda}x^{\lambda+k}
          </men>
           be the solution of eqn. <xref ref="eqn-powers_eq16"/>. 
           With the help of eqn. <xref ref="eqn-powers_eq17"/>, eqn. <xref ref="eqn-powers_eq16"/> becomes-
           <me>
            x^{2}\sum a_{\lambda}(\lambda+k)(\lambda+k-1)x^{\lambda+k-2}+x\sum a_{\lambda}(\lambda+k)x^{\lambda+k-1} 
           </me>
           <me>
            +(x^{2}-1)\sum a_{\lambda}x^{\lambda+k}=0
           </me>
           or,
           <me>
            \sum a_{\lambda}\left[(\lambda+k)(\lambda+k-1)+(\lambda +k)-1\right]x^{\lambda+k}+\sum a_{\lambda}x^{\lambda+k-2}=0
           </me>
           or,
           <me>
            \sum a_{\lambda}\left[(\lambda+k)^{2}-1\right]x^{\lambda+k}+\sum a_{\lambda}x^{\lambda+k+2}=0
           </me>
           or,
           <men xml:id="eqn-powers_eq18">
            \sum\limits_{\lambda=0}^{\infty} a_{\lambda}\left[(\lambda+k+1)(\lambda+k-1)\right]x^{\lambda+k}+\sum\limits_{\lambda=0}^{\infty} a_{\lambda}x^{\lambda+k+2}=0 
           </men>
           Equating the coefficient of <m>x^{k}</m> to zero, we get -
           <me>
             a_{o}(k+1)(k-1)=0 \quad \Rightarrow k=1,-1 \quad \because a_{o} \neq 0 
           </me>
           Equating the coefficient of  <m>x^{k+1}</m>  to zero, we get - 
           <me>
            a_{1}(k+2)k=0 \Rightarrow a_{1}=0  \quad \because (k+2)k \neq 0 \quad \text{for}\quad k=\pm 1
           </me>
           Equating the coefficient of <m>x^{\lambda+ k+2}</m> to zero, we get - 
           <me>
            a_{\lambda+ 2}\left[(\lambda +k+3)(\lambda+ k+1)\right]+a_{\lambda}=0 
           </me>
           or,
           <me>
             a_{\lambda+ 2}=- \frac{a_{\lambda}}{\left[(\lambda +k+3)(\lambda+ k+1)\right]} 
           </me>
           or,
           <me>
            a_{2}=- \frac{a_{o}}{(k+3)(k+1)}
           </me>
           or,
           <me>
            a_{3}=- \frac{a_{1}}{(k+4)(k+2)}=0 =a_{5}=a_{7}=\cdots
           </me>
           or,
           <me>
            a_{4}=- \frac{a_{2}}{(k+5)(k+3)}= \frac{a_{o}}{(k+1)(k+3)^{2}(k+5)} 
           </me>
           Hence, from eqn. <xref ref="eqn-powers_eq17"/>, we have 
           <me>
             y=a_{o}x^{k}\left[1-\frac{x^{2}}{(k+1)(k+3)}\right.
           </me>
           <men xml:id="eqn-powers_eq19">
            \left. +\frac{x^{4}}{(k+1)(k+3)^{2}(k+5)}-\cdots\right] 
           </men>
           putting <m>k=1</m> in eqn. <xref ref="eqn-powers_eq19"/>, we get -
           <men xml:id="eqn-powers_eq20">
            y=a_{o}x\left[1-\frac{x^{2}}{(2)(4)}+\frac{x^{4}}{(2)(4)^{2}(6)}-\cdots\right] 
           </men>
           Coefficient of <m>x^{2}{,}x^{4},</m> etc. in eqn. <xref ref="eqn-powers_eq19"/> 
           becomes infinite when <m>k=-1 </m>. If any one coefficient of the series 
           becomes infinite at <m>k=k_{2}</m>, we should put <m>a_{o}=b_{o}(k-k_{2})</m> 
           to overcome this difficulty. 
        </p>
        <p>
          Hence, put <m>a_{o}=b_{o}(k+1)</m> in eqn. <xref ref="eqn-powers_eq19"/>, we get - 
          <me>
            y=b_{o}x^{k}\left[(k+1)-\frac{(k+1)x^{2}}{(k+1)(k+3)}+\frac{(k+1)x^{4}}{(k+1)(k+3)^{2}(k+5)}-\cdots\right]
          </me>
          <men xml:id="eqn-powers_eq21">
            =b_{o}x^{k}\left[(k+1)-\frac{x^{2}}{(k+3)}+\frac{x^{4}}{(k+3)^{2}(k+5)}-\cdots\right] 
          </men>
           On differentiating eqn. <xref ref="eqn-powers_eq21"/> w.r.t. 'k', we get -
           <me>
            \frac{\partial y}{\partial k}=b_{o}x^{k}\log x\left[(k+1)-\frac{x^{2}}{(k+3)}+\frac{x^{4}}{(k+3)^{2}(k+5)}-\cdots\right]
           </me>
           <me>
            + b_{o}x^{k}\left[1+\frac{x^{2}}{(k+3)^{2}}-\frac{2x^{4}}{(k+3)^{2}(k+5)}-\frac{x^{4}}{(k+3)^{2}(k+5)^{2}}+\cdots\right]
           </me>
           on replacing <m>k</m> by -1, we get -
           <me>
            \left(\frac{\partial y}{\partial k}\right)_{k=-1}=b_{o}x^{-1}\log x\left[0-\frac{x^{2}}{2}+\frac{x^{4}}{2^{2}\cdot 4}-\cdots\right] 
           </me>
           <me>
            + b_{o}x^{-1}\left[1+\frac{x^{2}}{2^{2}}-\frac{2x^{4}}{2^{2}\cdot 4}-\frac{x^{4}}{2^{2}\cdot 4^{2}}+\cdots\right]
           </me>
           or,
           <me>
            y=b_{o}x\log x\left[-\frac{1}{2}+\frac{x^{2}}{2^{2}\cdot 4}-\cdots\right]+ b_{o}x^{-1}\left[1+\frac{x^{2}}{2^{2}}-\frac{x^{4}}{2^{2}\cdot 4}(1+\frac{1}{4})+\cdots\right]
           </me>
           <me>
            \therefore y=C_{1}x\left[1-\frac{x^{2}}{2\cdot 4}+\frac{x^{4}}{2\cdot 4^{2}\cdot 6}-\cdots\right]+ C_{2}x\log x\left[-\frac{1}{2}+\frac{x^{2}}{2^{2}\cdot 4}-\cdots\right]
           </me>
           <me>
             +C_{2}x^{-1}\left[1+\frac{x^{2}}{2^{2}}-\frac{x^{4}}{2^{2}\cdot 4}(1+\frac{1}{4})+\cdots\right] 
           </me>
          </p>
      </solution>
    </example>

    <example>
      <statement>
        <p>
          Solve 
          <me>
            x^{2}y''+4xy'+(x^{2}+2)y =0.
          </me>
        </p>
      </statement>
      <solution>
        <p>
          <men xml:id="eqn-powers_eq22">
            x^{2}y''+4xy'+(x^{2}+2)y =0 
          </men>
          Let 
          <me>
            y=\sum\limits_{\lambda =0}^{\infty}a_{\lambda}x^{\lambda+k}
          </me>
           be the solution of eqn. <xref ref="eqn-powers_eq22"/>. 
           Therefore from eqn. <xref ref="eqn-powers_eq22"/>, we have -
           <me>
             x^{2}\sum a_{\lambda}(\lambda+k)(\lambda+k-1)x^{\lambda+k-2}+4x\sum a_{\lambda}(\lambda+k)x^{\lambda+k-1}
           </me>
           <me>
           +(x^{2}+2)\sum a_{\lambda}x^{\lambda+k}=0
           </me>
           or,
           <me>
            \sum a_{\lambda}(\lambda+k)(\lambda+k-1)x^{\lambda+k}+4\sum a_{\lambda}(\lambda+k)x^{\lambda+k}
           </me>
           <me>
            +\sum a_{\lambda}x^{\lambda+k+2}+2\sum a_{\lambda}x^{\lambda+k}=0
           </me>
           or,
           <me>
            \sum a_{\lambda}\left[(\lambda+k)\{(\lambda+k-1)+4\}+2\right]x^{\lambda+k}+\sum a_{\lambda}x^{\lambda+k+2}=0 
           </me>
           or,
         <men xml:id="eqn-powers_eq23">
          \sum a_{\lambda}\left[(\lambda+k)^{2}+3(\lambda+k)+2\right]x^{\lambda+k}+\sum a_{\lambda}x^{\lambda+k+2}=0 
         </men>
         Equating the coefficient of <m>x^{k} </m> to zero, we get -
         <me>
          a_{o}(k^{2}+3k+2)=0, 
         </me>
         or,
         <me>
          (k+1)(k+2)=0 
         </me>
         <me>
          \because \quad a_{o}\neq 0.   \quad \therefore \quad k=-1,-2.
         </me>
         Equating the coefficient of <m>x^{k+1}</m> to zero, we get -
         <me>
          a_{1}\left[(k+1)^{2}+3(k+1)+2\right]=0 
         </me>
         or,
         <me>
           a_{1}\left[k^{2}+5k+6\right]=0
         </me>
         or,
         <me>
          a_{1}\left[(k+2)(k+3)\right]=0
         </me>
         for <m>k=-2</m>, <m>a_{1}</m>  may or may not be zero, also <m>k \neq -3</m>.
         for <m>k=-1,</m> <m>a_{1} =0</m>.
         Equating the coefficient of <m>x^{\lambda +k+2}</m> to zero, we get -
         <me>
          a_{\lambda+2}\left[(\lambda+ k+2)^{2}+3(\lambda+ k+2)+2\right]+a_{\lambda}=0
         </me>
         or,
         <me>
           a_{\lambda+2}\left[(\lambda+ k+2)(\lambda+ k+5)+2\right]+a_{\lambda}=0
         </me>
         or,
         <me>
          a_{\lambda+2}\left[k^{2}+(2\lambda+ 7)k+\lambda^{2}+ 7\lambda+12 \right]+a_{\lambda}=0
         </me>
         or,
         <men xml:id="eqn-powers_eq24">
           a_{\lambda+2}=-\frac{a_{\lambda}}{k^{2}+(2\lambda+ 7)k+\lambda^{2}+ 7\lambda+12}  
         </men>
         for <m>k=-1</m>, 
         <me>
          a_{\lambda+2}=-\frac{a_{\lambda}}{(-1)^{2}+(2\lambda+ 7)(-1)+\lambda^{2}+ 7\lambda+12} 
         </me>
         <me>
           =-\frac{a_{\lambda}}{1-(2\lambda+7)+\lambda^{2}+7\lambda+12}
         </me>
         
         At <m>\lambda=0</m>, 
         <me>
          a_{2}=-\frac{a_{o}}{1-7+12} =-\frac{a_{o}}{6};
         </me>
         <me>
          a_{3}=-\frac{a_{1}}{1-9+1+7+12} =0=a_{5}=a_{7}=\cdots;
         </me>
         <me>
          a_{4}=-\frac{a_{o}}{120}.
         </me>
          Hence, for <m>k=-1</m>,	
         <men xml:id="eqn-powers_eq25">
         y_{1}=a_{o}x^{-1}\left[1-\frac{x^{2}}{6}+\frac{x^{4}}{120}-\cdots\right]     
         </men>
         for <m>k=-2</m>, 
         <me>
          a_{\lambda+2}=-\frac{a_{\lambda}}{4-2(2\lambda+7)+\lambda^{2}+7\lambda +12}
         </me>
         	At <m>\lambda=0</m>, 
          <me>
            a_{2}=-\frac{a_{o}}{4-2(7)+12} =-\frac{a_{o}}{2};
          </me>
          At <m>\lambda=1</m>, 
          <me>
            a_{3}=-\frac{a_{1}}{4-18+1+7+12} =-\frac{a_{1}}{6};
          </me>
          At <m>\lambda=2</m>, 
          <me>
            a_{4}=-\frac{a_{2}}{4-2(11)+4+14+12}=\frac{a_{o}}{24};
          </me>
          At <m>\lambda=3</m>, 
          <me>
             a_{5} = \frac{a_{1}}{120}.
          </me>
          Hence, for <m>k=-2</m>, 
          <me>
             y_{2}=a_{o}x^{-2}\left[1-\frac{x^{2}}{2}+\frac{x^{4}}{24}-\cdots\right]
          </me>
          <men xml:id="eqn-powers_eq26">
           +a_{1}x^{-1}\left[1-\frac{x^{2}}{6}+\frac{x^{4}}{120}-\cdots\right] 
          </men>
          Here, the solution <xref ref="eqn-powers_eq25"/> is a part of solution 
          <xref ref="eqn-powers_eq26"/> which is not possible because expansion of <m>y_{1}</m> 
          and <m>y_{2}</m> are two different solutions of the same equation and 
          hence <m>a_{1}</m> must be zero in solution <xref ref="eqn-powers_eq26"/>. 
          <me>
            \therefore \quad y_{2}=a_{o}x^{-2}\left[1-\frac{x^{2}}{2}+\frac{x^{4}}{24}-\cdots\right]
          </me>
          Thus the complete solution is <m> y=Ay_{1} +By_{2}.</m>
          <me>
            \therefore \quad y = Ax^{-1}\left[1-\frac{x^{2}}{6}+\frac{x^{4}}{120}-\cdots\right]+Bx^{-2}\left[1-\frac{x^{2}}{2}+\frac{x^{4}}{24}-\cdots\right]
          </me>
        </p>
      </solution>
    </example>
</section>
