<?xml version="1.0" encoding="UTF-8"?>

<section xml:id="sec_sixth-diffLT" xmlns:xi="http://www.w3.org/2001/XInclude">
  <title>Solution of Differential Equations by Laplace Transforms</title>
  <introduction>
   <p>
    Ordinary linear differential equtions with constant coefficient or 
    variable coefficient can easily be solved using Laplace Transform method, 
    without finding the general solution and arbitrary constants.
    </p>
     </introduction>
 <subsection xml:id="subsec-usf_LT1">
  <title>Unit Step Function</title>

   <figure xml:id="fig-fig61">
                <caption>Unit step function</caption>
                <image source="fig61.png" width="50%"/>
            </figure>
            <introduction>
             
  <p>
    <idx>unit step function</idx> 
    With the help of unit step functions, we can find the inverse transform 
    of such functions which can not be determined with the previously explained methods. 
    The unit step functions  <m>u(t-a)</m> is defined as 
    <me>
      u(t-a) = \begin{cases}
 0,  &amp; \text{where} \quad t \lt a\\
 1,  &amp; \text{where} \quad  t\geq a
 \end{cases}
    </me>
and <m>a\geq 0</m>.  The unit step function can be visulized as figure <xref ref="fig-fig61"/>.
    </p>
     
            </introduction>
 

<subsubsection xml:id="subsubsec-usf_LT2">
  <title>Laplace Transform of Unit Step Function</title>
  <p>
    	<me>
        L[u(t-a)] =\frac{e^{-as}}{s}
      </me>
    </p>
    <proof>
      <p>
        <me>
           \mathscr{L}[u(t-a)] =\int\limits_{0}^{\infty} e^{-st}u(t-a)\,dt
        </me>
        <me>
          =\int\limits_{0}^{a} e^{-st}.0\,dt + \int\limits_{a}^{\infty} e^{-st}.1\,dt = 0+\left[\frac{e^{-st}}{-s}\right]_{a}^{\infty}= \frac{e^{-as}}{s}.
        </me>
      </p>
    </proof>
</subsubsection>
</subsection>

<subsection xml:id="subsec-ssp_LT">
  <title>Second-Shifting Property</title>
  <p> If
    <me>
      \mathscr{L}[f(t)] F(s)\text{and}\quad g(t) 
      = \begin{cases}
 f(t-a),  &amp; \text{where} \quad t\geq a\\
 0,  &amp; \text{where} \quad t \lt a
 \end{cases}
    </me>
  then <me>
     \mathscr{L}[g(t)] = e^{-as}F(s).
  </me>
     </p>
     <proof>
      <p>
      <me>
        \mathscr{L}[g(t)] = \int\limits_{0}^{\infty} e^{-st}g(t)\,dt
      </me>
      <me>
        = \int\limits_{0}^{a} e^{-st}g(t)\,dt +\int\limits_{a}^{\infty} e^{-st}g(t)\,dt
      </me>
      <me>
        = \int\limits_{0}^{a} e^{-st}.0\,dt +\int\limits_{a}^{\infty} e^{-st}f(t-a)\,dt
      </me>
      <me>
         = \int\limits_{0}^{\infty} e^{-s(h+a)}.f(h)\,dh 	=  e^{-as} \int\limits_{0}^{\infty}f(h)\,dh
      </me>
      <me>
        = e^{-as}F(s) 
      </me>
     [put <m>  t-a =h</m>] 
      </p>
     </proof>
</subsection>

<theorem xml:id="thm-usf">
  <statement>
    <p>
      <me>
        \mathscr{L}[f(t).u(t-a)] =e^{-as}L[f(t+a)]
      </me>
    </p>
    <proof>
      <p>
        <me>
          \mathscr{L}[f(t).u(t-a)]=\int\limits_{0}^{\infty}e^{-st}[f(t).u(t-a)]\,dt
        </me>
        <me>
          =\int\limits_{0}^{a}e^{-st}[f(t).u(t-a)]\,dt+\int\limits_{a}^{\infty}e^{-st}[f(t).u(t-a)]\,dt
        </me>
        <me>
           = 0+ \int\limits_{a}^{\infty}e^{-st}f(t).1\,dt
        </me>
        <me>
          = \int\limits_{0}^{\infty}e^{-s(y+a)}f(y+a)\,dy= e^{-as}\int\limits_{0}^{\infty}e^{-sy}f(y+a)\,dy = e^{-as}F(s+a)
        </me>
        [put <m>y+a = t</m>.]
      </p>
    </proof>
  </statement>
</theorem>

<subsection xml:id="subsec-pf_LT">
  <title>Priodic Functions</title>
  <p>
    Let <m>f(t)</m>  be a periodic function with period <m>T</m>, then 
    <me>
      \mathscr{L}\{f(t)\} = \frac{\int\limits_{0}^{T}e^{-st} f(t)\,dt}{1-e^{-sT}}
    </me>
    </p>
    <proof>
      <p>
        <me>
          \mathscr{L}\{f(t)\} = \int\limits_{0}^{\infty}e^{-st} f(t)\,dt
        </me>
        <me>
          = \int\limits_{0}^{T}e^{-st} f(t)\,dt+ \int\limits_{T}^{2T}e^{-st} f(t)\,dt+ \int\limits_{2T}^{3T}e^{-st} f(t)\,dt+\cdots
        </me>
        <me>
           =\sum\limits_{n=0}^{\infty}\int\limits_{nT}^{(n+1)T}e^{-st} f(t)\,dt
        </me>
      </p>
      <p>
        If we put <m>t=u+nT</m>, then <m>f(u+nT)=f(u)</m> as <m>T</m> is period of the given function. Thus
        <me>
          \mathscr{L}\{f(t)\} = \sum\limits_{n=0}^{\infty}\int\limits_{0}^{T}e^{-s(u+nT)} f(u)\,du 
        </me>
        <me>
          = \sum\limits_{n=0}^{\infty}e^{-snt}\int\limits_{0}^{T}e^{-su}f(u)\,du
        </me>
        
        <me>
          =1+e^{-st}+e^{-2st}+\cdots+\int\limits_{0}^{T}e^{-su}f(u)\,du 
        </me>
        <me>
          = \frac{1}{1-e^{-sT}}\int\limits_{0}^{T}e^{-su}f(u)\,du
        </me>
        
        <m>[\because \quad 1+a+a^{2}+a^{3}+\cdots=\frac{1}{1-a};</m> if <m>a \lt 1]</m>.
<me>
  \therefore \quad \mathscr{L}\{f(t)\} = \frac{\int\limits_{0}^{T}e^{-st} f(t)\,dt}{1-e^{-sT}}
</me>
by changing <m>u</m> into <m>t</m>.
        </p>
    </proof>
</subsection>

<subsection xml:id="subsec-conv_LT">
  <title>Convolution Theorem</title>
  <introduction>
   
  <p>
    Convolution theorem is a mathematical operation widely used in communication physics. 
    It is a very fine method to find the inverse of Laplace Transform. If 
    <m>\mathscr{L}\{f_{1}(t)\}=F_{1}(s)</m>  and <m>\mathscr{L}\{f_{2}(t)\}=F_{2}(s)</m> then, 
    the convolution theorem can be stated as 
    <me>
      \mathscr{L}\{\int\limits_{0}^{t}f_{1}(x)f_{2}(t-x)\,dx\} = F_{1}(s)\cdot F_{2}(s).
    </me>
    </p>
    <proof>
      <p> Let
        <me>
          \int\limits_{0}^{t}f_{1}(x)f_{2}(t-x)\,dx = H(t).
        </me>
        Then 
        <me>
          \mathscr{L}\{H(t)\}=\int\limits_{0}^{\infty}e^{-st}H(t)\,dt 
        </me>
<me>
  = \int\limits_{t=0}^{\infty}e^{-st}\left[\int\limits_{x=0}^{t}f_{1}(x)f_{2}(t-x)\,dx\right]\,dt 
</me>
<me>
 =\int\limits_{t=0}^{\infty}\left[\int\limits_{x=0}^{t}e^{-st}f_{2}(t-x)\,dx\right]\,dt 
</me>
the integration is being done w.r.t. 'x' first and then w.r.t 't'. 
      </p>
      <figure xml:id="fig-fig64">
                <caption></caption>
                <image source="fig64.png" width="50%"/>
            </figure>
      <p>
        The above integration is taken within the region lying below the line OP whose equation 
        is <m>x=t</m> and above OT, <m>t</m> is taken along OT  and <m>x</m>  is along OX, 
        with O as the origin, the axes is perpendicular to each other, as shown in figure <xref ref="fig-fig64"/>. 

 If the order of integration is changed, the strip will be taken parallel to OT so that the 
 limits of <m>t</m> are from <m>x</m> to <m>\infty</m> and the limits of <m>x</m> are from 0 to <m>\infty</m>.                     
Putting <m>t-x=\theta</m>, we have <m>\,dt=\,d\theta</m>.
<me>
  \therefore \quad \mathscr{L}\{H(t)\}=\int\limits_{0}^{\infty}e^{-sx}f_{1}(x)\int\limits_{0}^{\infty}e^{-s\theta}f_{2}(\theta)\,d\theta\,dx 
</me>
<me>
  = \int\limits_{0}^{\infty}e^{-sx}f_{1}(x)F_{2}(s)\,dx   = F_{1}(s)\cdot F_{2}(s) 
</me>

putting the value of <m>H(t)</m>, we get - 
<me>
   \mathscr{L}\{\int\limits_{0}^{t}f_{1}(x)F_{2}(t-x)\,dx\} = F_{1}(s)\cdot F_{2}(s).
</me>
        </p>
    </proof>
 </introduction>
 
    <subsubsection xml:id="subsubsec-varCoef_LT">
  <title>Differential Equation with Variable Coefficients</title>
  <p>
    see <xref ref="subsubsec-var_coef"/>
    </p>
</subsubsection>
</subsection>

  </section>

