<?xml version="1.0" encoding="UTF-8"?>

<section xml:id="sec_fourth-diff" xmlns:xi="http://www.w3.org/2001/XInclude">
  <title>Solution of a Differential Equation</title>
  <introduction>
   <p>
    Let the differential equation
    <men xml:id="eqn-diffsol1">
      \frac{\,dy}{\,dx}=\frac{1}{x}
    </men>
    Integrating both sides of eqn. <xref ref="eqn-diffsol1"/>, we get -
    <men xml:id="eqn-diffsol2">
      y=\int\frac{1}{x}\,dx = \log x+C
    </men>
    The eqn. <xref ref="eqn-diffsol2"/> is called the general solution of differential eqn. 
    <xref ref="eqn-diffsol1"/> and <m>C</m> is an arbitrary constant. 
    Consider the another differential equation 
    <men xml:id="eqn-diffsol3">
      \frac{\,d^{2}y}{\,dx^{2}}=x
    </men>
    Integrating both sides, we get -
    <me>
       \int\,d\left(\frac{\,dy}{\,dx}\right)=\int x\,dx
    </me>
    or,
    <men xml:id="eqn-diffsol4">
    \frac{\,dy}{\,dx}=\frac{x^{2}}{2}+C  
    </men>
    Integrating again, we get -
    <men xml:id="eqn-diffsol5">
      y=\frac{x^{3}}{6}+Cx+D
    </men>
    The eqn. <xref ref="eqn-diffsol5"/> is the general solution of differential eqn. <xref ref="eqn-diffsol3"/> 
    and C and D are two arbitrary constants. Hence it is clear from eqns. <xref ref="eqn-diffsol2"/> and 
    <xref ref="eqn-diffsol5"/> that if the order of differential equation is one the solution contains only 
    one arbitrary constant but if it is second ordered then its solution also contains two arbitrary constants. 
    The number of arbitrary constants in the solution is equal to the order of the differential equation. 
    An equation containing dependent variable y, independent variable x and free from derivative which 
    also satisfies the differential equation is called the <term>solution of the differential equation</term>. 
    The general solution becomes a particular solution by assigning the particular value of arbitrary 
    constant. Suppose we find C = 1 and D = 2 for eqn. <xref ref="eqn-diffsol5"/> then,
    <m>y=\frac{x^{3}}{6}+Cx+D</m> is the particular solution of differential eqn. <xref ref="eqn-diffsol3"/>.
    </p>
     </introduction>
 
 <subsection xml:id="subsec-first_order-diff">
  <title>First Order Linear Differential Equation</title>
  <p>
    The first order linear differential equation is obtained by putting <m>n = 1</m> in the standard form 
    of linear equation <xref ref="eqn-diffeq1"/>, i.e., 
    <me>
       f_{o}(x)\frac{\,dy}{\,dx}+ f_{o}(x)y =F(x)
    </me>
    or,
    <men xml:id="eqn-diffsol6">
      \frac{\,dy}{\,dx}+P(x)y = Q(x)
    </men>
    where <m>P(x)</m> and <m>Q(x)</m> are functions of <m>x</m> or constants. 
    To find its solution, first consider the homogeneous equation by setting <m>Q(x) = 0</m>.
    <me>
      \frac{\,dy}{\,dx}+P(x)y = 0 
    </me>
    <me>
       \frac{1}{y}\frac{\,dy}{\,dx} =-P(x)y
    </me>
    integrating, we get - 
    <me>
      \log y =-\int P(x)\,dx +C
    </me>
    where <m>C</m> is an arbitrary constant of integration.
    <me>
       y=exp\left[-\int P(x)\,dx +C\right] = exp\left[-\int P(x)\,dx\right]e^{C}
    </me>
    or,
    <me>
       y=A exp\left[-\int P\,dx\right]
    </me>
    where <m>A=e^{C}</m>.
   
    <me>
      \text{or,} \quad ye^{\int P\,dx}=A
    </me>
    Let,
    <me>
      I = \int P(x)\,dx \quad \text{so that}\quad \frac{\,dI}{\,dx} =P(x)
    </me>
    <men xml:id="eqn-diffsol7">
      \therefore \quad ye^{I}=A
    </men>
    Differentiate eqn. <xref ref="eqn-diffsol7"/>w.r.t. 'x', we get -
    <me>
      \frac{\,d}{\,dx}\left(ye^{I}\right)=0 
    </me>
    or,
    <me>
      \frac{\,dy}{\,dx}e^{I}+ye^{I}\frac{\,dI}{\,dx}=0
    </me>
    or,
    <me>
      \frac{dy}{dx}e^{I}+ye^{I}P=0
    </me>
    or,
    <men xml:id="eqn-diffsol8">
      e^{I}\left(\frac{dy}{dx}+yP\right)=0
    </men>
    Now multiplying eqn. <xref ref="eqn-diffsol6"/> by <m>e^{I} </m>, we get -
    <men xml:id="eqn-diffsol9">
     \left(\frac{\,dy}{\,dx}+Py\right)e^{I}=Qe^{I} 
    </men>
    which by using eqn. <xref ref="eqn-diffsol9"/>, becomes
    <men xml:id="eqn-diffsol10">
      \frac{\,d}{\,dx}\left(ye^{I}\right)=Qe^{I}
    </men>
    Integrating, we get - 
    <me>
      ye^{I}=\int Qe^{I}\,dx+C_{1}
    </me>
      where <m>C_{1}</m> is an arbitrary constant.
      <men xml:id="eqn-diffsol11">
         \text{or,} \quad ye^{\int P\,dx}=\int\left(Qe^{\int P\,dx}\right)\,dx+C_{1}
      </men>
     This is  the required solution and the factor <m>e^{\int P\,dx}</m> is known as 
     <term>integration factor (I.F.)</term>. Therefore the solution of first order linear 
     differential equation can be easily found by the formula  
     <me>
       y[I.F.] = \int Q[I.F.]\,dx + \quad\text{constant}.
     </me>
     Equation <xref ref="eqn-diffsol11"/> may be written as
     <men xml:id="eqn-diffsol12">
      y=C_{1}e^{-\int P\,dx}+e^{-\int P\,dx}\int\left(Qe^{\int P\,dx}\right)\,dx
     </men>
     i.e. the general solution of differential equation <xref ref="eqn-diffsol6"/> consists of two parts.
     <men xml:id="eqn-diffsol13">
      y=cu+v  \quad  \text{(say)}
     </men>
     where <m>u= e^{-\int P\,dx }</m>  and  <m>v=e^{-\int P\,dx}\int\left(Qe^{\int P\,dx}\right)\,dx</m> 
     also <m>C_{1}=c </m>.
    </p>
    <p>
      Now differentiating <m>u= e^{-\int P\,dx }</m> with respect to 'x', we have
      <me>
        \frac{\,du}{\,dx} =-P e^{-\int P\,dx}=-Pu
      </me>
      or,
      <me>
        \frac{\,du}{\,dx} +Pu =0 
      </me>
      or,
      <me>
        \frac{\,d(cu)}{\,dx} +P(cu) =0
      </me>
      which shows that <m>y=cu</m> is the solution of <m>\frac{\,du}{\,dx} +Pu =0</m>, again, differentiating 
      <me>
         v=e^{-\int P\,dx}\int\left(Qe^{\int P\,dx}\right)\,dx
      </me>
      w.r.t. 'x', we have -
      <me>
         \frac{\,dv}{\,dx}=-Pe^{-\int P\,dx}\left(Qe^{\int P\,dx}\right)\,dx + e^{-\int P\,dx}Qe^{\int P\,dx}
      </me>
      or,
      <me>
         \frac{\,dv}{\,dx} =-Pv+Q 
      </me>
      <me>
       \text{or,}\quad  \frac{\,dv}{\,dx} +Pv=Q 
      </me>
      which shows that <m>y=v</m> is the solution of <m>\frac{\,dy}{\,dx} +Py=Q</m>.
       Hence, the first part of the solution of differential equation is the solution of its 
       homogeneous equation and <m>cu </m> is known as <term>Complementry Function</term>. 
       Second part is free from any arbitrary constant and <m>v</m> is known as <term>Particular Integral</term>. 
       <m>\therefore</m> <term>Complete Solution = Complementry Function + Particular Integral</term>. That is,
       <me>
         y   =    C.F.   +    P.I.
       </me>
      </p>
 </subsection>

<subsection xml:id="subsec-second_order-diff">
  <title>Second Order Linear Differential Equations</title>
  <introduction>
     <p>
    Putting <m>n = 2</m> in the standard form of linear differential equation <xref ref="eqn-diffeq1"/>
    gives the second order linear differential equation.
    <me>
      f_{o}(x)\frac{\,d^{2}y}{\,dx^{2}}+f_{1}(x)\frac{\,dy}{\,dx}+Qy=R
    </me>
    or,
    <me>
       \frac{\,d^{2}y}{\,dx^{2}}+P\frac{\,dy}{\,dx}+Qy=R
    </me>
    where <m>P {,} Q</m>, and <m>R</m> are functions of <m>x</m> or constants.
    </p>
    <p>
       The method for finding the solution of linear differential equations is depends on the nature 
       of <m>P</m> and <m>Q</m>. If <m>P</m> and <m>Q</m> are constants then the differential 
       equation is said to be second order linear differential equation with constant coefficients. 
       But if <m>P</m> and <m>Q</m> are functions of <m>x</m> then the differential equation 
       is said to be differential equation with variable coefficients.
      </p>
  </introduction>
 
      <subsubsection xml:id="subsubsec-leqconst_coeff">
        <title>Linear Equations with Constant Coefficients</title>
        <p>
          The general form of linear differential equation of second order is 
        <men xml:id="eqn-diffsol14">
          	\frac{\,d^{2}y}{\,dx^{2}}+P\frac{\,dy}{\,dx}+Qy=R	
        </men>
        where <m>P</m> and <m>Q</m> are constants and <m>R</m> is a function of <m>x</m> or constant. 
        In the operator form,
        <me>
          (D^{2}+PD+Q)y = R [f(D)]y=R 
        </me>
        where,
        <me>
          \frac{\,d}{\,dx}\equiv D.
        </me>
          </p>
     

            <ol marker="a.">
            <li> 
              <p>
               Let <m>y=Ce^{mx}</m> be the trial solution of <m>C. F.</m> of eqn. <xref ref="eqn-diffsol14"/> 
              with m being root of the equation, then it satisfies the equation.
              <me>
                \therefore \quad \frac{\,dy}{\,dx}= mCe^{mx} = my
              </me>
              or,
              <me>
                \frac{\,d^{2}y}{\,dx^{2}}=m^{2}Ce^{mx} =m^{2}y
              </me>
              from eqn. <xref ref="eqn-diffsol14"/>,
              <me>
                m^{2}y+Pmy+Qy=0  \quad [\because  R=0]
              </me>
              or,
              <me>
                (m^{2}+Pm+Q)y =0.
              </me>
              <me>
               \text{Since}, y=\frac{R}{f(D)}
              </me>
              or,
              <me>
                 \frac{R}{f(m)}\neq 0
              </me>
              or,
              <me>
                \therefore \quad m^{2}+Pm+Q=0.
              </me>
              It is called an <term>Auxiliary Equation (A.E.)</term>. Which is quadratic in m (or D), 
              roots of which can be appeared by three ways. Viz. real and unequal, real and equal, 
              or a complex pair. Also it should be noted that if <m>y_{1}</m> and <m>y_{2}</m> are two 
              linearly independent solution of the corresponding homogenous equation then 
              <m>y=C_{1}y_{1}+C_{2}y_{2}</m>. The condition for <m>y_{1}</m> and <m>y_{2}</m> to be linearly 
              independent is 	
              <me>
                \begin{vmatrix} 
                y_{1} &amp; y_{2}\\ 
                y'_{1} &amp; y'_{2} 
                \end{vmatrix} \neq 0
              </me>
               This determinant is called <term>Wornskian</term> of <m>y_{1}</m> and <m> y_{2}</m>.
              </p>
              
               <p>
                 <alert>Case I. Roots are real and unequal:</alert> 
               If <m> m_{1}</m> and <m>m_{2}</m> are the roots of an A.E. then a C.F. is given by
               <me>
                y=C_{1}e^{m_{1}x}+C_{2}e^{m_{2}x} = C_{1} y_{1}+C_{2} y_{2}.
               </me>
               The wronskian for <m>y_{1}</m> and <m>y_{2}</m> is 
               <me>
                \begin{vmatrix} 
                C_{1}e^{m_{1}x} &amp; C_{2}e^{m_{2}x}\\ 
                m_{1}C_{1}e^{m_{1}x} &amp; m_{2}C_{2}e^{m_{2}x} 
                \end{vmatrix} 
               </me>
                since <m>m_{1}  \neq m_{2}</m>.  The wronskian <m>\neq 0</m>.  Hence <m>y_{1}</m> and 
                <m>y_{2}</m> are linearly independent.
               </p>
              <p>
                <alert>Case II. Roots are real and equal:</alert>
            If <m>m_{1} = m_{2} =m </m> (say), then C.F. is <m>y=(C_{1}+C_{2}x)e^{mx}</m>. why?
             </p>
             <p>
              If <m>m_{1} = m_{2} =m </m> then from case I, <m>y=(C_{1}+C_{2})e^{mx} =Ce^{mx}</m>. 
              Where C is only one constant in this solution. But the order of given equation is two 
              the solution must contain two constants in order to satisfy the given equation. 
              Hence we have to seek its solution by another way. Let's write equation 
              <xref ref="eqn-diffsol14"/> in the form
            <me>
              (D-m)(D-m)y=0
            </me>
            put 
            <me>
             (D-m)y=z 
            </me>
            then,
            <me>
             (D-m)z=0
            </me>
            or,
            <me>
              Dz-mz=0
            </me>
            or,
            <me>
               \frac{\,dz}{\,dx}-mz=0 \quad\Rightarrow z=Ae^{mx}
            </me>
            Thus,
            <me>
               (D-m)y=Ae^{mx}
            </me>
            or,
            <me>
               \frac{\,dy}{\,dx}-my=Ae^{mx}.
            </me>
            which is an inhomogenous first order linear differential equation. whose integrating factor is given by 
            <me>
              I.F. = e^{\int P\,dx}=e^{-mx}
            </me>
            Hence, the solution of this differential equation is given by equation <xref ref="eqn-diffsol11"/>
            <me>
              ye^{-mx} = \int Ae^{mx}\cdot e^{-mx}\,dx+B = \int A\,dx+B=Ax+B 
            </me>
            <me>
              \therefore  \quad y=(Ax+B)e^{mx}.
            </me>
             </p>
             <p>
              <term>Case III. Roots are imaginary pair.</term> 
              If the roots are <m>\alpha \pm i\beta,</m> then the solution will be
              <me>
                 y=C_{1}e^{(\alpha + i\beta)x}+C_{2}e^{(\alpha - i\beta)x} = e^{\alpha x}\left[C_{1}e^{i\beta x}+C_{2}e^{-i\beta x}\right]
              </me>
              <me>
                = e^{\alpha x}\left[C_{1}(\cos\beta x+i\sin\beta x)+C_{2}(\cos\beta x-i\sin\beta x)\right]
              </me>
              <me>
                  =e^{\alpha x}\left[(C_{1}+C_{2})\cos\beta x+i(C_{1}-C_{2})\sin\beta x)\right]
              </me>
              <me>
                  =e^{\alpha x}\left[A\cos\beta x+iB\sin\beta x)\right]
              </me>
              <me>
                 =Ce^{\alpha x}\sin(\beta x+\gamma).
              </me>
              where C and <m> \gamma</m> are arbitrary constants.
             </p>
            </li>
            <li>
              <p>
                There are various methods to find the particular integral of a differential equation, 
                here we discuss some of the easy methods.
              </p>
              </li>
          </ol>
           </subsubsection>  


<subsubsection xml:id="subsubsec-PI-funct">
  <title>General Method of Finding the Particular Integral of Any Function <m>\phi(x)</m></title>
  <p>
    <me>
      P.I.=\frac{1}{D-a}\phi(x) =v
    </me>
    or,
    <me>
      \phi(x) = (D-a)v
    </me>
    or,
    <me>
      \phi(x) = Dv-av
    </me>
    or,
    <me>
      \frac{\,dv}{\,dx}-av = \phi(x)
    </me>
    which is a first order linear differential equation. Its solution is  
    <me>
      ve^{-\int a\,dx}=\int e^{-\int a\,dx}\phi(x)\,dx =\int e^{-ax}\phi(x) \,dx
    </me>
    <men xml:id="eqn-pisol1">
      \therefore \quad v=e^{ax}\int e^{-ax}\phi(x)\,dx=P.I.
    </men>
    Particular Integral can also be obtained by inspection method which will be discussed 
    in examples given below. However, there may be developed a general method for solving 
    the differential equation directly, called the successive integration method. 
    Let the equation in the form 
    <men xml:id="eqn-pisol2">
      (D^{2}+PD+Q)y=f(x)
    </men>
    If <m>m_{1}=a</m> and <m>m_{2}=b</m> are the roots of A.E., then eqn. <xref ref="eqn-diffsol14"/> 
    can be written as 
    <men xml:id="eqn-pisol3">
      (D-a)(D-b)y=f(x)
    </men>
    put,
    <me>
       (D-b)y=v
    </me>
    so that 
    <me>
      (D-a)v=f(x)
    </me>
    or,
    <me>
       \frac{\,dv}{\,dx}-av=f(x)
    </me>
    Its solution is 
    <me>
      v\cdot e^{-\int a\,dx}=\int f(x)e^{-\int a\,dx}\,dx+C_{1}
    </me>
    <men xml:id="eqn-pisol4">
      \therefore \quad v= e^{ax}\int f(x) e^{-ax}\,dx+C_{1} e^{ax}
    </men>
    from eqn. <xref ref="eqn-pisol3"/>, we have
    <me>
       (D-b)y=e^{ax}\int f(x)e^{-ax}\,dx+C_{1}e^{ax}
    </me>
    or,
    <me>
      \frac{\,dy}{\,dx}-by=\bar{Q}(x)
    </me>
    or,
    <men xml:id="eqn-pisol5">
       \therefore  \quad y=e^{bx}\int\bar{Q}(x)e^{-bx}\,dx+C_{2}e^{bx}
    </men>
    where,
    <men xml:id="eqn-pisol6">
      \bar{Q}(x)=e^{ax}\int f(x) e^{-ax}\,dx+C_{1}e^{ax}
    </men>
    </p>
</subsubsection>

<subsubsection xml:id="subsubsec-var_coef">
  <title>Linear Equations with Variable Coefficients</title>
  <p>
    The linear equation of the form
    <me>
      f_{o}(x)\frac{\,d^{2}y}{\,dx^{2}}+f_{1}(x)\frac{\,dy}{\,dx}+f_{2}(x)y=F(x)
    </me>
    or,
    <me>
      \frac{\,d^{2}y}{\,dx^{2}}+P\frac{\,dy}{\,dx}+Qy=X
    </me>
    is called a linear differential equation with variable coefficient if <m>P {,} Q</m> and <m>X</m> 
    are function of <m>x</m> only.
    </p>
    <p>In fact, there is no general method to solve such differential equations. 
    However, we discuss one artificial but elegent method to solve such type of equations. 
    This method is known as <term>Method of Variation of Parameters</term>. 
    Lagrange developed it. It provides the complete solution of a linear equation whose 
    complementary function is known.
    </p>
    <p>Let the equation is
    <men xml:id="eqn-varcoef1">
      \frac{\,d^{2}y}{\,dx^{2}}+P(x)\frac{\,dy}{\,dx}+Q(x)y=X(x) 
    </men>
    The C.F. of which is given as
   <men xml:id="eqn-varcoef2">
    y=v_{1}y_{1}+v_{2}y_{2}
   </men>
   where <m>y_{1}</m> and <m>y_{2}</m> are two linearly independent solution of the 
   correspnding homogenous eqn. i.e.,	
    <men xml:id="eqn-varcoef3">
      y''_{1}+Py'_{1}+Qy_{1} =0
    </men>
    <men xml:id="eqn-varcoef4">
      y''_{2}+Py'_{2}+Qy_{2} =0
    </men>
    clearly equation <xref ref="eqn-varcoef2"/> will not satisfy the given equation 
    <xref ref="eqn-varcoef1"/>. As <m>X(x) \neq 0 </m>, so we should consider the 
    constants <m>v_{1}</m> and <m>v_{2}</m> as unknown parameters which are the functions of <m>x</m>, then  
    <men xml:id="eqn-varcoef5">
      y=v_{1}y_{1}+v_{2}y_{2}	 
    </men>
    be a complete solution of the given equation <xref ref="eqn-varcoef1"/>. Hence equation 
    <xref ref="eqn-varcoef5"/> must satisfy the equation <xref ref="eqn-varcoef1"/>.
      Now,
      <men xml:id="eqn-varcoef6">
         y' = v'_{1}y_{1}+v_{1}y'_{1}+v'_{2}y_{2}+v_{2}y'_{2}
      </men>
      If we set,
      <men xml:id="eqn-varcoef7">
         v'_{1}y_{1}+v'_{2}y_{2} =0
      </men>
      by assuming <m> v_{1}</m> and <m>v_{2} </m> to be the arbitrary constants for complementary 
      part of the equation. Then,
      <men xml:id="eqn-varcoef8">
         y' = v_{1}y'_{1}+v_{2}y'_{2}
      </men>
      and 
      <men xml:id="eqn-varcoef9">
         y''= v'_{1}y'_{1}+v_{1}y''_{1}+v'_{2}y'_{2}+v_{2}y''_{2}
      </men>
      Therefore, from given eqn. <xref ref="eqn-varcoef1"/>, we have -
      <me>
        v'_{1}y'_{1}+v_{1}y''_{1}+v'_{2}y'_{2}+v_{2}y''_{2}+P(v_{1}y'_{1}+v_{2}y'_{2})+Q(v_{1}y_{1}+v_{2}y_{2})=X
      </me>
      or, 
      <me>
         v_{1}(y''_{1}+Py'_{1}+Qy_{1})+v_{2}(y''_{2}+Py'_{2}+Qy_{2})+(v'_{1}y'_{1}+v'_{2}y'_{2})=X
      </me>
      from eqns. <xref ref="eqn-varcoef3"/> and <xref ref="eqn-varcoef4"/>, 
      we have the first two terms equal to zero.
      <men xml:id="eqn-varcoef10">
        \therefore \quad v'_{1}y'_{1}+v'_{2}y'_{2}=X
      </men>
      Solving eqns. <xref ref="eqn-varcoef7"/> and <xref ref="eqn-varcoef10"/>, we get -
      <me>
        \left.\begin{aligned}
        v'_{1}y'_{1}+v'_{2}y'_{2}=X \\
        v'_{1}y_{1}+v'_{2}y_{2}=0 
        \end{aligned}\right\}
      </me>
      multiplying top equation by <m>y_{2}</m> and bottom equation by <m>y'_{2}</m> we get-
      <me>
        v'_{1}(y'_{1}y_{2}-y_{1}y'_{2} = Xy_{2}
      </me>
      <me>
        \therefore \quad v'_{1} = \frac{-Xy_{2}}{y_{1}y'_{2}-y'_{1}y_{2}}
      </me>
      and 
      <me>
        v'_{2} = \frac{Xy_{1}}{y_{1}y'_{2}-y'_{1}y_{2}}
      </me>
      <men xml:id="eqn-varcoef11">
        \therefore v'_{1} = \frac{-Xy_{2}}{|W|} \quad \text{and}  \quad v'_{2} = \frac{Xy_{1}}{|W|}
      </men>
      where 
      <me>
        |W| = y_{1}y'_{2}-y'_{1}y_{2} =\begin{vmatrix}
        y_{1} &amp; y_{1}\\
        y'_{1} &amp; y'_{2}
        \end{vmatrix}
      </me>
      is known as the Wronskian for solutions <m>y_{1}</m> and <m>y_{2}</m>. 
      Which does not equal to zero if <m>y_{1}</m> and <m>y_{2}</m> are two 
      linearly independent solution of eqn. <xref ref="eqn-varcoef1"/>.
    </p>
    <p>
       Integrating eqn. <xref ref="eqn-varcoef11"/>, we get - 
       <men xml:id="eqn-varcoef12">
        v_{1} = -\int\frac{Xy_{2}}{|W|}	\,dx+C_{1};  \qquad  v_{2} = \int\frac{Xy_{1}}{|W|}\,dx+C_{2}
       </men>
       Substituting <m>v_{1}</m> and <m>v_{2}</m> in equation <xref ref="eqn-varcoef5"/>, we get -
       <men xml:id="eqn-varcoef13">
        y(x) = y_{1}(x)\left[-\int\frac{Xy_{2}}{|W|}\,dx+C_{1}\right]+y_{2}(x)\left[\int\frac{Xy_{1}}{|W|}\,dx+C_{2}\right]
       </men>
       <term>Note:</term>
        There are no specific method to solve the differential equation with variable 
        coefficients but it can be solved by many method according to the type of eqution. 
        If the equation containing decreasing power of x then put <m>x=e^{z}</m> 
        so that equation can be converted into variable coefficient to constant coefficient. 
        Here are some rules which help us to find the complementary function of the given 
        differential equation. When C.F. is not easily obtained we should use <term>Power Series</term> 
        method to solve such equation.
      </p>
      <p>
         Assume 
        <ol marker="i.">
          <li>
            <m>y_{1}=e^{mx}</m> be a known integral of C.F.  if <m>m^{2}+mP+Q=0</m>.
          </li>
          <li>
            <m>y_{1}=e^{x}</m> be a known integral of C.F.  if <m>1+P+Q=0 </m>.
            </li>
            <li>
              <m>y_{1}=e^{-x} </m> be a known integral of C.F.  if <m>1-P+Q=0</m>.
              </li>
              <li>
                <m>y_{1}=x </m> be a known integral of C.F.  if <m>P+Qx=0</m>. 
                </li>
                <li>
                 <m>y_{1}=x^{2}</m> be a known integral of C.F.  if <m>2+2Px+Qx^{2}=0 </m>.
                  </li>
            <li>
              and put <m>y=vy_{1}</m> be the solution of corresponding homogeneous differential 
              equation. Where <m>v</m> is any parameter depends on <m>x</m>.
              </li>
        </ol>
        </p>
</subsubsection>
</subsection>
  </section>

