<?xml version="1.0" encoding="UTF-8"?>

<section xml:id="sec_first-curvcord" xmlns:xi="http://www.w3.org/2001/XInclude">
      <title>Curvilinear Coordinates</title>
    <introduction>
    <p>
<idx><h>curvilinear coordinates</h></idx> In physics many coordinate systems have been 
develeoped to solve a problem of particular geometries. We can use a cartesian coordinate 
system to solve a problem of any kind but finding the solutions of become very tedious. 
Hence to make things easier some other systems of coordinates such as polar coordinates, 
cylindrical coordinates, and spherical coordinates are designed. Curvilinear coordinate 
is used to obtain an easy solution for specific problems, especially when we are solving 
vector equations. Curvilinear coordinates are useful in many areas of physics and engineering, 
where problems may be more naturally described in terms of non-Cartesian coordinate systems. 
For example, the motion of objects in a gravitational field is often more easily described 
in terms of spherical coordinates, and the behavior of fluids in a pipe may be more easily 
described in terms of cylindrical coordinates.
</p>
<p>
In curvilinear co-ordinates, at least one of the coordinate axes is 
curved and the direction of unit vectors vary with their position. Hence the time derivatives 
of unit vectors are non-zero. In a <em>Cartesian (rectangular) coordinate system</em>, the coordinate 
lines are straight and intersect at right angles, but in a <em>curvilinear coordinate system</em>, 
the coordinate lines are curved and may intersect at oblique angles. 
Let us consider a coordinate system where the rectangular co-ordinates <m>(x,y,z)</m> can be expressed as
<men xml:id="eqn-curvcord1">
  x=f_{1}(u,v,w){,} y= f_{2}(u,v,w){,} z=f_{3}(u,v,w)
</men>
and on solving eqn. <xref ref="eqn-curvcord1"/>, we will get the values of <m>u</m>, <m>v</m>, <m>w</m>  
in terms of <m>x</m>, <m>y</m>, and <m>z</m>, i.e. 
<men xml:id="eqn-curvcord2">
  u=g_{1}(x,y,z){,} v=g_{2}(x,y,z){,}  w=g_{3}(x,y,z)
</men>
The parameters <m>u</m>, <m>v</m>, <m>w</m> are three surfaces such that <m>u = constant</m>, <m>v =  constant</m>, 
and <m>w = constant</m>. If these surfaces are intersecting at a point <m>P</m> whose rectangular 
coordinates are <m>x,y,z</m>, then (<m>u,v,w</m>) are called curvilinear coordinates of <m>x,y,z</m>. 
The surfaces <m>u,v,w</m> are called coordinates surfaces. Each pair of these coordinate surfaces 
intersect in curves called the coordinate curves. One coordinate is variable on each of the  
coordinate curves. The curve on which <m>u</m> - varies is known as <m>u-curve</m>. 
Similarly <m>v</m> and <m>w</m> curves can be defined. One coordinate is constant on each of the 
coordinate surfaces. The surface on which <m>u</m> is constant is known as <m>u-surface</m>.  
Similarly  <m>v</m> and <m>w</m> surfaces are defined, as shown in <xref ref="fig-fig28"/>.
    </p>
      <figure xml:id="fig-fig28">
    <caption></caption>
    <image source="fig28.png" width ="35%"/>
</figure>
<p>
  Let <m>\vec{r}=x\hat{i}+y\hat{j}+z\hat{k}</m> be the  position vector of point P in a rectangular coordinate system, 
  Then, 
  <me>
    \vec{r}=f_{1}(u,v,w)\hat{i}+f_{2}(u,v,w)\hat{j}+f_{3}(u,v,w)\hat{k}  =\vec{F_{1}}(u,v,w)
  </me>
  Say, <m>\vec{F_{1}}(u,v,w) =\vec{r}(u,v,w)</m> for simplicity. Then, 
  <men xml:id="eqn-curvcord3">
    \vec{\,dr}=\frac{\partial\vec{r}}{\partial u}\,du+\frac{\partial\vec{r}}{\partial v}\,dv+\frac{\partial\vec{r}}{\partial w}\,dw   
  </men>
  Where <m>\frac{\partial\vec{r}}{\partial u}</m> is a tangent vector to <m>u</m>-curve at P. If 
  <m>\hat{e_{1}}</m> is a unit tangent vector at P on <m>u</m>-curve then,
  <me>
    \frac{\partial\vec{r}}{\partial u}=h_{1}\hat{e_{1}},\quad \frac{\partial\vec{r}}{\partial v}=h_{2}\hat{e_{2}}, \quad \frac{\partial\vec{r}}{\partial w}=h_{3}\hat{e_{3}}
  </me>
  <me>
    \left[\because  \hat{e_{1}} = \frac{\frac{\partial\vec{r}}{\partial u}}{\mid\frac{\partial\vec{r}}{\partial u}\mid},\quad h_{1}=\mid\frac{\partial\vec{r}}{\partial u}\mid\right] 
  </me>
  where <m>h_{1}, h_{2}, h_{3}</m> are called scalar factors.
  <men xml:id="eqn-curvcord4">
    \therefore  \vec{\,dr}= h_{1}\hat{e_{1}}\,du + h_{2}\hat{e_{2}}\,dv 
    +h_{3}\hat{e_{3}}\,dw \equiv \,ds 
  </men>
  here <m>\,ds</m> is a magnitude of <m>\vec{\,dr}</m>. If the coordinate surfaces intersect at right angles, 
  then the curvilinear coordinates are called the orthogonal curvilinear coordinates. The coordinate 
  curves <m>u,v,w</m> are then analogous to the <m>x,y,z</m> coordinate axes of a rectangular system. 
  Let us consider a very small parallelopiped whose diagonal is <m>\,ds</m> and faces coincides with 
  surface <m>u</m> or <m>v</m> or <m>w</m> and the length of edges are 
  <m>\,ds_{1}=h_{1}\,du, \quad \,ds_{2}=h_{2}\,dv,</m> and <m>\,ds_{3}=h_{3}\,dw</m>. 
    Then, 
    Volume of parallelopiped =
  <men xml:id="eqn-curvcord5">
     \,ds_{1}\,ds_{2}\,ds_{3} = h_{1}h_{2}h_{3}\,du\,dv\,dw
  </men>
  from eq. <xref ref="eqn-curvcord4"/>, we have -
  <men xml:id="eqn-curvcord6">
     \,ds^{2}=\vec{\,dr}\cdot\vec{\,dr}=h_{1}^{2}\,du^{2}+h_{2}^{2}\,dv^{2}+h_{3}^{2}\,dw^{2}
  </men>
  Let <m>\hat{N}_{1}, \hat{N}_{2}, \hat{N}_{3}</m> are the unit normal vectors on the surfaces 
  <m>u,v,w</m>, respectively, then 
  <me>
    \hat{N_{1}}=\frac{\vec{\nabla}u}{\mid\vec{\nabla}u\mid}; \quad \hat{N_{2}}=\frac{\vec{\nabla}v}{\mid\vec{\nabla}v\mid};\quad \hat{N_{3}}=\frac{\vec{\nabla}w}{\mid\vec{\nabla}w\mid}.
  </me>
  </p>
  </introduction>

    <subsection xml:id="subsec-grad_curvcord">
      <title>The Gradient in Curvilinear Coordinates</title>
      <p>
        Let <m>\phi</m> be the scalar function of orthogonal curvilinear coordinates <m>u,v,w</m>, then, 
         <idx>gradient in curv. coord.</idx> 
         <men xml:id="eqn-grad_curv1">
          \,grad \phi=\vec{\nabla}\phi = f_{1}\hat{e}_{1}+f_{2}\hat{e}_{2}+f_{3}\hat{e}_{3}
         </men>
         where <m>f_{1},f_{2},f_{3}</m> are to be determined. We know that 
         <me>
          \vec{\,dr}= h_{1}\hat{e}_{1}\,du+h_{2}\hat{e}_{2}\,dv+h_{3}\hat{e}_{3}\,dw
         </me>
         Now,
         <men xml:id="eqn-gradcurv2">
          \,d\phi=\vec{\nabla}\phi\cdot\vec{\,dr}=h_{1}f_{1}\,du+h_{2}f_{2}\,dv+h_{3}f_{3}\,dw
         </men>
         As, <m>\phi=\phi(u,v,w)</m>.
         <men xml:id="eqn-gradcurv3">
           \,d\phi= \frac{\partial\phi}{\partial u}\,du+\frac{\partial\phi}{\partial v}\,dv+\frac{\partial\phi}{\partial w}\,dw
         </men>
         from eqns. <xref ref="eqn-gradcurv2"/> and <xref ref="eqn-gradcurv3"/>, we get - 
         <me>
          h_{1}f_{1}=\frac{\partial\phi}{\partial u}\Rightarrow f_{1} = \frac{1}{h_{1}}\frac{\partial\phi}{\partial u}
         </me>
         Similarly,
         <me>
          f_{2} = \frac{1}{h_{2}}\frac{\partial\phi}{\partial v}, 
         </me>
         and 
         <me>
           f_{3} = \frac{1}{h_{3}}\frac{\partial\phi}{\partial w}
         </me>
         <me>
          \therefore \quad \vec{\nabla}\phi =\frac{1}{h_{2}}\frac{\partial\phi}{\partial u}\hat{e_{1}}+ \frac{1}{h_{2}}\frac{\partial\phi}{\partial v}\hat{e_{2}} +  \frac{1}{h_{3}}\frac{\partial\phi}{\partial w}\hat{e_{3}}
         </me>
         This indicates the del operator as 
         <me>
          \left[\vec{\nabla} = \frac{\hat{e_{1}}}{h_{1}}\frac{\partial}{\partial u}+ \frac{\hat{e_{2}}}{h_{2}}\frac{\partial}{\partial v}+\frac{\hat{e_{3}}}{h_{3}}\frac{\partial}{\partial w}\right] 
         </me>
        </p>
    </subsection>

  <subsection xml:id="subsec-div_curvcord">
    <title>The Divergence in Curvilinear Coordinates</title>
    <p>
       <idx>divergence in curv. coord.</idx> Let <m>\vec{F}=F_{1}\hat{e}_{1}+F_{2}\hat{e}_{2}+F_{3}\hat{e}_{3}</m> be the vector function of orthoganal 
      curvilinear coordinates <m>u,v,w</m>, then 
      <me>
        div\vec{F} =\vec{\nabla}\cdot\vec{F} 
      </me>
      <me>
        = \left(\frac{\hat{e_{1}}}{h_{1}}\frac{\partial}{\partial u}+ \frac{\hat{e_{2}}}{h_{2}}\frac{\partial}{\partial v}+\frac{\hat{e_{3}}}{h_{3}}\frac{\partial}{\partial w}\right)\cdot(F_{1}\hat{e_{1}}+F_{2}\hat{e_{2}}+F_{3}\hat{e_{3}})
      </me>
      <me>
        =\left(\frac{1}{h_{1}}\frac{\partial F_{1}}{\partial u}+ \frac{1}{h_{2}}\frac{\partial F_{2}}{\partial v}+\frac{1}{h_{3}}\frac{\partial F_{3}}{\partial w}\right) 
      </me>
      <me>
        = \frac{1}{h_{1}h_{2}h_{3}}\left[\frac{\partial}{\partial u}(F_{1}h_{2}h_{3})+\frac{\partial}{\partial v}(F_{2}h_{3}h_{1})+\frac{\partial}{\partial w}(F_{3}h_{1}h_{2})\right]
      </me>
      </p>
  </subsection>

<subsection xml:id="subsec-curl_curvcord">
  <title>The Curl in Curvilinear Coordinates</title>
  <p>
    <idx>curl in curv. coord.</idx> 
    <me>
      \,curl\vec{F} =\vec{\nabla}\times\vec{F} = \vec{\nabla}\times F_{1}\hat{e}_{1}+F_{2}\hat{e}_{2}+F_{3}\hat{e}_{3}
    </me>
    <me>
      =\left(\frac{\hat{e}_{1}}{h_{1}}\frac{\partial}{\partial u}+ \frac{\hat{e}_{2}}{h_{2}}\frac{\partial}{\partial v}+\frac{\hat{e}_{3}}{h_{3}}\frac{\partial}{\partial w}\right)\times(F_{1}\hat{e}_{1}+F_{2}\hat{e}_{2}+F_{3}\hat{e}_{3})
    </me>
    <me>
      = {\begin{vmatrix} 
       \hat{e}_{1} &amp; \hat{e}_{2} &amp; \hat{e}_{3} \\ 
        \frac{1}{h_{1}}\frac{\partial}{\partial u} &amp; \frac{1}{h_{1}}\frac{\partial}{\partial v}  &amp; \frac{1}{h_{1}}\frac{\partial}{\partial w} \\ 
         F_{1} &amp; F_{2} &amp; F_{3} 
          \end{vmatrix}}
    </me>
    <me>
      =\hat{e}_{1}\left[\frac{1}{h_{2}}\frac{\partial F_{3}}{\partial v} 
      -\frac{1}{h_{3}}\frac{\partial F_{2}}{\partial w}\right] - 
      \hat{e}_{2}\left[\frac{1}{h_{1}}\frac{\partial F_{3}}{\partial u} 
      -\frac{1}{h_{3}}\frac{\partial F_{1}}{\partial w}\right]
    </me>
    <me>
      + \hat{e}_{3}\left[\frac{1}{h_{1}}\frac{\partial F_{2}}{\partial u} 
      -\frac{1}{h_{2}}\frac{\partial F_{1}}{\partial v}\right]
    </me>
    <me>
      =\frac{\hat{e}_{1}}{h_{2}h_{3}}\left[\frac{\partial}{\partial v}(F_{3}h_{3}) 
      -\frac{\partial}{\partial w}(F_{2}h_{2})\right]
    </me>
    <me>
       + \frac{\hat{e}_{2}}{h_{3}h_{1}}\left[\frac{\partial}{\partial w}(F_{1}h_{1}) 
       -\frac{\partial}{\partial u}(F_{3}h_{3})\right]
    </me>
    <me>
       +\frac{\hat{e}_{3}}{h_{1}h_{2}}\left[\frac{\partial}{\partial u}(F_{2}h_{2}) 
      -\frac{\partial}{\partial v}(F_{1}h_{1})\right]
    </me>
    <me>
      \therefore  	\vec{\nabla}\times\vec{F}= {\begin{vmatrix} 
       h_{1}\hat{e}_{1} &amp; h_{2}\hat{e}_{2}  &amp; h_{3}\hat{e}_{3} \\ 
      \frac{\partial}{\partial u} &amp; \frac{\partial}{\partial v} &amp; \frac{\partial}{\partial w} \\ 
       F_{1}h_{1}  &amp; F_{2}h_{2}  &amp; F_{3}h_{3} 
        \end{vmatrix}} 
    </me>
    </p>
</subsection>

<subsection xml:id="subsec-lapl_curvcord">
  <title>Laplacian in Curvilinear Coordinate Systems</title>
  <p>
    <idx>Laplacian in curv. coord.</idx> 
    we know that <m>\nabla^{2}\psi=\vec{\nabla}\cdot\vec{\nabla \psi}</m>,	 
    put  <m>\vec{\nabla \psi}=\vec{F}</m>, then
    <me>
       \vec{\nabla}\cdot\vec{F} 
    </me>
    <men xml:id="eqn-lapcurv1">
     = \frac{1}{h_{1}h_{2}h_{3}}\left[\frac{\partial}{\partial u}(F_{1}h_{2}h_{3}) 
     +\frac{\partial}{\partial v}(F_{2}h_{3}h_{1}) 
     +\frac{\partial}{\partial w}(F_{3}h_{1}h_{2})\right]
    </men>
     also
    <me>
      \vec{F} = \vec{\nabla \psi} = \left(\frac{\hat{e_{1}}}{h_{1}}\frac{\partial \psi}{\partial u} 
      + \frac{\hat{e_{2}}}{h_{2}}\frac{\partial \psi}{\partial v} 
      +\frac{\hat{e_{3}}}{h_{3}}\frac{\partial \psi}{\partial w}\right) 
    </me>
    Hence, 
    <me>
       F_{1}= \frac{1}{h_{1}}\frac{\partial \psi}{\partial u}, \quad F_{2} 
       = \frac{1}{h_{2}}\frac{\partial \psi}{\partial v},\quad F_{3} 
       = \frac{1}{h_{3}}\frac{\partial \psi}{\partial w} 
    </me>
    and from eqn. <xref ref="eqn-lapcurv1"/>, 
    <me>
      \vec{\nabla}\cdot\vec{F} = \vec{\nabla}\cdot\vec{\nabla \psi} =  \nabla^{2}\psi 
    </me>
    <me>
      =  \frac{1}{h_{1}h_{2}h_{3}}\left[\frac{\partial}{\partial u}\left(\frac{h_{2}h_{3}}{h_{1}}\frac{\partial \psi}{\partial u}\right) 
      +\frac{\partial}{\partial v}\left(\frac{h_{3}h_{1}}{h_{2}}\frac{\partial \psi}{\partial v}\right) 
      +\frac{\partial}{\partial w}\left(\frac{h_{1}h_{2}}{h_{3}}\frac{\partial \psi}{\partial w}\right)\right]
    </me>
    which is the required expression. 
    </p>

    <p>
    <alert>Note:</alert> If <m>h_{1}=h_{2}=h_{3}=1</m>  and 
    <m>\hat{e}_{1}, \hat{e}_{2}, \hat{e}_{3}</m>, are replaced by <m>\hat{i}, \hat{j}, \hat{k}</m> 
    then all the above expressions reduce into usual expressions in rectangular coordinates where 
    <m>(u,v,w)</m> is replaced by <m>(x,y,z)</m>.
    </p>

</subsection>

<subsection xml:id="subsec-cylind_cord">
  <title>Cylindrical  Orthogonal Curvilinear Coordinates</title>
  <p>
    <idx>cylindrical curv. Coord.</idx> Let  the  curvilinear  coordinates of point P 
    in space be <m>(u,v,w)</m> and  corresponding  cartesian coordinates be <m>(x,y,z)</m>. The  
    projection  of  point P on  the z-plane is Q as shown in <xref ref="fig-fig29"/>, whose polar 
    coordinates  in this plane are <m>(\rho, \phi)</m>. The cylindrical coordinates of point P are 
    then specified by <m>(\rho, \phi, z)</m> where, <m>(\rho\geq 0, \quad 0\leq\phi\leq 2\pi,\quad -\infty \lt z \lt \infty)</m>. 
    The corresponding transformation into cartesian systems are 
    </p>
      <figure xml:id="fig-fig29">
    <caption></caption>
    <image source="fig29.png" width ="30%"/>
</figure>
<p>
  <men xml:id="eqn-cylind_cord1">
    x=\rho \cos\phi, \quad y= \rho\sin\phi, \quad z=z
  </men>
  Let <m>\vec{r}= x\hat{i}+y\hat{j}+z\hat{k}</m> be the position vector of point P in 
  a cartesian system, then we can write 
  <men xml:id="eqn-cylind_cord2">
    \vec{r}= \rho \cos\phi\hat{i}+\rho \sin\phi\hat{j}+z\hat{k} 
  </men>
  [from eqn. <xref ref="eqn-cylind_cord1"/>], in a cylindrical system.  
Now the tangent vectors of <m>\vec{r}</m>  in a cylindrical system are  
<me>
  \frac{\partial\vec{r}}{\partial \rho} = \cos\phi\hat{i}+\sin\phi\hat{j}+0.\hat{k}, 
</me>
<me>
  \frac{\partial\vec{r}}{\partial \phi} = -\rho\sin\phi\hat{i}+\rho\cos\phi\hat{j}+0.\hat{k},
</me>
<me>
\text{and} \quad   \frac{\partial\vec{r}}{\partial z} = \hat{k}.
</me>
But, scale factors are the magnitude of tangent vectors, then we have -
<me>
  h_{1}=\mid\frac{\partial\vec{r}}{\partial \rho}\mid = \sqrt{\cos^{2}\phi + \sin^{2}\phi}=1;
</me>
<me>
  h_{2}=\mid\frac{\partial\vec{r}}{\partial \phi}\mid = \rho ;
</me>
<me>
  \text{and} \quad h_{3}=\mid\frac{\partial\vec{r}}{\partial z}\mid = 1.
</me>
If <m>\hat{e}_{\rho}, \hat{e}_{\phi}, \hat{e}_{z}</m>  are the unit tangent vectors along the curves 
<m>u,v,w</m>, respectively then in cylindrical coordinates, we have - 
<me>
  \,grad\psi = \vec{\nabla\psi}= \frac{\hat{e}_{\rho}}{1}\frac{\partial\psi}{\partial \rho} 
  +\frac{\hat{e}_{\phi}}{\rho}\frac{\partial\psi}{\partial \phi}+\frac{\hat{e}_{z}}{1}\frac{\partial\psi}{\partial z},
</me>
<me>
  \left[\because   \vec{\nabla} = \frac{\hat{e_{1}}}{h_{1}}\frac{\partial}{\partial u} 
  +\frac{\hat{e_{2}}}{h_{2}}\frac{\partial}{\partial v} 
  +\frac{\hat{e_{3}}}{h_{3}}\frac{\partial}{\partial w}\right]
</me>
in curvilinear coordinates.
<me>
  \,div\vec{F} = \vec{\nabla}\cdot\vec{F} 
  = \frac{1}{\rho}\left[\frac{\partial}{\partial \rho}(F_{1}\rho) 
  +\frac{\partial}{\partial \phi}(F_{2}) 
  +\frac{\partial}{\partial z}(F_{3}\rho)\right],
</me>
<me>
  curl\vec{F} = \vec{\nabla}\times\vec{F}= {\begin{vmatrix}
\hat{e}_{\rho} &amp; \rho\hat{e}_{\phi} &amp; \hat{e}_{z} \\ 
\frac{\partial}{\partial \rho} &amp; \frac{\partial}{\partial \phi} &amp; \frac{\partial}{\partial z} \\
F_{1} &amp; \rho F_{2} &amp; F_{3}
\end{vmatrix}}
</me>
and 
<me>
 \nabla^{2}\psi 
 = \frac{1}{\rho}\left[\frac{\partial}{\partial \rho}\left(\rho\frac{\partial \psi}{\partial \rho}\right) 
 +\frac{\partial}{\partial \phi}\left(\frac{1}{\rho}\frac{\partial \psi}{\partial \phi}\right)) 
 +\frac{\partial}{\partial z}\left(\rho\frac{\partial \psi}{\partial z}\right)\right]
</me>
<me>
  =\frac{1}{\rho}\frac{\partial\psi}{\partial \rho} 
  + \frac{\partial^{2}\psi}{\partial \rho^{2}} 
  + \frac{1}{\rho^{2}}\frac{\partial^{2}\psi}{\partial \phi^{2}} 
  +\frac{1}{\rho}\frac{\partial^{2}\psi}{\partial z^{2}}.
</me>
we can also find the values of <m>h_{1},h_{2},h_{3}</m> as - 
<me>
  x=\rho \cos\phi, \quad y= \rho\sin\phi, \quad z=z,  
</me>
and 
<me>
  \rho^{2} = x^{2} + y^{2}, \quad   \phi= \tan^{-1}\frac{y}{x}, \quad  z=z. 
</me>
Now, if <m>x</m> is a function of <m>\rho, \phi, z</m>,  i.e. <m>x=x(\rho, \phi,z)</m>, then 
<me>
  \,dx=	 \frac{\partial x}{\partial \rho}\,d\rho + \frac{\partial x}{\partial \phi}\,d\phi 
  + \frac{\partial x}{\partial z}\,dz=\cos\phi \,d\rho-\rho \sin\phi d\phi+0.
</me>

<me>
 \text{similarly,} \,dy= \sin\phi \,d\rho+\rho \cos\phi \,d\phi+0, 
</me>
and
<me>
    \,dz=\,dz.
</me>
<me>
  \therefore  \,ds^{2}= \vec{dr}\cdot\vec{dr} = \,dx^{2}+\,dy^{2}+\,dz^{2} 
</me>
<men xml:id="eqn-cylind_cord3">
  = \,d\rho^{2}+\rho^{2}\,d\phi^{2}+\,dz^{2}
</men>

But in curvilinear coordinates, 
<men xml:id="eqn-cylind_cord4">
  \,ds^{2}= h_{1}^{2} \,du^{2}+h_{2}^{2} \,dv^{2}+h_{3}^{2} \,dw^{2}
</men>
equating eqns. <xref ref="eqn-cylind_cord3"/> and <xref ref="eqn-cylind_cord4"/>, we get -
</p>
  <p>
<m>h_{1} = 1,\quad h_{2}=\rho, \quad  h_{3}=1;</m> and <m>\hat{e}_{1} =\hat{e}_{\rho},\quad 
 \hat{e}_{2} =\hat{e}_{\phi}, \quad  \hat{e}_{3} =\hat{e}_{z}</m>.
</p>
</subsection>

<subsection xml:id="subsec-spher_cord">
  <title>Spherical  Orthogonal Curvilinear  Coordinates</title>
  <p>
    <idx>spherical curv. coord.</idx> Let <m>(u,v,w)</m> be the curvilinear coordinates of 
    point P and <m>(x,y,z)</m> be its corresponding cartesian coordinates. If <m>\vec{r}</m> be the position 
    vector of point P then the spherical coordinates of point P are specified by <m>(r, \theta, \phi)</m>, 
    as shown in <xref ref="fig-fig30"/>. where <m>r\geq 0, \quad 0\leq \theta \leq \pi, \quad 0\leq \phi \leq 2\pi</m>. 
    The corresponding transformation into cartesian systems are <m>x=OQ\cos\phi = O'P\cos\phi = r\sin\theta \cos\phi</m>, 
        <m>y=OQ\sin\phi = r\sin\theta \sin\phi</m>, and <m>z=PQ= OO'= OP\cos\theta = r\cos\theta</m>. 
    Here,
    <me>
      x=x(r{,}\theta{,}\phi)
    </me>
    or,
    <me>
      \,dx=  \frac{\partial x}{\partial r}\,dr +\frac{\partial x}{\partial \theta}\,d\theta 
      + \frac{\partial x}{\partial \phi}d\phi 
    </me>
    <me>
      = \sin\theta\cos\phi \,dr+ r\cos\theta\cos\phi \,d\theta-r\sin\theta \sin\phi \,d\phi 
    </me>
    Similarly,
    <me>
      \,dy=  \sin\theta\sin\phi \,dr+ r\cos\theta\sin\phi \,d\theta +r\sin\theta \cos\phi \,d\phi
    </me>
    and 
    <me>
      \,dz=  \cos\theta \,dr+ -r\sin\theta \,d\theta.
    </me>
    <me>
       \therefore \quad  \,ds^{2}= dx^{2}+dy^{2}+\,dz^{2}
    </me>
    <men xml:id="eqn-spher_cord1">
     = \,dr^{2}+r^{2}\,d\theta^{2}+r^{2}\sin^{2}\phi \,d\phi^{2}
    </men>
    </p>
      <figure xml:id="fig-fig30">
    <caption></caption>
    <image source="fig30.png" width ="30%"/>
</figure>
<p>
  But in curvilinear coordinates
  <me>
    \,ds^{2}= h_{1}^{2} \,du^{2}+h_{2}^{2} \,dv^{2}+h_{3}^{2} \,dw^{2}  
  </me>
  from eqn. <xref ref="eqn-cylind_cord4"/>. Equating eqns. <xref ref="eqn-cylind_cord4"/>
   and <xref ref="eqn-spher_cord1"/>, we get- 
   <me>
    h_{1} = 1,\quad h_{2}=r, \quad h_{3}=r\sin\theta,
   </me>
   and (u,v,w) is replaced by
   <m>(r, \theta, \phi)</m>, and <m>\hat{e}_{1} = \hat{e}_{r}{,} 
   \hat{e}_{2}=\hat{e}_{\theta}{,} 
   \hat{e}_{3} =\hat{e}_{\phi}</m>.
  </p>
  <p>
    <alert>Alternative method to find <m>h_{1},h_{2},h_{3}</m></alert>
    The position vector of point P in spherical coordinates is 
    <me>
      \vec{r}= x\hat{i}+y\hat{j}+z\hat{k} 
      = r\sin\theta \cos\phi\hat{i}+r\sin\theta \sin\phi\hat{j}+r\cos\theta\hat{k}
    </me>
    The tangent vectors of which is given as
    <me>
      \frac{\partial\vec{r}}{\partial r} 
      =\sin\theta \cos\phi\hat{i}+\sin\theta \sin\phi\hat{j}+\cos\theta\hat{k} \quad
       \Rightarrow h_{1}=\mid\frac{\partial\vec{r}}{\partial r}\mid =1.
    </me>
    <me>
       \frac{\partial\vec{r}}{\partial \theta} 
       =r\cos\theta \cos\phi\hat{i}+r\cos\theta \sin\phi\hat{j}-r\sin\theta\hat{k}\quad 
        \Rightarrow h_{2}=\mid\frac{\partial\vec{r}}{\partial \theta}\mid =r;
    </me>
    <me>
       \frac{\partial\vec{r}}{\partial \phi} 
       = -r\sin\theta \sin\phi\hat{i}+r\sin\theta \cos\phi\hat{j} \quad	
       \Rightarrow h_{3}=\mid\frac{\partial\vec{r}}{\partial \phi}\mid =r\sin\theta.
    </me>
    </p>
  <p>
    Now, substituting these values in different expressions in curvilinear system, we get - 
    <me>
      \vec{\nabla\psi}=\frac{\partial \psi}{\partial r}\hat{e_{r}} 
      +\frac{1}{r}\frac{\partial \psi}{\partial \theta}\hat{e_{\theta}} 
      +\frac{1}{r\sin\theta}\frac{\partial \psi}{\partial \phi}\hat{e_{\phi}};
    </me>
    <me>
      \vec{\nabla}\cdot\vec{F}=\frac{1}{r^{2}}\frac{\partial}{\partial r}(r^{2}F_{1}) 
      +\frac{1}{r\sin\theta}\frac{\partial}{\partial \theta}(\sin\theta F_{2}) 
      +\frac{1}{r\sin\theta}\frac{\partial F_{3}}{\partial \phi}
    </me>
    <me>
      \vec{\nabla}\times\vec{F} = \frac{1}{r\sin^{2}\theta}{\begin{vmatrix} 
      \hat{e}_{r} &amp; r\hat{e}_{\theta} &amp; r\sin\theta\hat{e}_{\phi} \\ 
      \frac{\partial}{\partial r} &amp; \frac{\partial}{\partial \theta} &amp; \frac{\partial}{\partial \phi} \\ 
      F_{1} &amp; r F_{2} &amp; r\sin\theta F_{3} 
      \end{vmatrix}}; 
    </me>
    <me>
      \nabla^{2}\psi 
      = \frac{1}{r^{2}\sin\theta} \left[\sin\theta\frac{\partial}{\partial r}\left(r^{2}\frac{\partial \psi}{\partial r}\right)
     +\frac{\partial}{\partial \theta}\left(\sin\theta \frac{\partial \psi}{\partial \theta}\right) 
     +\frac{1}{\sin\theta}\frac{\partial^{2}\psi}{\partial \phi^{2}}\right]
    </me>   
    <me>
      =\frac{1}{r^{2}}\frac{\partial}{\partial r}\left(r^{2}\frac{\partial \psi}{\partial r}\right)+
      \frac{1}{r^{2}\sin^{2}\theta}\frac{\partial}{\partial \theta}\left(\sin\theta\frac{\partial \psi}{\partial \theta}\right)
    </me>
    <me>
      + \frac{1}{r^{2}\sin^{2}\theta}\frac{\partial^{2}\psi}{\partial \phi^{2}}
    </me>
    <me>
      =\frac{\partial^{2} \psi}{\partial r^{2}} 
      +\frac{1}{r^{2}}\frac{\partial^{2} \psi}{\partial \theta^{2}} 
      +\frac{1}{r^{2}\sin^{2}\theta}\frac{\partial^{2}\psi}{\partial \phi^{2}}
    </me>
    <me>
      +\frac{2}{r}\frac{\partial \psi}{\partial r} 
      +\frac{\cot\theta}{r^{2}}\frac{\partial \psi}{\partial \theta}.
    </me>
    </p>
</subsection>
</section>

