<?xml version="1.0" encoding="UTF-8"?>

<section xml:id="sec_first-examplesC" xmlns:xi="http://www.w3.org/2001/XInclude">
  <title>Examples C</title>
<example>
  <statement>
    <p>
      Prove that a cylindrical coordinate system is orthogonal.
    </p>
  </statement>
  <solution>
    <p>
      The position vector of any point P in a cylindrical coordinate is 	
      <me>
        \vec{r}= x\hat{i}+y\hat{j}+z\hat{k}= \rho\cos\phi\hat{i}+\rho\sin\phi\hat{j}+z\hat{k}
      </me>
      Now,
      <me>
         \frac{\partial \vec{r}}{\partial \rho}, \frac{\partial \vec{r}}{\partial \phi}, \frac{\partial \vec{r}}{\partial z}
      </me>
      are the tangent vectors along the curves <m>\rho, \phi,z,</m>, respectively.
      <me>
        \therefore \quad  \frac{\partial \vec{r}}{\partial \rho} = \cos\phi\hat{i}+\sin\phi\hat{j},
      </me>
      <me>
        \frac{\partial \vec{r}}{\partial \phi} = -\rho\sin\phi\hat{i}+\rho\cos\phi\hat{j},
      </me>
      <me>
        \text{and} \quad \frac{\partial \vec{r}}{\partial z} = \hat{k}.
      </me>
      The unit vectors along the tangents are
      <me>
      \hat{e}_{1}=\hat{e}_{\rho}=\frac{\frac{\partial \vec{r}}{\partial \rho}}{\mid\frac{\partial \vec{r}}{\partial \rho}\mid}
      </me>
      <men xml:id="eqn-unit_vect1">
        = \frac{\cos\phi\hat{i}+\sin\phi\hat{j}}{\sqrt{\cos^{2}\phi + \sin^{2}\phi}} = \cos\phi\hat{i}+\sin\phi\hat{j},
      </men>
      <me>
        \hat{e}_{2}=\hat{e}_{\phi}=\frac{\frac{\partial \vec{r}}{\partial \phi}}{\mid\frac{\partial \vec{r}}{\partial \phi}\mid} 
      </me>
      <men xml:id="eqn-unit_vect2">
        = \frac{-\rho\sin\phi\hat{i}+\rho\cos\phi\hat{j}}{\sqrt{\rho^{2}\sin^{2}\phi + \rho^{2}\cos^{2}\phi}} = -\sin\phi\hat{i}+\cos\phi\hat{j},
      </men>
      <men xml:id="eqn-unit_vect3">
        \hat{e}_{3}=\hat{e}_{z}=\frac{\frac{\partial \vec{r}}{\partial z}}{\mid\frac{\partial \vec{r}}{\partial z}\mid} = \hat{k}
      </men>
      Then,
      <me>
        \hat{e}_{1}\cdot\hat{e}_{2} = (\cos\phi\hat{i}+\sin\phi\hat{j})\cdot(-\sin\phi\hat{i}+\cos\phi\hat{j}) = 0,
      </me>
      <me>
        \hat{e}_{1}\cdot\hat{e}_{3} = (\cos\phi\hat{i}+\sin\phi\hat{j})\cdot (\hat{k})=0,
      </me>
      and 
      <me>
        \hat{e}_{2}\cdot\hat{e}_{3} = (-\sin\phi\hat{i}+\cos\phi\hat{j})\cdot (\hat{k}) = 0.
      </me>
      Hence <m>\hat{e_{1}}, \hat{e_{2}}</m>, and  <m>\hat{e_{3}}</m> are mutually perpendicular 
      and the coordinate system is orthogonal.
    </p>
  </solution>
</example>
  
  <example>
    <statement>
      <p>
        Express the velocity <m>v</m> and acceleration <m>a</m> of a particle in cylindrical coordinates.
      </p>
    </statement>
    <solution>
      <p>
        The position vector of any point in a cylindrical coordinate is defined as 
        <me>
          \vec{r}= x\hat{i}+y\hat{j}+z\hat{k}= \rho\cos\phi\hat{i}+\rho\sin\phi\hat{j}+z\hat{k}
        </me>
        <me>
          =\rho\cos\phi(\cos\phi\hat{e}_{\rho}-\sin\phi\hat{e}_{\phi})+\rho\sin\phi(\sin\phi\hat{e}_{\rho}+\cos\phi\hat{e}_{\phi})+z\hat{e}_{z}
        </me>
        <me>
          =\rho\hat{e_{\rho}} +z \hat{e_{z}}
        </me>
        from solving the entities <xref first="eqn-unit_vect1" last="eqn-unit_vect3"/> 
        <me>
          \left[\hat{e}_{\rho}= \cos\phi\hat{i}+\sin\phi\hat{j}, \hat{e}_{\phi} = -\sin\phi\hat{i}+\cos\phi\hat{j}, \hat{e}_{z} = \hat{k}\right] 
        </me>
        We get -
        <men xml:id="eqn-unit_vect4">
          \hat{i}= \cos\phi\hat{e}_{\rho}-\sin\phi\hat{e}_{\phi},
        </men>
        <men xml:id="eqn-unit_vect5">
          \hat{j}= \sin\phi\hat{e_{\rho}}+\cos\phi\hat{e_{\phi}}, 
        </men>
        <men xml:id="eqn-unit_vect6">
          \hat{k}=\hat{e_{z}}
        </men>
        and,
        <me>
          \vec{v}= \frac{d \vec{r}}{d t} =  \frac{d\rho}{d t}\hat{e}_{\rho} +\rho\frac{d\hat{e}_{\rho}}{d t}+ 
          \frac{d z}{d t}\hat{e}_{z} +z\frac{d\hat{e}_{z}}{d t}
        </me>
        <me>
          = \dot{\rho} \hat{e_{\rho}}+\rho \hat{e_{\phi}}\dot{\phi} + \dot{z}\hat{e_{z}} +0
        </me>
        Again differentiating <m>v</m> w.r.to 't', we get -
        <me>
          \vec{a}=  \frac{d^{2} \vec{r}}{d t^{2}}	 = \frac{d}{dt}(\dot{\rho} \hat{e}_{\rho}+\rho \hat{e}_{\phi}\dot{\phi} + \dot{z}\hat{e}_{z})
        </me>
        <me>
          =\dot{\rho} \frac{d \hat{e}_{\rho}}{dt}+\ddot{\rho}\hat{e}_{\rho} + \rho\dot{\phi}\frac{d \hat{e}_{\phi}}{dt} + \rho\ddot{\phi} \hat{e}_{\phi} + \dot{\rho} \dot{\phi}\hat{e}_{\phi} + \ddot{z}\hat{e}_{z}
        </me>
        <me>
          =\dot{\rho}\dot{\phi}\hat{e}_{\phi} + \ddot{\rho}\hat{e}_{\rho}+\rho\dot{\phi}(-\dot{\phi}\hat{e}_{\rho})+\rho\ddot{\phi} \hat{e}_{\phi}+\dot{\rho} \dot{\phi}\hat{e}_{\phi} + \ddot{z}\hat{e}_{z}
        </me>
        <me>
          =(\ddot{\rho}-\rho\dot{\phi}^{2})\hat{e}_{\rho} +(\rho\ddot{\phi}+2\dot{\rho}\dot{\phi})\hat{e}_{\phi} + \ddot{z}\hat{e}_{z}
        </me>
        <fn>
        <me>
           \frac{\,d\hat{e}_{\rho}}{\,dt}= \frac{\,d\hat{e}_{\rho}}{\,d\phi}\cdot\frac{\,d\phi}{\,dt} = \dot{\phi}\hat{e}_{\phi}
        </me>
        after differentiating  <m>\hat{e}_{\rho}</m> w.r.to <m>'\phi'</m>; also 
        <me>
          \frac{\,d\hat{e}_{\phi}}{\,dt}= \frac{\,d\hat{e}_{\phi}}{\,d\phi}\cdot\frac{\,d\phi}{\,dt} = -\dot{\phi}\hat{e}_{\rho} 
        </me>
        after differentiating <m> \hat{e_{\phi}}</m> w.r.to <m>'\phi'</m>.
        </fn>
      </p>
    </solution>
  </example>

  <example>
    <statement>
      <p>
        Find an expression for <m>\,ds^{2}</m> in orthogonal curvilinear system.
      </p>
    </statement>
    <solution>
      <p>
        We know that the position vector 
        <me>
          \vec{r} = \vec{r}(u,v,w)
        </me>
        and 
        <me>
          \,ds^{2} = \vec{\,dr}\cdot\vec{\,dr} =\left(\frac{\partial \vec{r}}{\partial u} \,du + \frac{\partial \vec{r}}{\partial v} \,dv +\frac{\partial \vec{r}}{\partial w} \,dw\right)^{2}
        </me>
        <me>
          =\left(\frac{\partial \vec{r}}{\partial u}\right)^{2} \,du^{2}	
           +\left(\frac{\partial \vec{r}}{\partial v}\right)^{2} \,dv^{2}	
           + \left(\frac{\partial \vec{r}}{\partial w}\right)^{2} \,dw^{2}	
        </me>
        <me>
          + 2 \left(\frac{\partial \vec{r}}{\partial u}\right)\cdot \left(\frac{\partial \vec{r}}{\partial v}\right)dudv 
        </me>
        <me>
          + 2 \left(\frac{\partial \vec{r}}{\partial v}\right)\cdot \left(\frac{\partial \vec{r}}{\partial w}\right)\,dv\,dw + 
          2 \left(\frac{\partial \vec{r}}{\partial w}\right)\cdot \left(\frac{\partial \vec{r}}{\partial u}\right)\,dw\,du
        </me>
        Since, <m>\frac{\partial \vec{r}}{\partial u}</m>, <m>\frac{\partial \vec{r}}{\partial v}</m>, and 
        <m>\frac{\partial \vec{r}}{\partial w} </m> are the tangent vectors along the curves <m>u,v,w</m>, we have -
        <me>
          \left(\frac{\partial \vec{r}}{\partial u}\right)\cdot \left(\frac{\partial \vec{r}}{\partial v}\right)= \left(\frac{\partial \vec{r}}{\partial v}\right)\cdot \left(\frac{\partial \vec{r}}{\partial w}\right)= \left(\frac{\partial \vec{r}}{\partial w}\right)\cdot \left(\frac{\partial \vec{r}}{\partial u}\right)=0 
        </me>
       which are the conditions of orthogonality. 
        <me>
          \therefore \quad \,ds^{2}=\left(\frac{\partial \vec{r}}{\partial u}\right)^{2} \,du^{2}+ \left(\frac{\partial \vec{r}}{\partial v}\right)^{2} \,dv^{2}+\left(\frac{\partial \vec{r}}{\partial w}\right)^{2} \,dw^{2}.
        </me>
      </p>
    </solution>
  </example>

  <example>
    <statement>
      <p>
        A force is described by <m>\vec{F}=\frac{y}{x^{2}+y^{2}}\hat{i} +\frac{x}{x^{2}+y^{2}}\hat{j}</m>. 
        Find <m>\vec{F}</m> in a cylindrical coordinates.
      </p>
    </statement>
    <solution>
      <p>
        Use eqns. <xref first="eqn-unit_vect4" last="eqn-unit_vect6"/> 
        <me>
          \hat{i}= \cos\phi\hat{e_{\rho}}-\sin\phi\hat{e_{\phi}},  \quad 
          \hat{j}= \sin\phi\hat{e_{\rho}}+\cos\phi\hat{e_{\phi}},   \quad 
          \hat{k}=\hat{e_{z}}
        </me>
        to find 
        <me>
          \vec{F} =\frac{\hat{e_{\phi}}}{\rho}.
        </me>
      </p>
    </solution>
  </example>

  <example>
    <statement>
      <p>
        Show that <m>\vec{A}= -\phi\frac{\sin\theta}{r} \hat{e}_{\theta}</m> is a solution of 
        <m>\nabla \times \vec{A}=-\frac{1}{r^{2}}\hat{e}_{r}</m> in spherical coordinates.
      </p>
    </statement>
    <solution>
      <p>
        we have -
        <me>
          \nabla\times\vec{A}=\frac{1}{r^{2}\sin\theta}\begin{vmatrix} 
          \hat{e}_{r} &amp; r\hat{e}_{\theta} &amp; r\sin\theta\hat{e}_{\phi}\\ 
          \frac{\partial}{\partial r} &amp; \frac{\partial}{\partial \theta} &amp; \frac{\partial}{\partial \phi}\\ 
          0 &amp; -\frac{r\phi\sin\theta}{r} &amp; 0 \end{vmatrix}
        </me>
        <me>
          = \frac{1}{r^{2}\sin\theta}[\hat{e}_{r}(-\sin\theta)-0+0] = - \frac{1}{r^{2}}\hat{e}_{r}
        </me>
      </p>
    </solution>
  </example>

  <example>
    <statement>
      <p>
        Find the velocity and acceleration of a moving particle in a spherical coordinates.
      </p>
    </statement>
    <solution>
      <p>
      We have -
      <me>
        \vec{r}=r\hat{e}^{r}+\theta\hat{e}_{\theta}+\phi\hat{e}_{\phi}
      </me>
        Where,
        <me>
          \hat{e}_{r} = \frac{\frac{\partial \vec{r}}{\partial r}}{\mid\frac{\partial \vec{r}}{\partial r}\mid} 
          = \sin\theta\cos\phi\hat{i}+\sin\theta\sin\phi\hat{j}+\cos\theta\hat{k};
        </me>
        <me>
           \hat{e}_{\theta}  = \cos\theta\cos\phi\hat{i}+\cos\theta\sin\phi\hat{j}-\sin\theta\hat{k};
        </me>
        <me>
          \text{and}\quad \hat{e}_{\phi}=-\sin\phi\hat{i}+\cos\phi\hat{j}.
        </me>
        Now,
        <me>
          \frac{\partial \vec{r}}{\partial t}=\dot{r}\hat{e}_{r}+r\frac{\partial\hat{e}_{r}}{\partial t} 
          +\dot{\theta}\hat{e}_{\theta}+\theta\frac{\partial\hat{e}_{\theta}}{\partial t}
          +\dot{\phi}\hat{e}_{\phi}+\phi\frac{\partial\hat{e}_{\phi}}{\partial t} 
        </me>
        where,
        <me>
          \frac{\partial\hat{e}_{r}}{\partial t} = \dot{\theta}\phi\frac{\partial\hat{e}_{r}}{\partial\theta} 
          + \theta\dot{\phi}\frac{\partial\hat{e}_{r}}{\partial\phi};
        </me>
        <me>
          \frac{\partial\hat{e}_{r}}{\partial\theta} = \dot{\theta}\phi\hat{e}_{\theta};
        </me>
        <me>
           \text{and} \quad \frac{\partial\hat{e}_{r}}{\partial\phi} = \theta\sin\theta\dot{\phi}\hat{e}_{\phi}
        </me>
        Similarly, other components can be found to obtain the velocity and acceleration. 
      </p>
    </solution>
  </example>
</section>

