<?xml version="1.0" encoding="UTF-8"?>

<section xml:id="sec_fourth-examplesD" xmlns:xi="http://www.w3.org/2001/XInclude">
  <title>Examples D</title>
  <paragraphs>
  <title>Bessels's Function</title>
  <example>
    <statement>
      <p>
        Prove that <m> J_{-n}(x)=(-1)^{n}J_{n}(x)</m> where <m>n</m> is a positive integer.
      </p>
    </statement>
    <solution>
      <p>
        We have 
        <me>
          J_{-n}(x)=\sum\limits_{r=0}^{\infty}\frac{(-1)^{r}}{r!(-n+r)!}\left(\frac{x}{2}\right)^{-n+2r}
        </me>
        <me>
          =\sum\limits_{r=0}^{n-1}\frac{(-1)^{r}}{r!(-n+r)!}\left(\frac{x}{2}\right)^{-n+2r}+\sum\limits_{r=n}^{\infty}\frac{(-1)^{r}}{r!(-n+r)!}\left(\frac{x}{2}\right)^{-n+2r}
        </me>
        <me>
          =0+\sum\limits_{r=n}^{\infty}\frac{(-1)^{r}}{r!(-n+r)!}\left(\frac{x}{2}\right)^{-n+2r}
        </me>
          Since, <m>!(-ve \quad integer) = \infty</m>. Hence, for <m>r=0,1,2,\cdots</m>, we have  
          <me>
          \frac{1}{(-n+r)!}=0
          </me>
            putting <m>r=n+s</m>, where <m>s</m> is a positive integer, we have 
            <me>
              J_{-n}(x)=\sum\limits_{s=0}^{\infty}\frac{(-1)^{n+s}}{s!(n+s)!}\left(\frac{x}{2}\right)^{n+2s}
            </me>
            <me>
              =(-1)^{n}\sum\limits_{s=0}^{\infty}\frac{(-1)^{s}}{s!(n+s)!}\left(\frac{x}{2}\right)^{n+2s} =(-1)^{n}J_{n}(x) 
            </me>
      </p>
    </solution>
  </example>

  <example>
    <statement>
        Prove that 	
        <ol marker ="a.">
          <li>
            <p>
              <me>
                J_{\frac{1}{2}}(x)=\sqrt{\left(\frac{2}{\pi x}\right)}\sin x 
              </me>
            </p>
          </li>
          and 
          <li>
            <p>
              <me>
                J_{-\frac{1}{2}}(x)=\sqrt{\left(\frac{2}{\pi x}\right)}\cos x
              </me>
              
            </p>
          </li>
        </ol>
    </statement>
    <solution>
      <p>
        We know that
        <me>
          J_{-n}(x)=\sum\limits_{r=0}^{\infty}\frac{(-1)^{r}}{r!(n+r)!}\left(\frac{x}{2}\right)^{n+2r}	
        </me>
        <me>
          =	\frac{x^{n}}{2^{n}}	\left[\frac{1}{n!}-\frac{x^{2}}{2^{2}(n+1)!}+\frac{x^{4}}{2!(n+2)!2^{4}}-\cdots\right]
        </me>
        <men xml:id="eqn-bessl_eq1">
          = \frac{x^{n}}{2^{n}n!}\left[1-\frac{x^{2}}{2\cdot 2(n+1)}+\frac{x^{4}}{2\cdot 4\cdot 2^{2}(n+1)(n+2)}-\cdots\right]
        </men>
      </p>
       <ol marker ="a.">
          <li>
            <p>
              putting <m>n=\frac{1}{2}</m>  in eqn. <xref ref="eqn-bessl_eq1"/>, we get - 
              <me>
                J_{\frac{1}{2}}(x)=\frac{x^{\frac{1}{2}}}{2^{\frac{1}{2}}\frac{1}{2}!}\left[1-\frac{x^{2}}{2\cdot 2(\frac{1}{2}+1)}\right.
              </me>
              <me>
               \left. +\frac{x^{4}}{2\cdot 4\cdot 2^{2}(\frac{1}{2}+1)(\frac{1}{2}+2)}-\cdots\right]	
              </me>
              
              <me>
                =\frac{\sqrt{x}}{\sqrt{2}\Gamma{(\frac{1}{2}+1})}\left[1-\frac{x^{2}}{3!}+\frac{x^{4}}{5!}-\cdots\right]
              </me>
              <me>
                =\frac{\sqrt{x}}{\sqrt{2}\cdot\frac{1}{2}\Gamma{(\frac{1}{2})}}\cdot\frac{1}{x}\left[x-\frac{x^{3}}{3!}+\frac{x^{5}}{5!}-\cdots\right]
              </me>
              
                since, <m>\left[n!=\Gamma(n+1)=n\Gamma n\right]</m>,  the Gamma function	  
                <me>
                  \therefore J_{\frac{1}{2}}(x)=\frac{1}{\sqrt{2x}\cdot \frac{\sqrt{\pi}}{2}}\sin x=\sqrt{\left(\frac{2}{\pi x}\right)}\sin x 
                </me>
                <m> [\because \Gamma(\frac{1}{2})=\sqrt{\pi}</m> and <m>(\frac{1}{2})!=\frac{\sqrt{\pi}}{2}]	</m>.     
            </p>
          </li>
          <li>
            <p>
              Againg putting <m>n=-\frac{1}{2}</m> in equation <xref ref="eqn-bessl_eq1"/>, we get - 
              <me>
                J_{-\frac{1}{2}}(x)=\frac{x^{-\frac{1}{2}}}{2^{-\frac{1}{2}}\frac{1}{2}!}\left[1-\frac{x^{2}}{2\cdot 2(-\frac{1}{2}+1)}\right.
              </me>
              <me>
                \left.+\frac{x^{4}}{2\cdot 4\cdot 2^{2}(-\frac{1}{2}+1)(-\frac{1}{2}+2)}-\cdots\right]
              </me>
              
              <me>
                =\frac{\sqrt{2}}{\sqrt{x}\Gamma{(-\frac{1}{2}+1})}\left[1-\frac{x^{2}}{2!}+\frac{x^{4}}{2\cdot3\cdot4}-\cdots\right]
              </me>
              <me>
                =\frac{\sqrt{2}}{\sqrt{x}\Gamma{(\frac{1}{2})}}\left[1-\frac{x^{2}}{2!}+\frac{x^{4}}{4!}-\cdots\right]
              </me>
              
                <me>
                  =\sqrt{\left(\frac{2}{\pi x}\right)}\cos x 
                </me>
                [since <m>\Gamma(\frac{1}{2})=\sqrt{\pi}</m>].
            </p>
          </li>
        </ol>
    </solution>
  </example>

  <example>
    <statement>
      <p>
        Find the values of <m>J_{\pm\frac{3}{2}}(x)</m>.
      </p>
    </statement>
    <solution>
      <p>
        We have the recurrence relation (4) from <xref ref="subsubsec-bessl_recr"/>,
        <men xml:id="eqn-bessl_eq2">
          2nJ_{n}=x(J_{n-1}+J_{n+1}) 
        </men>
        putting <m>n=\frac{1}{2}</m>, we get -
        <me>
          J_{\frac{1}{2}}=x\left(J_{-\frac{1}{2}}+J_{\frac{3}{2}}\right)
        </me>
        or,
        <me>
          J_{\frac{3}{2}}=\frac{1}{x}\left(J_{\frac{1}{2}}\right)-J_{-\frac{1}{2}}
        </me>
        <men xml:id="eqn-bessl_eq3">
          =\frac{1}{x}\sqrt{\frac{2}{\pi x}}\sin x- \sqrt{\frac{2}{\pi x}}\cos x = \sqrt{\frac{2}{\pi x}}\left[\frac{\sin x}{x}-\cos x\right] 
        </men>
           Similarly on putting <m>n=-\frac{1}{2}</m> in eqn. <xref ref="eqn-bessl_eq2"/>, we get -
           <men xml:id="eqn-bessl_eq4">
            J_{-\frac{3}{2}}=\sqrt{\frac{2}{\pi x}}\left[\frac{-\cos x}{x}-\sin x\right] 
           </men>
           We can also prove it by putting <m>n=\pm\frac{3}{2}</m> in the eqn. 
           <xref ref="eqn-bessl_eq1"/> of previous problem 2.
      </p>
    </solution>
  </example>

  <example>
    <statement>
      <p>
        Prove that <m>J'_{2}(x)=(1-\frac{4}{x^{2}})J_{1}(x)+\frac{2}{x}J_{o}(x)</m>.
      </p>
    </statement>
    <solution>
      <p>
        By recurrnce relation 2 from <xref ref="subsubsec-bessl_recr"/>,
        <men xml:id="eqn-bessl_eq5">
          xJ'_{n}(x)=-nJ_{n}(x)+xJ_{n-1}(x)
        </men>
          putting <m>n=2</m> in eqn. <xref ref="eqn-bessl_eq5"/>, we have 
          <me>
            xJ'_{2}=-2J_{2}+xJ_{1}
          </me>
          or,
          <men xml:id="eqn-bessl_eq6">
            J'_{2}=-\frac{2}{x}J_{2}+J_{1} 
          </men>
          By recurrnce relation 4 from <xref ref="subsubsec-bessl_recr"/>,
          <me>
             2nJ_{n}=x(J_{n-1}+J_{n+1})
          </me>
              putting <m>n=1</m>, we have 
              <me>
                2\cdot1\cdot J_{1}=x(J_{o}+J_{2})
              </me>
              <men xml:id="eqn-bessl_eq7">
                J_{2}=\frac{2J_{1}}{x}-J_{o} 
              </men>
                  putting the value of <m>J_{2}</m> in eqn. <xref ref="eqn-bessl_eq6"/>, we get - 
                  <me>
                   J'_{2}=-\frac{2}{x}\left(\frac{2}{x}J_{1}-J_{o}\right)+J_{1}=-\frac{4}{x^{2}}J_{1}+\frac{2}{x}J_{o}+J_{1} 
                  </me>
                  <me>
                    = (1-\frac{4}{x^{2}})J_{1}(x)+\frac{2}{x}J_{o}(x)  
                  </me>   
      </p>
    </solution>
  </example>

  <example>
    <statement>
      <p>
        Using recurrence relations, show that <m>4J''_{n}(x)=J_{n-2}(x)-2J_{n}(x)+J_{n+2}(x)</m>.
      </p>
    </statement>
    <solution>
      <p>
        By the recurrnce relation 3 from <xref ref="subsubsec-bessl_recr"/>,
        <men xml:id="eqn-bessl_eq8">
          2J'_{n}=J_{n-1}-J_{n+1}
        </men>
        differentiating, we get-
       <men xml:id="eqn-bessl_eq9">
        2J''_{n}=J'_{n-1}-J'_{n+1}  
       </men>
          replacing <m>n</m> by <m>n-1</m>in eqn. <xref ref="eqn-bessl_eq8"/> and 
          <m>n</m> by <m>n+1</m> in eqn.  <xref ref="eqn-bessl_eq9"/>, we get -
          <me>
            2J'_{n-1}=J_{n-2}-J_{n}
          </me>
          or,
          <men xml:id="eqn-bessl_eq10">
            J'_{n-1}=\frac{1}{2}J_{n-2}-\frac{J_{n}}{2} 
          </men>
          and 
          <me>
            2J'_{n+1}=J_{n}-J_{n+2}
          </me>
          or,
          <men xml:id="eqn-bessl_eq11">
            J'_{n+1}=\frac{1}{2}J_{n}-\frac{1}{2}J_{n+2}
          </men>
            putting the values of <m>J'_{n-1} </m> and <m>J'_{n+1}</m> 
            in eqn. <xref ref="eqn-bessl_eq9"/>, we get - 
            <me>
              	2J''_{n}=\frac{1}{2}\left[J_{n-2}-J_{n}\right]-\frac{1}{2}\left[J_{n}-J_{n+2}\right]
            </me>
            or,
            <me>
              4J''_{n}=J_{n-2}-2J_{n}+J_{n+2}.
            </me>
      </p>
    </solution>
  </example>

  <example>
    <statement>
      <p>
        Prove that <m>J''_{1}=\left(\frac{2}{x^{2}}-1\right)J_{1}-\frac{1}{x}J_{o}</m>.
      </p>
    </statement>
    <solution>
      <p>
        By recurrence relation 2 from <xref ref="subsubsec-bessl_recr"/>,
        <men xml:id="eqn-bessl_eq12">
          xJ'_{n}=-nJ_{n}+xJ_{n-1}
        </men>
        Differentiating, we get -
        <me>
          xJ''_{n}+J'_{n}=-nJ'_{n}+xJ'_{n-1}+J_{n-1}
        </me>
          Putting, <m>n=1</m>,
          <me>
            xJ''_{1}+J'_{1}=-J'_{1}+xJ'_{o}+J_{o}	
          </me>
          or,
           <men xml:id="eqn-bessl_eq13">
            J''_{1}=-\frac{2}{x}J'_{1}+J'_{o}+\frac{1}{x}J_{o} 
           </men>
           By recurrence relation 1,
           <me>
            xJ'_{n}=nJ_{n}-xJ_{n+1}
           </me>
            putting <m>n=0</m>
            <me>
              xJ'_{o}=-xJ_{1}
            </me>
            or,
            <me>
               J'_{o}=-J_{1}
            </me>
            putting the value of <m>J'_{o} </m> in eqn. <xref ref="eqn-bessl_eq13"/>, we get -
            <me>
              J''_{1}=-\frac{2}{x}J'_{1}-J_{1}+\frac{1}{x}J_{o}
            </me>
                putting <m>n=1</m>, in eqn. <xref ref="eqn-bessl_eq12"/>, we get -
                <me>
                   xJ'_{1}=-J_{1}+xJ_{o}
                </me>
                or,
                <men xml:id="eqn-bessl_eq14">
                J'_{1}=-\frac{1}{x}J_{1}+J_{o} 
                </men>
                  putting <m>J'_{1}</m> in eqn. <xref ref="eqn-bessl_eq14"/>, we have
                  <me>
                    J''_{1}=-\frac{2}{x}\left(-\frac{J_{1}}{x}+J_{o}\right)-J_{1}+\frac{1}{x}J_{o} =\frac{2}{x^{2}}J_{1}-J_{1}+\frac{J_{o}}{x}(1-2)
                  </me>
                  <me>
                    =\left(\frac{2}{x^{2}}-1\right)J_{1}-\frac{J_{o}}{x} 
                  </me> 
      </p>
    </solution>
  </example>

  <example>
    <statement>
      <p>
        Prove that 	<m>\frac{\,d}{\,dx}\left[x^{n}J_{n}(x)\right]=x^{n}J_{n-1}(x)</m>.
      </p>
    </statement>
    <solution>
      <p>
        <me>
          x^{n}J_{n}(x)=x^{n}\sum\limits_{r=0}^{\infty}\frac{(-1)^{r}}{r!(n+r)!}\left(\frac{x}{2}\right)^{n+2r}
        </me>
        <me>
          =\sum\limits_{r=0}^{\infty}\frac{(-1)^{r}x^{2n+2r}}{r!(n+r)!\cdot 2^{n+2r}}
        </me>
        <me>
          \therefore \frac{d}{dx}\left[x^{n}J_{n}(x)\right]=\sum\limits_{r=0}^{\infty}\frac{(-1)^{r}(2n+2r)x^{2n+2r-1}}{r!(n+r)!\cdot 2^{n+2r}}
        </me>
        <me>
          =x^{n}\sum\limits_{r=0}^{\infty}\frac{(-1)^{r}(n+r)x^{n+2r-1}}{r!(n+r)!(n+r-1)\cdot 2^{n+2r-1}}
        </me>
        <me>
          =x^{n}\sum\limits_{r=0}^{\infty}\frac{(-1)^{r}}{r!(n-1+r)!}\left(\frac{x}{2}\right)^{\overline{n-1}+2r} 
        </me>
        <me>
          = x^{n}J_{n-1}(x)
        </me>
      </p>
    </solution>
  </example>

  <example>
    <statement>
      <p>
        Prove that 
        <me>
          x\sin x=2\left[2^{2}J_{2}-4^{2}J_{4} +6^{2}J_{6}-\cdots\right] 
        </me>
        and 
        <me>
          x\cos x=2\left[1^{2}J_{1}-3^{2}J_{3} +5^{2}J_{5}-\cdots\right]
        </me>
      </p>
    </statement>
    <solution>
      <p>
        We know that -
        <men xml:id="eqn-bessl_eq15">
          \cos(x\sin\theta)=J_{o}+2J_{2}\cos2\theta+2J_{4}\cos4\theta+\cdots 
        </men>
        and 
        <men xml:id="eqn-bessl_eq16">
           \sin(x\sin\theta)=2J_{1}\sin\theta+2J_{3}\sin3\theta+2J_{5}\sin5\theta+\cdots 
        </men>
          Differentiating eqn. <xref ref="eqn-bessl_eq15"/> w. r. t. <m>\theta</m>, we get -
          <men xml:id="eqn-bessl_eq17">
            [-\sin(x\sin\theta)]x\cos\theta=0-4J_{2}\sin2\theta-8J_{4}\sin4\theta+\cdots 
          </men>
        again, differentiating eqn. <xref ref="eqn-bessl_eq17"/> w. r. t. <m>'\theta'</m>, we get -
        <me>
            [-\sin(x\sin\theta)](-x\sin\theta)+[-\cos(x\sin\theta)](x\cos\theta)(x\cos\theta)
        </me>
<men xml:id="eqn-bessl_eq18">
=-8J_{2}\cos2\theta-32J_{4}\cos4\theta+\cdots  
</men>
putting <m>\theta=\frac{\pi}{2}</m>  in eqn. <xref ref="eqn-bessl_eq18"/>, we get -
<me>
  x\sin x=8J_{2}-32J_{4}+\cdots =2[2^{2}J_{2}-4^{2}J_{4}+\cdots]
</me>
similarly, differentiating eqn. <xref ref="eqn-bessl_eq16"/> twice and putting 
<m>\theta=\frac{\pi}{2}</m>, we get -
<me>
  x\cos x=2[1^{2}J_{1}-3^{2}J_{3}+\cdots]
</me>
      </p>
    </solution>
  </example>
 </paragraphs>


    
</section>
