<?xml version="1.0" encoding="UTF-8"?>

<section xml:id="sec_fourth-lagurfn" xmlns:xi="http://www.w3.org/2001/XInclude">
  <title>Laguerre Differential Equation</title>
  <introduction>

    <figure xml:id="fig-fig46">
    <caption>hermite's Polynomial</caption>
    <image source="fig46.png" width ="45%"/>
</figure>

  <p>
    <idx><h>Laguerre's Differential Equation</h></idx>
    The differential equation  
    <men xml:id="eqn-laguer_eq1">
      x\frac{d^{2}y}{dx^{2}}+(1-x)\frac{dy}{dx}+\lambda y=0
    </men>
        where <m>\lambda</m> is constant, is known as Laguerre's differential equation. 
        Such type of equation yields on solving Shrodinger's equation for Hydrogen atom. 
        It has regular singularities at <m>x=0</m>. Let us assume the series solution of 
        such equation is 
        <men xml:id="eqn-laguer_eq2">
          y=\sum\limits_{k=0}^{\infty}a_{k}x^{m+k}
        </men>
        so that 
        <me>
          \frac{dy}{dx}=\sum\limits_{k=0}^{\infty}a_{k}(m+k)x^{m+k-1} 
        </me>
        and 
        <me>
           \frac{d^{2}y}{dx^{2}}=\sum a_{k}(m+k)(m+k-1)x^{m+k-2}
        </me>
          Substituting these values in equation <xref ref="eqn-laguer_eq1"/>, we have
          <me>
            \sum a_{k}(m+k)(m+k-1)x^{m+k-1}+\sum a_{k}(m+k)x^{m+k-1} 
          </me>
          <me>
            -\sum a_{k}(m+k)x^{m+k}+\sum a_{k}\lambda x^{m+k}=0
          </me>
          
          or,
          <me>
            \sum a_{k}[(m+k)(m+k-1)+(m+k)]x^{m+k-1}
          </me>
          <me>
            -\sum a_{k}[m+k-\lambda]x^{m+k}=0
          </me>
          
          or,
          <men xml:id="eqn-laguer_eq3">
            \sum a_{k}[(m+k)^{2}x^{m+k-1}-\sum a_{k}(m+k-\lambda)x^{m+k}=0
          </men>
            Equating the coefficient of lowest power of <m>x</m> i.e., <m>x^{m-1}</m> to zero, 
            we get the indicial equation as <m>a_{o}m^{2}=0</m>	[<m>\because k=0</m>]
            Since <m>a_{o} \neq 0 </m>, therefore <m>m=0</m>. Again, equating the coefficient 
            of <m>x^{m+k}</m>, the general term, to zero, we get the recurrence relations 
            among the coefficients as -
            <me>
              a_{k+1}(m+k+1)^{2}-a_{k}(m+k-\lambda)=0
            </me>
            or,
            <men xml:id="eqn-laguer_eq4">
              a_{k+1}=\frac{m+k-\lambda}{(m+k+1)^{2}}a_{k}
            </men>
            for <m>m=0</m>, we have 
            <men xml:id="eqn-laguer_eq5">
              a_{k+1}=\frac{k-\lambda}{(k+1)^{2}}a_{k}
            </men>
            Thus,
            <me>
              a_{1} =-\frac{\lambda}{1^{2}}a_{o}=(-1)\lambda a_{o}  
            </me>
             [set <m>k=0</m>]
              <me>
                a_{2}=\frac{1-\lambda}{2^{2}}a_{1}=\frac{\lambda-1}{2^{2}}\lambda a_{o} =\frac{\lambda(\lambda-1)}{2^{2}} a_{o}=(-1)^{2}\frac{\lambda(\lambda-1)}{(2!)^{2}} a_{o}
              </me>
              <me>
                a_{3}=\frac{2-\lambda}{3^{2}}a_{2}=\frac{(-1)(\lambda-2)}{3^{2}}\cdot \frac{(-1)^{2}\lambda(\lambda-1)}{(2!)^{2}}a_{o} 
              </me>
              <me>
                =(-1)^{3}\frac{\lambda(\lambda-1)(\lambda-2)}{(3!)^{2}}a_{o}
              </me>
              
              <me>
                a_{r}=(-1)^{r}\frac{\lambda(\lambda-1)(\lambda-2)\cdots(\lambda-r+1)}{(r!)^{2}}a_{o}
              </me>
                so, 
                <me>
                  y=\sum\limits_{k=0}^{\infty}a_{k}x^{k} =a_{o}\left[1-\lambda x+\frac{\lambda(\lambda-1)}{(2!)^{2}}x^{2}-\cdots\right.
                </me>
                <me>
                  	\left.\cdots+(-1)^{r}\frac{\lambda(\lambda-1)(\lambda-2)\cdots(\lambda-r+1)}{(r!)^{2}}x^{r}+\cdots\right]
                </me>
                <men xml:id="eqn-laguer_eq6">
                  =a_{o}\sum\limits_{r=0}^{\infty}\frac{(-1)^{r}\lambda !}{(r!)^{2}(\lambda-r)!}x^{r}
                </men>
                If <m>\lambda =n</m> is a positive integer then 
                <men xml:id="eqn-laguer_eq7">
                 	y= a_{o}\sum\limits_{r=0}^{n+1}\frac{(-1)^{r} n!}{(r!)^{2}(n-r)!}x^{r} 
                </men>
                  If we choose <m>a_{o}=n!</m>, then the solution for <m>y</m> becomes 
                  the Laguerre's Polynomial, <m>L_{n}(x)</m>.
                    Thus,
                  <men xml:id="eqn-laguer_eq8">
                    L_{n}(x) = \sum\limits_{r=0}^{n+1}\frac{(-1)^{r} (n!)^{2}}{(r!)^{2}(n-r)!}x^{r}
                  </men>
                  The family of Laguerre's Polynomial is 
                  <me>
                    L_{n}(0)=n!; \quad L_{o}(x) =1;  \quad L_{1}(x) =1-x; 
                  </me>
                  <me>
                    L_{2}(x)  =x^{2}-4x+2^{2}; L_{3}(x) =-x^{3}+9x^{2}-36x+6;
                  </me>
                  
                  <me>
                 L_{4}(x) =x^{4}-16x^{3}+72x^{2}-96x+48;
                  </me>
                  and so on. Thus Laguerre's polynomial is the solution of equation.
                  <me>
                    xL''_{n}(x)+(1-x)L'_{n}(x)+nL_{n}(x)=0
                  </me>
                  The graph of Laguerre's polynomial is shown in figure <xref ref="fig-fig46"/>	
    </p>
     </introduction>
 
 <subsection xml:id="subsec-laguer_pol">
  <title>Laguerre's Polynomial</title>
  <introduction>
   
  <paragraphs>
    <title>Python Code:</title>
    <p> import numpy as np </p>
 <p>from scipy.special import genlaguerre </p>
<p> from scipy.special import laguerre </p>
<p> import matplotlib.pyplot as plt </p>
  <p>    x = np.arange(-1.0, 5.0, 0.01) </p>
<p> fig, ax = plt.subplots() </p>
<p> ax.set_ylim(-5.0, 5.0) </p>
<p> ax.set_title(r'Laguerre polynomials $L_n$') </p>
<p> for n in np.arange(0, 5): </p>
  <p>  ax.plot(x, laguerre(n)(x), label=rf'$L_{n}(x)$') </p>
<p> plt.legend(loc='best') </p>
<p> plt.xlabel("x") </p>
<p> plt.ylabel(r'$L_n(x)$') </p>
<p> plt.legend(loc='lower right') </p>
<p> plt.show() </p>
 
  </paragraphs>
 
  </introduction>


  <subsubsection xml:id="subsubsec-laguer_genfn">
    <title>Generating Function for <m>L_{n}(x)</m></title>
    <p>
      <idx><h>generating function for Laguerre's polynomial</h></idx> 
      The generating function for Laguerre's polynomial is defined as 
      <me>
      f(x,t)=\frac{e^{-xt/(1-t)}}{1-t}=\sum\limits_{n=0}^{\infty}\frac{L_{n}(x)}{n!}t^{n}\quad |t| \lt 1.
      </me>
      
      </p>
      <proof>
        <p>
        We have 
        <me>
           e^{-xt/(1-t)}=1-\frac{xt}{1-t}+\frac{1}{2!}\left(\frac{xt}{1-t}\right)^{2}+\cdots
        </me>
        
        <men xml:id="eqn-laguer_gen1">
         =\sum\limits_{r=0}^{\infty}\frac{(-1)^{r}x^{r}t^{r}}{(1-t)^{r}r!}
        </men>
        or,
        <me>
          \frac{e^{-xt/(1-t)}}{1-t}=\sum\limits_{r=0}^{\infty}(-1)^{r}\frac{t^{r}x^{r}}{r!(1-t)^{r+1}}
        </me>
        <me>
          =\sum\limits_{r=0}^{\infty}(-1)^{r}\frac{x^{r}t^{r}}{r!}(1-t)^{-(r+1)}
        </me>
        
        <me>
          =\sum\limits_{r=0}^{\infty}\frac{(-1)^{r}}{r!}x^{r}t^{r}\left[1+(r+1)t+\frac{(r+1)(r+2)}{2!}t^{2}\right.
        </me>
        <me>
          \left.+\cdots+\frac{(r+1)(r+2)\cdots(r+s)}{s!}t^{s}+\cdots\right]
        </me>
        
        <me>
           =\sum\limits_{r=0}^{\infty}\frac{(-1)^{r}x^{r}t^{r}}{r!}\sum\limits_{s=0}^{\infty}\frac{(r+1)(r+2)\cdots(r+s)}{s!}t^{s}
        </me>
        
        <men xml:id="eqn-laguer_gen2">
         =\sum\limits_{r=0}^{\infty}\frac{(-1)^{r}x^{r}t^{r}}{r!}\sum\limits_{s=0}^{\infty}\frac{(r+s)!}{r!s!}t^{s}
        </men>
          on putting <m>r+s=n</m>, the coefficient of <m>t^{n}</m> for fixed value of 
          <m>r</m>  is <m>\frac{(-1)^{r}n!}{(r!)^{2}(n-r)!}x^{r}</m>,  as <m>n-r=s</m>  and  
          <m>s \geq 0</m>. 	Thus <m> n-r \geq 0</m>	or, <m>r \leq n</m>. Hence the coefficient 
          of <m>t^{n}</m> on RHS of equation <xref ref="eqn-laguer_gen2"/> is 
          <me>
            \sum\limits_{r=0}^{n}\frac{(-1)^{r}n!}{(r!)^{2}(n-r)!}x^{r} =\frac{L_{n}(x)}{n!}
          </me>
          Therefore,
          <me>
             \frac{e^{-xt/(1-t)}}{1-t}=\sum\limits_{r=0}^{n}\frac{L_{n}(x)}{n!}t^{n}
          </me>
          is the generating function of <m>L_{n}(x)</m>.		
	 </p>
      </proof>
  </subsubsection>

<subsubsection xml:id="subsubsec-laguer_rodr">
  <title>Rodrigue's Differential Formula for <m>L_{n}(x)</m></title>
  <p>
    <me>
      L_{n}(x)=e^{x}\frac{d^{n}}{dx^{n}}(x^{n}e^{-x}).
    </me>
    </p>
    <proof>
      <p>
        We have the generating function for <m>L_{n}(x)</m> is 
        <me>
          \frac{e^{-xt/(1-t)}}{1-t}=\sum\limits_{n=0}^{\infty}\frac{L_{n}(x)}{n!}t^{n}
        </me>
        Differentiating <m>n</m> times w. r. to 't', we get - 
        <me>
          \frac{d^{n}}{dt^{n}}\left(\frac{e^{-xt/(1-t)}}{1-t}\right)=	L_{n}(x)+L_{n+1}(x)t+\cdots
        </me>
        or,
        <me>
            e^{x}\frac{d^{n}}{dt^{n}}\left[(1-t)^{-1}e^{-x/(1-t)}\right] 
        </me>
        
        <men xml:id="eqn-laguer_rodr1">
        =L_{n}(x)+L_{n+1}(x)t+\cdots	
        </men>
        But,
        <me>
          \frac{d}{dt}\left[(1-t)^{-1}e^{-x/(1-t)}\right]=\frac{1-x-t}{(1-t)^{3}}e^{-x/(1-t)}
        </me>
        or,
        <me>
          \lim\limits_{t \to 0}\frac{d}{dt}\left[(1-t)^{-1}e^{-x/(1-t)}\right]=(1-x)e^{-x}=\frac{d}{dx}(xe^{-x})
        </me>
        similarly,
        <me>
           \lim\limits_{t \to 0}\frac{d^{2}}{dt^{2}}\left[(1-t)^{-1}e^{-x/(1-t)}\right]=\frac{d^{2}}{dx^{2}}(x^{2}e^{-x})
        </me>
        In general,
        <me>
          \lim\limits_{t \to 0}\frac{d^{n}}{dt^{n}}\left[(1-t)^{-1}e^{-x/(1-t)}\right]=\frac{d^{n}}{dx^{n}}(x^{n}e^{-x})
        </me>
        Hence from equation <xref ref="eqn-laguer_rodr1"/>, we have 
        <me>
          e^{x}\lim\limits_{t \to 0}\frac{d^{n}}{dt^{n}}\left[(1-t)^{-1}e^{-x/(1-t)}\right]=e^{x}\frac{d^{n}}{dx^{n}}(x^{n}e^{-x})=L_{n}(x).
        </me>
        Thus, 
        <me>
          L_{n}(x)= e^{x}\frac{d^{n}}{dx^{n}}(x^{n}e^{-x})
        </me>
        This is the Rodrigue's formula for <m>L_{n}(x)</m>.				
      </p>
    </proof>
</subsubsection>

<subsubsection xml:id="subsubsec-laguer_recr">
  <title>Recurrence Relation for <m>L_{n}(x)</m></title>
  <ol>
    <li>
      <p>
        <me>
          (1+2n-x)L_{n}=n^{2}L_{n-1}+L_{n+1}
        </me>
      </p>
      <proof>
        <p>
          We have the generating function 
          <men xml:id="eqn-laguer_recr1">
            \frac{e^{-xt/(1-t)}}{1-t}=\sum\limits_{n=0}^{\infty}\frac{L_{n}(x)}{n!}t^{n} \qquad |t| \lt 1.
          </men>
        
          Differentiating equation <xref ref="eqn-laguer_recr1"/> w. r. to 't', we get -
          <me>
            \frac{1-x-t}{(1-t)^{3}}e^{-xt/(1-t)}=\sum\limits_{n=0}^{\infty}\frac{L_{n}(x)}{(n-1)!}t^{n-1}
          </me>
          or,
          <me>
           (1-x-t)\sum\limits_{n=0}^{\infty}\frac{L_{n}(x)}{(n)!}t^{n}=(1-t)^{2}\sum\limits_{n=0}^{\infty}\frac{L_{n}(x)}{(n-1)!}t^{n-1}
          </me>
          or,
          <me>
            (1-x)\sum\limits_{n=0}^{\infty}\frac{L_{n}(x)}{(n)!}t^{n}-\sum\limits_{n=0}^{\infty}\frac{L_{n}(x)}{(n)!}t^{n+1}	
          </me>
          <me>
            =\sum\limits_{n=0}^{\infty}\frac{L_{n}(x)}{(n-1)!}t^{n-1}-2\sum\limits_{n=0}^{\infty}\frac{L_{n}(x)}{(n-1)!}t^{n}+\sum\limits_{n=0}^{\infty}\frac{L_{n}(x)}{(n-1)!}t^{n+1}
          </me>
          Equating the coefficient of <m>t^{n}</m> on both sides, we get -
          <me>
            (1-x)\frac{L_{n}}{(n)!}-\frac{L_{n-1}}{(n-1)!}=\frac{L_{n+1}}{(n)!}-2\frac{L_{n}}{(n-1)!}+\frac{L_{n-1}}{(n-2)!}
          </me>
          or,
       <me>
  (1-x) L_{n}-nL_{n-1}=L_{n+1}-2nL_{n}+n(n-1)L_{n-1} 
</me>
 [on multiplying by <m> n!</m>] Or,
 <me>
  \therefore (1+2n-x)L_{n}=n^{2}L_{n-1}+L_{n+1}
 </me>
        </p>
      </proof>
    </li>
    <li>
      <p>
        <me>
          L'_{n}=n[L'_{n-1}-L_{n+1}
        </me>
      </p>
      <proof>
        <p>
          Differentiating above equation <xref ref="eqn-laguer_recr1"/> w. r. to 'x', we get - 
          <me>
            -(1-t)^{-1}\frac{1}{(1-t)}e^{-xt/(1-t)}=\sum\limits_{n=0}^{\infty}\frac{L'_{n}}{(n)!}t^{n}
          </me>
          or,
          <me>
            -t\sum\limits_{n=0}^{\infty}\frac{L_{n}}{(n)!}t^{n}=(1-t)\sum\limits_{n=0}^{\infty}\frac{L'_{n}}{(n)!}t^{n}
          </me>
          or,
          <me>
            -\sum\limits_{n=0}^{\infty}\frac{L_{n}}{(n)!}t^{n+1}=\sum\limits_{n=0}^{\infty}\frac{L'_{n}}{(n)!}t^{n}-\sum\limits_{n=0}^{\infty}\frac{L'_{n}}{(n)!}t^{n+1}
          </me>
          Equating the coefficient of <m>t^{n}</m> on both sides, we get - 
          <me>
            -\frac{L_{n+1}}{(n-1)!}=\frac{L'_{n}}{n!}-\frac{L'_{n-1}}{(n-1)!}
          </me>
          <me>
            L'_{n}=nL'_{n-1}-nL_{n-1}
          </me>
          or,
          <me>
            \therefore L'_{n}=n[L'_{n-1}-L_{n-1}] 
          </me>
        </p>
      </proof>
    </li>
    <li>
      <p>
        <me>
          xL'_{n}=n[L_{n}-n^{2}L_{n-1}
        </me>
      </p>
      <proof>
        <p>
          Differentiating the recurrence relation (1) w. r. to 'x', we get -
          <men xml:id="eqn-laguer_recr2">
            (1+2n-x)L'_{n}-L_{n}=n^{2}L'_{n-1}+L'_{n+1}
          </men>
            Replacing <m>n</m> by <m>n+1</m> in relation (2), we get -
            <me>
              L'_{n+1}=(n+1)[L'_{n}-L_{n}]
            </me>
            or,
            <men xml:id="eqn-laguer_recr3">
              L'_{n+1}=(n+1)L'_{n}-(n+1)L_{n}]
            </men>
            Also, from relation (2), we have 
            <men xml:id="eqn-laguer_recr4">
              L'_{n-1}=L_{n-1}+\frac{1}{n}L'_{n}
            </men>
              Substituting equations <xref ref="eqn-laguer_recr3"/> and <xref ref="eqn-laguer_recr4"/> 
              in equation <xref ref="eqn-laguer_recr2"/>, we get -
              <me>
                 (1+2n-x)L'_{n}-L_{n}=n^{2}[L_{n-1}+\frac{1}{n}L'_{n}]
              </me>
              <me>
                \qquad +(n+1)L'_{n}-(n+1)L_{n}
              </me>
              
              or,
              <me>
                 (1+2n-x)L'_{n}-L_{n}=n^{2}L_{n-1}+nL'_{n}+nL'_{n}+L'_{n}-nL_{n}-L_{n}
              </me>
              or,
              <me>
                (1+2n)L'_{n}-xL'_{n}=n^{2}L_{n-1}+(1+2n)L'_{n}-nL_{n}
              </me>
                or,
                <me>
                   -xL'_{n}=n^{2}L_{n-1}-nL_{n}
                </me>
                or,
                <me>
                  \therefore xL'_{n}=nL_{n}-n^{2}L_{n-1} 
                </me>
        </p>
      </proof>
    </li>
  </ol>
</subsubsection>

<subsubsection xml:id="subsubsec-laguer-orth">
  <title>Orthogonal Property of Laguerre Polynomials</title>
  <p>
    <me>
      \int\limits_{0}^{\infty}e^{-x}\frac{L_{m}(x)}{m!}\frac{L_{n}(x)}{n!}\,dx = \delta_{m,n} 
      =\begin{cases}
	0, &amp; \text{if}\quad m \neq n\\
	1, &amp; \text{if}\quad m = n
	\end{cases}
    </me>
    </p>
    <proof>
      <p>
        We have 
        <me>
          \sum\limits_{m=0}^{\infty}\frac{L_{m}(x)}{m!}s^{m}=\frac{1}{1-s}e^{-xs/(1-s)}
        </me>
        and 
        <me>
          \sum\limits_{n=0}^{\infty}\frac{L_{n}(x)}{n!}t^{n}=\frac{1}{1-t}e^{-xt/(1-t)}
        </me>
        <me>
          \therefore \sum\limits_{m,n=0}^{\infty}e^{-x}\frac{L_{m}(x)}{m!}s^{m}\frac{L_{n}(x)}{n!}t^{m}s^{m}t^{n}
        </me>
        <me>
          =e^{-x}\frac{1}{(1-s)(1-t)}e^{\frac{-xs}{1-s}}e^{\frac{-xt}{1-t}}
        </me>
        
        thus,
        <me>
          \int\limits_{0}^{\infty}e^{-x}\frac{L_{m}(x)}{m!}\frac{L_{n}(x)}{n!}\,dx =  \text{coefficient of}\quad  s^{m}t^{n}\quad \text{in}
        </me>
        
        <me>
          \int\limits_{0}^{\infty}e^{-x}\frac{1}{(1-s)(1-t)}e^{\frac{-xs}{1-s}}e^{\frac{-xt}{1-t}}\,dx.
        </me>
        Now,
        <me>
          \int\limits_{0}^{\infty}e^{-x}\frac{1}{(1-s)(1-t)}e^{\frac{-xs}{1-s}}e^{\frac{-xt}{1-t}}\,dx  
        </me>
        <me>
          =\frac{1}{(1-s)(1-t)}\int\limits_{0}^{\infty}e^{-x\left[1+\frac{t}{1-t}+\frac{s}{1-s}\right]}\,dx
        </me>
        
        <me>
          =\frac{1}{(1-s)(1-t)}\frac{1}{[1+\frac{s}{1-s}+\frac{t}{1-t}}\left[e^{-x}\{[1+\frac{s}{1-s}+\frac{t}{1-t}\}\right]_{0}^{\infty}
        </me>
        <me>
          =\frac{1}{(1-s)(1-t)}\frac{(1-s)(1-t)}{(1-s)(1-t)+s(1-t)+t(1-s)}[0-1]
        </me>
        <me>
          =\frac{1}{1-st}=(1-st)^{-1}=1+st+(st)^{2}+\cdots+(st)^{n}+\cdots
        </me>
        in which coefficient of <m>s^{m}t^{n}</m> is <m>0</m> if <m>m \neq n</m>  and <m>1</m> 
         if <m>m=n</m>. Hence,	
         <me>
          \int\limits_{0}^{\infty}e^{-x}\frac{L_{m}(x)}{m!}\frac{L_{n}(x)}{n!}\,dx = \delta_{m,n} 
          =\begin{cases} 
          	0, &amp; \text{if}\quad m \neq n\\ 
            	1, &amp; \text{if}\quad m = n 
              	\end{cases}
         </me>
      </p>
    </proof>
</subsubsection>
 </subsection>


  </section>

