<?xml version="1.0" encoding="UTF-8"?>

<section xml:id="sec_first-examplesB" xmlns:xi="http://www.w3.org/2001/XInclude">
  <title>Examples B</title>

  <paragraphs>
    <title>Vector Integration</title>
   <example>
    <statement>
      <p>
        Find the total work done by a force  <m>\vec{F}=2x^{2}y\hat{i}+3xy\hat{j}</m> 
        if it displaces a particle from (0,0) to (1,4) along a curve <m>y=4x^{2}</m>. 
      </p>
    </statement>
    <solution>
      <p>
        Along the given curve, 
        <me>
          \vec{F}=2x^{2}.4x^{2}\hat{i}+3x.4x^{2}\hat{j}=8x^{4}\hat{i}+12x^{3}\hat{j} 
        </me>
             as <m>y=4x^{2}</m>, and 
             <me>
              \vec{r}=x\hat{i}+y\hat{j}= x\hat{i}+4x^{2}\hat{j}
             </me>
             or,
             <me>
              \vec{\,dr} = \,dx\hat{i}+8x\,dx\hat{j}
             </me>
              
             <me>
              \therefore \text{Work done} \quad \int_{c}\vec{F}\cdot\vec{\,dr} = \int^{1}_{0} (8x^{4}\hat{i}+ 12x^{3}\hat{j}) \cdot (dx\hat{i}+8x\,dx\hat{j})
             </me>
             <me>
              =\int^{1}_{0} (8x^{4}dx+ 96x^{4}dx)=\int^{1}_{0} 104x^{4}\,dx 
             </me>
             <me>
              = 104\int^{1}_{0}x^{4}\,dx = 104\left[x^{5}/5\right]^{1}_{0}=104/5.
             </me>
      </p>
    </solution>
   </example>

   <example>
    <statement>
      <p>
        Find <m>\int_{c}\vec{F}\cdot\vec{\,dr}</m>, if a particle is traversing counter clockwise 
        on the curve <m>c</m> due to the influence of force 
        <me>
          \vec{F}=\frac{\hat{i}y-\hat{j}x}{x^{2}+y^{2}}.
        </me>
        Here <m>c</m> is a circle <m>x^{2}+y^{2}=1</m> <image source="fig18.png" width ="25%"/>. 
      </p>
    </statement>
    <solution>
      <p>
        Suppose 
        <m>\vec{r}=x\hat{i}+y\hat{j}+z\hat{k}</m> and <m>\vec{\,dr}=\,dx\hat{i}+\,dy\hat{j}+\,dz\hat{k}</m>. Then,
        <me>
          \int_{c}\vec{F}\cdot\vec{\,dr}
          =\int_{c}\left(\frac{\hat{i}y-\hat{j}x}{x^{2}+y^{2}}\right)\cdot (\,dx\hat{i}+\,dy\hat{j}+\,dz\hat{k}) 
        </me>
        <me>
          =\int_{c}\left(\frac{y\,dx-x\,dy}{x^{2}+y^{2}}\right) = \int_{c}\left({y\,dx-x\,dy}\right)
        </me>
        Parametric equations of the circle are 
        <md>
          <mrow> x\amp = 1 \cos\theta</mrow>
          <mrow> y\amp =1 \sin\theta</mrow>
        </md>
         from the given figure.
      
        <me>
          \therefore   \,dx= -\sin\theta \,d\theta, \,dy=\cos\theta \,d\theta
        </me>
         and 
         <me>
          \int\limits_{c}\vec{F}\cdot\vec{dr} 
          =\int\limits_{0}^{2\pi} \left[\sin\theta(-\sin\theta \,d\theta)-\cos\theta (\cos\theta \,d\theta)\right]  
         </me>
         <me>
          =-\int\limits_{0}^{2\pi}( \sin^{2}\theta+\cos^{2}\theta)\,d\theta 
          =-\int\limits_{0}^{2\pi} \,d\theta=-\left(\theta\right)_{0}^{2\pi}=-2\pi.
         </me>
         </p>
    </solution>
   </example>

<example>
  <statement>
    <p>
      Show that the flux, <m>\iint\limits_{S}\vec{F}\cdot \hat{n}ds= \frac{3}{2}</m>, 
      where <m>\vec{F}=4xz\hat{i}-y^{2}\hat{j}+yz\hat{k}</m> and  <m>S</m>  is the surface of the 
      cube bounded by the planes  <m>x=0</m>, <m>x=1</m>, <m>y=0</m>, <m>y=1</m>, and <m>z=0</m>, 
      <m>z=1</m> as shown in figure <image source="fig19.png" width ="35%"/>
    </p>
  </statement>
  <solution>
    <p>
      <me>
        \iint\limits_{S}\vec{F}\cdot \hat{n}\,ds= \iint\limits_{OABC}\vec{F}\cdot \hat{n}\,ds+\iint\limits_{DEFG}\vec{F}\cdot \hat{n}\,ds
      </me>
      <me>
        \quad +\iint\limits_{OAFG}\vec{F}\cdot \hat{n}\,ds +\iint\limits_{BCDE}\vec{F}\cdot \hat{n}\,ds 
      </me>
      <men xml:id="eqn-vectint3">
        \qquad +\iint\limits_{ABEF}\vec{F}\cdot \hat{n}\,ds+\iint\limits_{OCDG}\vec{F}\cdot \hat{n}\,ds 
      </men>
      <me>
        Now,\quad \iint\limits_{OABC}\vec{F}\cdot \hat{n}\,ds= \iint\limits_{OABC}(4xz\hat{i}-y^{2}\hat{j}+yz\hat{k})\cdot (-\hat{k})\,dx\,dy
      </me>
      <me>
       \quad  =-\int\limits_{0}^{1}\int\limits_{0}^{1}yz\,dx\,dy=0.\quad [\because z=0 \quad\text{for face OABC}]
      </me>
      <me>
        \iint\limits_{DEFG}\vec{F}\cdot \hat{n}\,ds= \iint\limits_{DEFG}(4xz\hat{i}-y^{2}\hat{j}+yz\hat{k})\cdot (\hat{k})\,dx\,dy 
      </me>
      <me>
        =\int\limits_{0}^{1}\int\limits_{0}^{1}yz\,dx\,dy  
        =\int\limits_{0}^{1}\int\limits_{0}^{1}y.1 \,dx\,dy  = \int\limits_{0}^{1}\,dx\int\limits_{0}^{1}y\,dy 
      </me>
      <me>
        = \int\limits_{0}^{1}\,dx\left(\frac{y^{2}}{2}\right)_{0}^{1}
        =\frac{1}{2}(x)^{1}_{0}=\frac{1}{2}. \hspace{3pt} \text{(as z=1)} 
      </me>
      <me>
        \iint\limits_{OAFG}\vec{F}\cdot \hat{n}\,ds 
        = \iint\limits_{OAFG}(4xz\hat{i}-y^{2}\hat{j}+yz\hat{k})\cdot (-\hat{j})\,dx\,dz
      </me>
      <me>
        =\int\limits_{0}^{1}\int\limits_{0}^{1}y^{2}\,dx\,dz=0.   \quad \text{(as y = 0)}
      </me>
      <me>
        \iint\limits_{BCDE}\vec{F}\cdot \hat{n}\,ds 
        = \iint\limits_{BCDE}(4xz\hat{i}-y^{2}\hat{j}+yz\hat{k})\cdot (\hat{j})\,dx\,dz=\int\limits_{0}^{1}\int\limits_{0}^{1}-y^{2}\,dx\,dz 
      </me>
      <me>
        =-\int\limits_{0}^{1}\int\limits_{0}^{1} dxdz  
        = -\int\limits_{0}^{1}\,dx\int\limits_{0}^{1}\,dz 
         = -\left(x\right)^{1}_{0}\left(z\right)^{1}_{0}=-1.   \hspace{3pt} \text{(as y=1)}
      </me>
      <me>
        \iint\limits_{ABEF}\vec{F}\cdot \hat{n}\,ds= \iint\limits_{ABEF}(4xz\hat{i}-y^{2}\hat{j}+yz\hat{k})\cdot (\hat{i})\,dy\,dz=\int\limits_{0}^{1}\int\limits_{0}^{1}(4xz\,dy\,dz
      </me>
      <me>
        =\int\limits_{0}^{1}\int\limits_{0}^{1} 4.1.z \,dy\,dz = 2.  \quad \text{(as x=1)}
      </me>
      <me>
        \iint\limits_{OCDG}\vec{F}\cdot \hat{n}\,ds= \iint\limits_{OCDG}(4xz\hat{i}-y^{2}\hat{j}+yz\hat{k})\cdot (-\hat{i})\,dy\,dz
      </me>
      <me>
        =-\int\limits_{0}^{1}\int\limits_{0}^{1}(4xz\,dy\,dz= 0. \quad \text{(as x=0)} 
      </me>
      
      On putting these values in eqn. <xref ref="eqn-vectint3"/>, we get -
      <me>
        \iint\limits_{S}\vec{F}\cdot \hat{n}\,ds = 0+\frac{1}{2}+0-1+2+0=\frac{3}{2}. \hspace{3pt} proved.
      </me>
    </p>
  </solution>
</example>

  
<example>
  <statement>
    <p>
      Evaluate <m>\iint\limits_{S}\vec{F}\cdot \hat{n}\,ds</m>, where 
      <m>\vec{F}=18z\hat{i}-12\hat{j}+3y\hat{k}</m> and  <m>S</m> is the part of plane 
      <m>2x+3y+6z=12</m>, which is located in the first octant. [In first octant the value of 
      <m>x, y, z</m> coordinates are positive.]
      <image source="fig20.png" width ="35%"/>
      </p>
  </statement>
  <solution>
    <p>
      The surface  <m>S</m> and its projection <m>R</m> on the x-y plane are shown in figure. 
      Now,
  <men xml:id="eqn-vectint4">
    \iint\limits_{S}\vec{F}\cdot \hat{n}ds=\iint\limits_{R}\vec{F}\cdot \hat{n}\frac{dxdy}{\mid \hat{n}\cdot\hat{k}\mid}
  </men>
  Where, <me>\hat{n}=\frac{\text{grad f} }{\mid \text{grad f} \mid}</me>
  <me>
    \text{grad} f=\vec{\nabla}f = \vec{\nabla}(2x+3y+6z-12)=2\hat{i}+3\hat{j}+6\hat{k}
  </me>
  <me>
    \mid \text{grad} f\mid =\sqrt{4+9+36} =\sqrt{49} = 7.
  </me>
  <me>
    \therefore  \hat{n}=\frac{2\hat{i}+3\hat{j}+6\hat{k}}{7}
  </me>
  and 
  <me>
    \hat{n}\cdot\hat{k} = \frac{1}{7}(2\hat{i}+3\hat{j}+6\hat{k})\cdot\hat{k}=\frac{6}{7}
  </me>
  also,
  <me>
   \vec{F}\cdot\hat{n}=(18z\hat{i}-12\hat{j}+3y\hat{k})\cdot \frac{1}{7}(2\hat{i}+3\hat{j}+6\hat{k}) = \frac{36z-36+18y}{7},
  </me>
  but from the equation of surface, ,<me>
    z=\frac{12-2x-3y}{6}
  </me>
  <me>
    \therefore   \vec{F}\cdot\hat{n}=\frac{1}{7}\left[36\left(\frac{12-2x-3y}{6}\right)-36+18y\right] 
  </me>
  <me>
    = \frac{1}{7}(72-12x-18y-36+18y) = \frac{1}{7}(36-12x).
  </me>
  From eqn. <xref ref="eqn-vectint4"/>
  <me>
    \iint\limits_{S}\vec{F}\cdot \hat{n}ds=\iint\limits_{R}\vec{F}\cdot \hat{n}\frac{dxdy}{\mid \hat{n}\cdot\hat{k}\mid}
=\iint\limits_{R} \frac{1}{7}(36-12x)\frac{dxdy}{6}\cdot7  
  </me>
  <me>
    = \iint\limits_{R} (6-2x) \,dx\,dy
  </me>
  To integrate it, consider the relation <m>2x+3y=12</m> and cover the whole region R, 
  i.e., the region BOA where y varies from <m>y=0</m> to <m>y=\frac{12-2x}{3}</m>, and 
  x varies from <m>x=0</m> to <m>x=6.</m>
<me>
  \therefore \quad \iint\limits_{S}\vec{F}\cdot \hat{n}\,ds
=\int\limits_{x=0}^{6}\int\limits_{y=0}^{(12-2x)/3}(6-2x)\,dx\,dy
</me>
<me>
 =\int\limits_{x=0}^{6}(6-2x)dx[y]^{(12-2x)/3}_{3} = \int\limits_{x=0}^{6}(24-12x+\frac{4}{3}x^{2})dx
</me>
<me>
  =24.
</me>
    </p>
  </solution>
</example>

<example>
  <statement>
    <p>
      Evaluate <m>\iint\limits_{S}\vec{F}\cdot \hat{n}ds</m>, 
      where <m>\vec{F}=z\hat{i}-x\hat{j}+3y^{2}z\hat{k}</m> and  <m>S</m> is the sutface of 
      cylinder <m>x^{2}+y^{2}=16</m> included in the first octant between <m>z=0,</m>  
      to <m>z=5,</m> as shown in figure.
      <image source="fig21.png" width="30%"/>
    </p>
  </statement>
  <solution>
    <p>
      <me>
        \iint\limits_{S}\vec{F}\cdot \hat{n}ds=\iint\limits_{R}\vec{F}\cdot \hat{n}\frac{dxdz}{\mid \hat{n}\cdot\hat{j}\mid} 
      </me>
      But,
      <me>
        \hat{n}=\frac{grad f}{\mid grad f\mid}= \frac{\vec{\nabla f}}{\mid\vec{\nabla f}\mid} =\frac{\vec{\nabla}(x^{2}+y^{2}-16)}{\mid\vec{\nabla}(x^{2}+y^{2}-16)\mid} 
      </me>
      <me>
        =\frac{(2x\hat{i}+2y\hat{j})}{\sqrt{(4x^{2}+4y^{2})}} 
        =\frac{(x\hat{i}+y\hat{j})}{\sqrt{(x^{2}+y^{2})}} 
        =\frac{(x\hat{i}+y\hat{j})}{4},
      </me>
      and 
      <me>
        \vec{F}\cdot\hat{n}=(z\hat{i}-x\hat{j}+3y^{2}z\hat{k}).\frac{1}{4}(x\hat{i}+y\hat{j}) 
        = \frac{1}{4}(xz+xy),
      </me>
      also,
      <me>
        \hat{n}\cdot\hat{j}= \frac{1}{4}(x\hat{i}+y\hat{j})\cdot\hat{j}=\frac{1}{4}y
      </me>
      <me>
        \therefore   \iint\limits_{R}\vec{F}\cdot \hat{n}\frac{dxdz}{\mid \hat{n}\cdot\hat{j}\mid} =\iint\limits_{R}\frac{1}{4}(xz+xy)\cdot\frac{4}{y}\,dx\,dz 
      </me>
      <me>
        =\iint\limits_{R}\left(\frac{xz}{\sqrt{(16-x^{2})}}+x\right)\,dx\,dz
      </me>
      <me>
        = \int\limits_{x=0}^{4}\int\limits_{z=0}^{5}\left(\frac{xz}{\sqrt{(16-x^{2})}}+x\right)dxdz 
         = \int\limits_{z=0}^{5}(4z+8)dz=90.    
      </me>
    </p>
  </solution>
</example>

<example>
  <statement>
    <p>
      If <m>\vec{F}=2z\hat{i}-x\hat{j}+y\hat{k}</m>, evaluate <m>\iiint\limits_{V}\vec{F}\,dv</m> 
      where <m>V</m> is the region bounded by the surfaces <m>x=0</m>,  <m>x=2</m>, <m>y=0</m>,
      <m>y=4</m>, and <m>z=x^2</m>,  <m>z=2</m>.
    </p>
  </statement>
  <solution>
    <p>
     <me>
      \iiint\limits_{V}\vec{F}dv=\iiint\limits_{V}(2z\hat{i}-x\hat{j}+y\hat{k})\,dx\,dy\,dz 
     </me>
      <me>
        =\int\limits_{x=0}^{2}\int\limits_{y=0}^{4}\int\limits_{z=x^{2}}^{2}(2z\hat{i}-x\hat{j}+y\hat{k})\,dx\,dy\,dz 
      </me>
      <me>
        =\int\limits_{0}^{2}dx\int\limits_{0}^{4}dy[z^{2}\hat{i}-xz\hat{j}+yz\hat{k}]^{2}_{x^{2}} 
      </me>
      <me>
        =\int\limits_{0}^{2}dx\int\limits_{0}^{4}dy[4\hat{i}-2x\hat{j}+2yz\hat{k}-x^{4}\hat{i}+x^{3}\hat{j}-x^{2}y\hat{k}]
      </me>
      <me>
        = \int\limits_{0}^{2}dx\left[4y\hat{i}-2xy\hat{j}+y^{2}\hat{k}-x^{4}y\hat{i}+x^{3}y\hat{j}-\frac{x^{2}y^{2}}{2}\hat{k}\right]^{4}_{0}  
      </me>
      <me>
        =	\int\limits_{0}^{2}(16\hat{i}-8x\hat{j}+16\hat{k}-4x^{4}\hat{i}+4x^{3}\hat{j}-8x^{2}\hat{k})\,dx
      </me>
      <me>
        = \left[16x\hat{i}-4x^{2}\hat{j}+16\hat{k}-\frac{4}{5}x^{5}\hat{i}+x^{4}\hat{j}-\frac{8}{3}x^{3}\hat{k}\right]^{2}_{0}
      </me>
      <me>
        =32\hat{i}-16\hat{j}+32\hat{k}-\frac{128}{5}\hat{i}+16\hat{j}-\frac{64}{3}\hat{k}
      </me>
      <me>
        =\frac{32}{5}\hat{i}+32\hat{k}=\frac{32}{5}(3\hat{i}+5\hat{k}).   
      </me>
    </p>
  </solution>
</example>

<example>
  <statement>
    <p>
    Evaluate <m>\iiint\limits_{V}\phi \,dV</m>, where <m>V</m> is the closed region bounded 
    by the planes <m>4x+2y+z=8</m>, <m>x=0</m>, <m>y=0</m> and <m>z=0</m>, and <m>\phi=45x^{2}y</m>.
    </p>
  </statement>
  <solution>
    <p>
      <me>
        \iiint\limits_{V}\phi dV=\iiint\limits_{V}45x^{2}y \,dx\,dy\,dz.
      </me>
      <hint>
        <p>
         <m>z</m> varies from <m>0</m> to <m>8-4x-2y</m>, <m>y</m> varies from <m>0</m> to 
         <m>4-2x</m>, and <m>x</m> varies from <m>0</m> to <m>2</m>.
        </p>
      </hint>
      <answer>
        <p>
          On solving, we get- 
          <me>
            \iiint\limits_{V}\phi \,dV = 128.
          </me>	 
        </p>
      </answer>
    </p>
  </solution>
</example>
  </paragraphs>
 
  <paragraphs>
    <title>Gauss's Divergence Theorem</title>
   <example>
    <statement>
      <p>
        The electric field <m>\vec{E}</m> of a certain space is given by <m>E_{x}=(ax+by+c), E_{y}=0, E_{z}=0.</m> 
        Use Gauss's theorem to evaluate the charge enclosed in a cube of side length <m>L</m>.
      </p>
    </statement>
    <solution>
      <p>
        From divergence theorem, we have
        <me>
          \mathop{\vcenter{\huge\unicode{x222F}\,}}\limits_{S} \vec{E}\cdot\vec{\,dS}= \iiint\limits_{V}(\vec{\nabla}\cdot \vec{E})\,dV=\iiint\limits_{V}\left[\frac{\delta E_{x}}{\delta x}+\frac{\delta E_{y}}{\delta y}+\frac{\delta E_{z}}{\delta z}\right] \,dV 
        </me>
        Here, <m>\frac{\delta E_{x}}{\delta x}=a</m>, while <m>E_{y}</m>  and <m>E_{z}</m> is each zero.
<men xml:id="eqn-diver1">
  \therefore  \quad \mathop{\vcenter{\huge\unicode{x222F}\,}}_{S} \vec{E}\cdot\vec{\,dS} = \iiint\limits_{V} a \,dV = aV=aL^{3} 
</men>
Since, volume of a cube = <m>L^{3}</m>. 
      </p>
      <p>
        But, from Gauss's  law in electrostatics, we have  -
        <men xml:id="eqn-diver2">
          \mathop{\vcenter{\huge\unicode{x222F}\,}}\limits_{S} \vec{E}\cdot\vec{\,dS} = \frac{q}{\epsilon_{o}}   
        </men>
        where <m>q</m> is the charge within the surface <m>S</m> which encloses the volume <m>V</m>. 
        Equating eqns. <xref ref="eqn-diver1"/> and <xref ref="eqn-diver2"/>, we get -
        <me>
          \frac{q}{\epsilon_{o}}  = aL^{3}.
        </me>
        <me>
          \therefore   \quad    q =  \epsilon_{o} a L^{3}.
        </me>
      </p>
    </solution>
   </example>

   <example>
    <statement>
      <p>
        Use divergence theorem to evaluate <m>\mathop{\vcenter{\huge\unicode{x222F}\,}}\limits_{S} \vec{A}\cdot\vec{dS}</m> 
        where <m>\vec{A}=x^{3}\hat{i}+ y^{3}\hat{j}+z^{3}\hat{k}</m> and <m>S</m> is the surface of the sphere 
        <m>x^{2}+y^{2}+z^{2}=a^{2}</m>.
      </p>
    </statement>
    <solution>
      <p>
        The divergence theorem is 
        <me>
          \mathop{\vcenter{\huge\unicode{x222F}\,}}\limits_{S} \vec{A}\cdot\vec{dS}=\iiint\limits_{V} div\vec{A} \,dV
        </me>
         <me>
          = \iiint\limits_{V} \left(\hat{i}\frac{\partial}{\partial x}+\hat{j}\frac{\partial}{\partial y} 
          +\hat{k}\frac{\partial}{\partial z}\right)\cdot (x^{3}\hat{i}+ y^{3}\hat{j}+z^{3}\hat{k})\,dV
         </me>
         <me>
          =\iiint\limits_{V} \left(3x^{2}+ 3y^{2}+3z^{2}\right)dV= 3\iiint\limits_{V} \left(x^{2}+ y^{2}+z^{2}\right)\,dV 
          =3\iiint\limits_{V}a^{2}dV= 3a^{2}\iiint\limits_{V}\,dV = 3a^{2}\left(\frac{4}{3}\pi a^{3}\right) = 4\pi a^{5}.
         </me>
           </p>
    </solution>
   </example>

   <example>
    <statement>
      <p>
        Evaluate surface integral <m>\iint\limits_{S} \vec{F}\cdot\hat{n}\,dS</m> 
        where <m>\vec{F}=(x^{2}+ y^{2}+z^{2})(\hat{i}+\hat{j}+\hat{k})</m>, and S is the surface 
        of the tetrahedron <m>x=0,y=0,z=0, x+y+z=2,</m> and <m>\hat{n}</m> is the unit normal 
        in the outward direction to the closed surface S, as shown in the figure.
         <image source="fig24.png" width="30%"/>
       </p>
    </statement>
    <solution>
      <p>
       We have -
       <me>
        \iint\limits_{S} \vec{F}\cdot\hat{n}\,dS = \iiint\limits_{V} div\vec{F} \,dV 
       </me>
        <me>
          =\iiint\limits_{V} \left(\hat{i}\frac{\partial}{\partial x}+\hat{j}\frac{\partial}{\partial y}+\hat{k}\frac{\partial}{\partial z}\right)\cdot (x^{2}+ y^{2}+z^{2})(\hat{i}+\hat{j}+\hat{k})\,dV
        </me>
        <me>
          =\iiint\limits_{V} \left(2x+2y+2z\right)\,dV =2\iiint\limits_{V} \left(x+y+z\right)\,dV = 2\iiint\limits_{V}2\,dV 
        </me>
        <me>
          = 4 \text{[volume of tetrahedron OABC]}
        </me>
        <me>
          = 4[\frac{1}{3} \text{Area of the base}\hspace{2pt} OAB \times \text{height}\hspace{2pt} OC] 
        </me>
        <me>
          = 4[\frac{1}{3}(\frac{1}{2}\times 2 \times 2)\times 2] = \frac{16}{3}.       
        </me>
      </p>
    </solution>
   </example>
  </paragraphs>

  <paragraphs>
    <title>Stoke's Theorem</title>
    <example>
      <statement>
        <p>
          Use Stoke's theorem to evaluate <m>\oint\limits_{C}\left[(2x-y)\,dx-yz^{2}\,dy-y^{2}z\,dz\right]</m> 
          where C is the circle <m>x^{2}+y^{2}=1</m>,  corresponding to the surface of sphere of unit 
          radius, as shown in the figure.  <image source="fig25.png" width="30%"/>
        </p>
      </statement>
      <solution>
        <p>
          <me>
            \int\limits_{C}\left[(2x-y)\,dx-yz^{2}\,dy-y^{2}z\,dz\right] 
          </me>
          <me>
            =\int\limits_{C}\left[(2x-y)\hat{i}-yz^{2}\hat{j}-y^{2}z\hat{k}\right]\cdot(\hat{i}dx+\hat{j}dy+\hat{k}\,dz) =\int\limits_{C}\vec{F}\cdot\vec{\,dr} 
          </me>
          From Stoke's theorem,
         <men xml:id="eqn-stcurl1">
          \int\limits_{C}\vec{F}\cdot\vec{dr}=\iint\limits_{S}curl\vec{F}\cdot\hat{n}ds 
         </men>
         <me>
          \therefore \quad curl\vec{F}=\vec{\nabla}\times\vec{F}=
          {\begin{vmatrix} \hat{i} &amp; \hat{j} &amp; \hat{k} \\ \frac{\partial}{\partial x} &amp; \frac{\partial}{\partial y} &amp; \frac{\partial}{\partial z}\\2x-y &amp; -yz^{2} &amp; -y^{2}z \end{vmatrix}}
         </me>
         Putting the value of <m>curl\vec{F}</m> in eqn. <xref ref="eqn-stcurl1"/>, we get -
          <me>
            \int\limits_{C}\vec{F}\cdot\vec{\,dr}=\iint\limits_{S}\hat{k}\cdot\hat{n}\,ds=\iint\limits_{S}\,dx\,dy 
          </me>
          <m>[\because \,dx\,dy=\hat{n}\cdot\hat{k}\,ds]</m>
          <me>
            =\int\limits_{-1}^{+1}\,dx\int\limits_{-\sqrt{1-x^{2}}}^{+\sqrt{1-x^{2}}}\,dy=\int\limits_{-1}^{+1}[\sqrt{1-x^{2}}+\sqrt{1-x^{2}}] \,dx 
          </me>
         
          <me>
            =2\int\limits_{-1}^{+1}[\sqrt{1-x^{2}}]dx =2\left[\frac{x}{2} \sqrt{1-x^{2}}+\frac{1}{2} sin^{-1}x\right]^{+1}_{-1} 
          </me>
          <me>
            =2\left[0+\frac{1}{2} (\frac{\pi}{2})-\frac{1}{2} (\frac{-\pi}{2})\right] = \pi. 
          </me>
        </p>
      </solution>
    </example>

    <example>
      <statement>
        <p>
          Apply Stoke's theorem to evaluate <m>\iint\limits_{S}curl\vec{V}\cdot\hat{n}\,ds</m>, 
          where <m>\vec{V}=\hat{i}y+\hat{j}z+\hat{k}x</m>, S is the surface of the paraboloid 
          <m>z=1-x^{2}-y^{2},\quad z\geq 0,</m> and <m>\hat{n}</m> is the  unit normal to S, as shown in figure below.
          <image source="fig26.png" width="30%"/>
        </p>
      </statement>
      <solution>
        <p>
          <me>
            \iint\limits_{S}curl\vec{V}\cdot\hat{n}ds = \int\limits_{c}\vec{V}\cdot\vec{\,dr} 
            =\int\limits_{c}(\hat{i}y+\hat{j}z+\hat{k}x)\cdot(\,dx\hat{i}+\,dy\hat{j}+\,dz\hat{k})
          </me>
          <me>
            =\int\limits_{C}(y\,dx+z\,dy)= \int\limits_{C}y\,dx \quad  [\because z=0]
          </me>
          Now for circle, we have - 
        <m>x=1.\cos\theta, \quad y= 1.\sin\theta </m> 
        <me>
          \therefore \iint\limits_{S}curl\vec{V}\cdot\hat{n}\,ds= \int\limits_{0}^{2\pi}\sin\theta.(-\sin\theta)\,d\theta = \int\limits_{0}^{2\pi}\sin^{2}\theta \,d\theta 
        </me>
        <me>
          =\frac{1}{2}\int\limits_{0}^{2\pi}(\cos 2\theta -1) \,d\theta
          =\frac{1}{2}\left(\frac{\sin2\theta}{2}-\theta\right)^{2\pi}_{0} = -\pi. 
        </me>
        </p>
      </solution>
    </example>

    <example>
      <statement>
        <p>
          Verify Stoke's thereom for the vector field <m>\vec{F}=(2y+z)\hat{i}+(x-z)\hat{j}+(y-x)\hat{k}</m> 
          ver the portion of the plane <m>x+y+z=1</m> cut off by the coordinate planes.
        </p>
      </statement>
      <solution>
        <p>
          Consider the surface <m>S</m> of boundary <m>ABC</m> as shown by the arrows in the figure below.	
          <image source="fig27.png" width="30%"/>
          <me>
            \int\limits_{C}\vec{F}\cdot\vec{\,dr}=\int\limits_{C}[(2y+z)\hat{i}+(x-z)\hat{j}+(y-x)\hat{k}]\cdot (\,dx\hat{i}+\,dy\hat{j}+\,dz\hat{k}) 
          </me>
          <me>
            =\int\limits_{C}[(2y+z)\,dx+(x-z)\,dy+(y-x)\,dz].
          </me>
          But,
          <men xml:id="eqn-stcurl2">
            \int\limits_{C}\vec{F}\cdot\vec{\,dr}=\int\limits_{AB}\vec{F}\cdot\vec{\,dr}+\int\limits_{BC}\vec{F}\cdot\vec{\,dr}+\int\limits_{CA}\vec{F}\cdot\vec{\,dr}. 
          </men>
          Along AB, <m>z=0</m>, <m>\,dz=0</m>, and <m>x+y=1.</m>
          <me>
            \int\limits_{AB}\vec{F}\cdot\vec{\,dr}= \int\limits_{A}^{B}(2y\,dx+x\,dy) = \int\limits_{1}^{0}2(1-x)\,dx+\int\limits_{0}^{1}(1-y)\,dy 
          </me>
          <me>
            =2\left(x-\frac{x^{2}}{2}\right)^{0}_{1}+\left(y-\frac{y^{2}}{2}\right)^{1}_{0}=-\frac{1}{2}.
          </me>
          Along BC, <m>x=0</m>, <m>\,dx=0</m>, and <m>y+z=1</m>.
          <me>
            \int\limits_{BC}\vec{F}\cdot\vec{\,dr}= \int\limits_{B}^{C}(-z\,dy+y\,dz) = \int\limits_{1}^{0}(1-y)\,dy+\int\limits_{0}^{1}(1-z)\,dz
          </me>
          <me>
            =-\left(y-\frac{y^{2}}{2}\right)^{0}_{1}+\left(z-\frac{z^{2}}{2}\right)^{1}_{0}=1.
          </me>
          Along CA, <m>y=0</m>, <m>\,dy=0</m>, and <m>x+z=1</m>.
          <me>
            \int\limits_{CA}\vec{F}\cdot\vec{\,dr}= \int\limits_{C}^{A}(z\,dx-x\,dz)= \int\limits_{0}^{1}(1-x)\,dx-\int\limits_{1}^{0}(1-z)\,dz
          </me>
          <me>
            =\left(x-\frac{x^{2}}{2}\right)^{1}_{0}-\left(z-\frac{z^{2}}{2}\right)^{0}_{1}=1. 
          </me>
          Hence, 
          <men xml:id="eqn-stcurl3">
            \int\limits_{C}\vec{F}\cdot\vec{\,dr}=-\frac{1}{2}+1+1=\frac{3}{2}. 
          </men>
          Also,
          <me>
            {\begin{vmatrix} \hat{i} &amp; \hat{j} &amp; \hat{k} \\ \frac{\partial}{\partial x} &amp; \frac{\partial}{\partial y} &amp; \frac{\partial}{\partial z}\\2y+z &amp; x-z &amp; y-x \end{vmatrix}} 
          </me>
          <me>
            = \hat{i}(1+1)-\hat{j}(-1-1)+\hat{k}(1-2) = 2\hat{i}+2\hat{j}-\hat{k}.
          </me>
          
        </p>
        <p>
          Now integrate this vector over the three surfaces <m>OAB</m>, <m>OBC</m>, and <m>OCA</m> 
          lying on the plane <m>x+y+z=1</m>. Over the surface  <m>OAB</m>, 
          <m>\hat{n}=\hat{k}, \,ds=\frac{1}{2}\,dx\,dy</m>,  
           The surface integral over the surface <m>OAB</m>,
           <me>
            \iint\limits_{S}\left(\vec{\nabla}\times\vec{F}\right)\cdot\hat{n}ds=\iint\limits_{S}(2\hat{i}+2\hat{j}-\hat{k})\cdot\hat{k}\frac{1}{2}\,dx\,dy
           </me>
           <me>
            =\int\limits_{0}^{1}\int\limits_{0}^{1}(-\frac{1}{2})\,dx\,dy= -\frac{1}{2}[x]^{1}_{0}[y]^{1}_{0}=-\frac{1}{2}
           </me>
           Over the surface  <m>OBC</m>, <m>\hat{n}=\hat{i}, \,ds=\frac{1}{2}\,dy\,dz</m>, 
           The surface integral over the surface <m>OBC</m>,
           <me>
            \iint\limits_{S}\left(\vec{\nabla}\times\vec{F}\right)\cdot\hat{n}\,ds=\iint\limits_{S}(2\hat{i}+2\hat{j}-\hat{k})\cdot\hat{i}(\frac{1}{2})\,dy\,dz
           </me>
           <me>
            =\int\limits_{0}^{1}\int\limits_{0}^{1}(2.\frac{1}{2})\,dy\,dz= 1.
           </me>
        </p>
        <p>
          Over the surface  <m>OCA</m>, <m>\hat{n}=\hat{j}, \,ds=\frac{1}{2}\,dx\,dz</m>, 
          The surface integral over the surface <m>OCA</m>,
          <me>
            \iint\limits_{S}\left(\vec{\nabla}\times\vec{F}\right)\cdot\hat{n}\,ds=\iint\limits_{S}(2\hat{i}+2\hat{j}-\hat{k})\cdot\hat{j}(\frac{1}{2})\,dx\,dz
          </me>
          <me>
            =\int\limits_{0}^{1}\int\limits_{0}^{1}(2.\frac{1}{2})\,dx\,dz= 1.
          </me>
          Therefore, total surface integral = 
          <men xml:id="eqn-stcurl4">
             \iint\limits_{S}\left(\vec{\nabla}\times\vec{F}\right)\cdot\hat{n}\,ds =-\frac{1}{2}+1+1=\frac{3}{2}. 
          </men>
          Hence from eqns. <xref ref="eqn-stcurl3"/>  and <xref ref="eqn-stcurl4"/>, Stoke's theorem is verified.
        </p>
      </solution>
    </example>
  </paragraphs>

</section>

