<?xml version="1.0" encoding="UTF-8"?>

<section xml:id="sec_fifth-frinterval" xmlns:xi="http://www.w3.org/2001/XInclude">
  <title>Change of Interval</title>
  <introduction>
   <p>  <idx><h>Change of interval</h></idx>
    The period of a function in Fourier series sometimes appears in time like <m>T</m>  
    or in length like <m>2c</m>, then in order to use Fourier series expansion such 
    period must be converted into in angle like <m>2\pi</m>. In that case the independent 
    variable <m>x</m> of a function <m>f(x)</m> must also be changed proportionally. 
    Suppose we want to represent the function <m>f(x)</m> defined in the closed 
    interval <m>(-c, c)</m> by a Fourier series, <m>c</m> being any positive real 
    number. We consider this interval as a result of elongating (or compressing) 
    the interval <m>[-\pi, \pi]</m>. The interval <m>-c \leq x \leq c</m> is transformed 
    into the interval <m>-\pi \leq x \leq \pi</m> by the transformation <m>z=\frac{\pi x}{c}</m>.
				</p>
        <p>
        Suppose the function <m>F(z)</m> is expanded in the interval of <m>2\pi</m> as 
        <men xml:id="eqn-fourier_chinter1">
          F(z) =	\frac{a_{o}}{2} + \sum\limits_{n=1}^{\infty}\left[a_{n}\cos nz + b_{n}\sin nz\right] 
        </men>
          If <m>f(x)</m> has an interval of <m>2c</m>, then we can write the <m>2c </m> is a period 
          of variable <m>x</m>.
          or, <m>1</m> is the period of variable <m>x/2c,</m>
          <me>\therefore   2\pi \quad 	\text{is the period of variable} </me>
          <me>
             \frac{x}{2c}.2\pi = \frac{\pi x}{c}
          </me>
            i.e., <m>z=\frac{\pi x}{c}</m>, (because both the variables have same period of <m>2\pi</m>.)
    </p>
    <p>
      Now, 
      <me>
        f(x) = f\left(\frac{cz}{\pi}\right) = F(z)\quad \text{(say)}
      </me>
        Hence, 
        <me>
          a_{0}=  \frac{1}{\pi}\int\limits_{-\pi}^{\pi}F(z)\,dz
        </me>
         <me>
          =\frac{1}{\pi}\int\limits_{-\pi}^{\pi} f\left(\frac{cz}{\pi}\right)\,dz = \frac{1}{\pi}\int\limits_{-c}^{c} f(x)\,d\left(\frac{\pi x}{c}\right) = \frac{1}{c}\int\limits_{-c}^{c}f(x)\,dx 
         </me>
         <me>
          a_{n}= \frac{1}{\pi}\int\limits_{-\pi}^{\pi}F(z) \cos nz\,dz = \frac{1}{\pi}\int\limits_{-\pi}^{\pi}f\left(\frac{cz}{\pi}\right)\cos nz\,dz 
         </me>
         <me>
          = \frac{1}{\pi}\int\limits_{-c}^{c}f(x)\cos  \left(\frac{n \pi x}{c}\right)\,d \left(\frac{\pi x}{c}\right) = \frac{1}{c}\int\limits_{-c}^{c}f(x)\cos  \frac{n \pi x}{c}\,dx
         </me>
         and 
         <me>
          b_{n}= \frac{1}{\pi}\int\limits_{-\pi}^{\pi}F(z) \sin nz\,dz = \frac{1}{c}\int\limits_{-c}^{c}f(x)\sin  \frac{n \pi x}{c}\,dx 
         </me>
          The function <m>f(x)</m> is now expressed as 
          <men xml:id="eqn-fourier_chinter2">
            f(x) = \frac{a_{o}}{2} + \sum\limits_{n=1}^{\infty}\left[a_{n}\cos \left(\frac{n\pi x}{c}\right) + b_{n}\sin \left(\frac{n\pi x}{c}\right)\right] 
          </men>
          for the period <m>2c</m>.
      </p>
   
     </introduction>
 
 <subsection xml:id="subsec-fourier_complex">
  <title>Complex Form of Fourier Series</title>
  <p> <idx><h>complex fourier series</h></idx>
    The complex form of Fourier series is obtained by expressing  <m>\cos nx</m> and 
    <m>\sin nx</m> in the exponential form, i.e.,	 
    <me>
      f(x) = \frac{a_{o}}{2} + \sum\limits_{n=1}^{\infty}\left[a_{n}\cos nx + b_{n}\sin nx\right]
    </me>
    <me>
      =\frac{a_{o}}{2} + \sum\limits_{n=1}^{\infty}a_{n}\left[\frac{e^{inx}+e^{-inx}}{2}\right] + \sum\limits_{n=1}^{\infty}b_{n}\left[\frac{e^{inx}-e^{-inx}}{2i}\right]	
    </me>
    <me>
      =\frac{a_{o}}{2} + \sum\limits_{n=1}^{\infty}\left[\frac{a_{n}}{2}-\frac{ib_{n}}{2}\right]e^{inx}+\sum\limits_{n=1}^{\infty}\left[\frac{a_{n}}{2}+\frac{ib_{n}}{2}\right]e^{-inx} 
    </me>
    <me>
       =c_{0}+\sum\limits_{n=1}^{\infty}c_{n}e^{inx}+\sum\limits_{n=1}^{\infty}c_{-n}e^{-inx}
    </me>
    
      <men xml:id="eqn-comp_fourier1">
        \therefore  \quad f(x) = \sum\limits_{n=-\infty}^{\infty}c_{n}e^{inx};
      </men>
      where,
        <me>
          \begin{cases} 
               c_{0} = \frac{a_{0}}{2}\\
                   c_{n} = \frac{1}{2}(a_{n}-ib_{n})\\ 
                      c_{-n} = \frac{1}{2}(a_{n}+ib_{n}) 
                      \end{cases}	
        </me>
          Equation <xref ref="eqn-comp_fourier1"/> is a complex form of Fourier series. 
          On multiplying both sides of equation <xref ref="eqn-comp_fourier1"/> by  
          <m>e^{-imx}</m> and integrating w.r.t. 'x', we get -
           	 	<me>
                \int\limits_{c}^{c+2\pi}f(x)e^{-imx} \,dx = \sum\limits_{n=-\infty}^{\infty}c_{n}\int\limits_{c}^{c+2\pi}e^{i(n-mx)} \,dx 
              </me>
              <me>
                = \sum\limits_{n=-\infty}^{\infty}c_{n}2\pi \delta_{mn}=2\pi c_{m}
              </me>
              
              	<me>
                  \therefore  c_{n}	=\frac{1}{2\pi}\int\limits_{c}^{c+2\pi}f(x)e^{-inx} \,dx.
                </me>
              The function <m>f(x)</m> is being defined in the interval <m>[c, c+2\pi]</m>. Hence,
              <me>
                c_{0}=\frac{1}{2\pi}\int\limits_{c}^{c+2\pi}f(x) \,dx = \frac{a_{0}}{2}.
              </me>
    </p>
 </subsection>

<subsection xml:id="subsec-fourier_intg">
  <title>Fourier Integral</title>
  <p>
    <idx><h>Fourier integral</h></idx>
    Fourier series of a periodic function <m>f(x)</m> in the interval [-l,l]  is given by 
    <men xml:id="eqn-fourier_intg1">
      f(x) = \frac{a_{o}}{2} + \sum\limits_{n=1}^{\infty}\left[a_{n}\cos \left(\frac{n\pi x}{l}\right) + b_{n}\sin \left(\frac{n\pi x}{l}\right)\right] 
    </men>
    	where,
      <me>
        a_{0}=\frac{1}{l}\int\limits_{-l}^{l}f(t) \,dt,
      </me>
      <me>
        a_{n} = \frac{1}{l}\int\limits_{-l}^{l}f(t) \cos \left(\frac{n\pi t}{l}\right)\,dt, 
      </me>
      and 
      <me>
        b_{n} = \frac{1}{l}\int\limits_{-l}^{l}f(t) \sin \left(\frac{n\pi t}{l}\right)\,dt.
      </me>
        Substituting these values in equation <xref ref="eqn-fourier_intg1"/>, we get -
        <me>
           f(x) = \frac{1}{2l}\int\limits_{-l}^{l}f(t) \,dt 
        </me>
        <me>
          + \frac{1}{l}\sum\limits_{n=1}^{\infty}\left[\int\limits_{-l}^{l}f(t)\left\{\cos \left(\frac{n\pi x}{l}\right) \cos \left(\frac{n\pi t}{l}\right)\right.
        </me>
        <me>
          \left.+ \sin \left(\frac{n\pi x}{l}\right)\sin \left(\frac{n\pi t}{l}\right)\right\}\,dt \right]
        </me>
        
        or,
        <men xml:id="eqn-fourier_intg2">
          f(x) = \frac{1}{2l}\int\limits_{-l}^{l}f(t) \,dt+ \frac{1}{l}\sum\limits_{n=1}^{\infty}f(t) \cos \left[\frac{n\pi}{l}(x-t)\right]\,dt
        </men>
        If we set
        <m> u=\frac{n\pi}{l} </m>  so that  <m> \bigtriangleup u= \frac{\bigtriangleup n\pi}{l}, </m>
        where  <m> \bigtriangleup n = 1  </m>  and 
        <m>\frac{1}{l}=\frac{\bigtriangleup u} {\pi}.</m> Hence, equation 
        <xref ref="eqn-fourier_intg2"/> becomes
          <me>
           f(x) = \frac{1}{2l}\int\limits_{-l}^{l}f(t) \,dt+ \frac{1}{\pi}\sum\limits_{u=\pi/l}^{\infty}\bigtriangleup u \int\limits_{-l}^{l}f(t) \cos \left[u(x-t)\right]\,dt  
          </me>
          or,
           <men xml:id="eqn-fourier_intg3">
            f(x) = \frac{1}{\pi}\int\limits_{0}^{\infty}\, du \int\limits_{-\infty}^{\infty}[u(x-t)]\,dt 
           </men>
            Since
            <me>
               \frac{1}{2l}\int\limits_{-l}^{l}f(t) \,dt \rightarrow 0,
            </me>
           and 
           <me>
             \sum\limits_{u=\pi/l}^{\infty}\bigtriangleup u \rightarrow   \int\limits_{0}^{\infty} \,du 
           </me>
          [as <m>l\rightarrow \infty</m>]. Equation <xref ref="eqn-fourier_intg3"/>
           is called the Fourier integral formula.
    </p>
</subsection>

<subsection xml:id="subsec-gibbs_phen">
  <title>Gibb's Phenomenon</title>
  <p>
    <idx><h>Gibb's Phenomenon</h></idx> Gibb's phenomenon describes a special case 
    where a funciton has a jump discontinuity. An anomaly occurs near the discontinuity 
    in an approximation of an original function using its Fourier series. 
    The values of the partial sums near the discontinuity overshoot or undershoot 
    the fuction value. As more and more terms incorporate in the partial sums the 
    graph of the function resembles the original function more closely away from 
    the point of discontinuity. However, the blips near the discontinuity persists. 
    Although the size of blips decreases in width they appear to remain at the same height. 
    In other words, the series converges correctly at any point due to increase of terms 
    in the partial sums, but the blips do not converges to zero as shown in figure <xref ref="fig-Gibbs"/>. 
    This lack of improvement in the approximation near the discontinuity menifested in 
    the continual presence of the overshoot or undershoot is the Gibb's phenomenon. 
    </p>
     <figure xml:id="fig-Gibbs">
              <caption>Gibbs Phenomena</caption>
              <image source="Gibbs.png" width ="65%"/>
          </figure>

          <p>
            In the immediate vicinity of a jump discontinuity i.e. at 
            <m>x{+}</m> or <m>x{-}</m>, the function <m>f(x)</m> is not same and 
            hence the convergence of the Fourier series is not uniform 
            since <m>f(x) \rightarrow \frac{1}{2}[f(x+0)+f(x-0)]</m>. 
            Here partial sums move progressively closer to the function as the number of terms 
            is increased, but the partial sums (approximating curves) overshoot or undershoot 
            the function at the jump discontinuity. To verify the validity of Gibbs phenomenon, 
            i.e. Fourier expansion for functions which are discontinuous but piecewise smooth, 
            Bocher considered the following specific function defined by 	
            <men xml:id="eqn-gibbs1">
              f(x) = \frac{1}{2}(\pi-x)   \quad  (0\leq x \leq 2\pi)
            </men>
              here <m>f(0) = 0</m> and <m>f(x+2\pi) =f(x)</m>. i.e., 
              the function jumps by <m>\pi</m> at the points <m>x = \pm 2m\pi</m> 
              where <m> m=0,1,2,\cdots</m>. The Fourier coefficients of this function 
              are <m>a_{0}=a_{n}=0, \quad b_{n}=\frac{1}{n}</m>.
            </p>
            <p>
              Thus, if the Fourier expansion for such functions is valid, we have 
              <men xml:id="eqn-gibbs2">
                s(x)=\displaystyle{\lim_{p \to \infty}} s_{p}(x) = \sum\limits_{n=1}^{\infty}\frac{\sin nx}{n}
              </men>
              The partial sum is given by 
              <me>
                s_{p}(x) =	 \sum\limits_{n=1}^{p}\frac{\sin nx}{n} = \sin x +\frac{1}{2}\sin 2x +\cdots+\frac{1}{p}\sin px
              </me>
              <me>
                =\int\limits_{0}^{x}(\cos u +\cos 2u + \cdots + \cos pu)\,du  =\int\limits_{0}^{x}\left(\sum\limits_{n=1}^{p}\cos nu\right)\,du
              </me>
              <me>
                =\frac{1}{2} \int\limits_{0}^{x}\frac{\sin\left[\left(p+\frac{1}{2}\right)u\right]}{\sin u/2}\,du -\frac{x}{2} 
              </me>
              <me>
                \left[\because  \sum\limits_{n=1}^{p}\cos nx = \frac{\sin \left(p+\frac{1}{2}\right)x}{2\sin x/2}-\frac{1}{2}\right]
              </me>
              The remainder, 
              <me>
                R_{p}(x) = 	\sum\limits_{n=p+1}^{\infty}\frac{\sin nx}{n}		=f(x)-s_{p}(x) = \frac{\pi-x}{2}-s_{p}(x)
              </me>
              <men xml:id="eqn-gibbs3">
               	\therefore  \quad R_{p}(x)=\frac{\pi}{2}-	\frac{1}{2}\int\limits_{0}^{x}\frac{\sin\left[\left(p+\frac{1}{2}\right)u\right]}{\sin u/2}\,du 
              </men>
              or, 
              <men xml:id="eqn-gibbs4">
                R_{p}(x)=\frac{\pi}{2}-	\int\limits_{0}^{(p+1/2)x}\frac{\sin u}{u}\,du +\rho_{p}(x)
              </men>
              where  
              <men xml:id="eqn-gibbs5">
                \rho_{p}(x)=\int\limits_{0}^{x}\left\{ \frac{\sin u/2 -u/2}{u \sin u/2}\right\}\sin \left[\left(p+\frac{1}{2}\right)u\right]\,du
              </men> 
              On differentiating equation <xref ref="eqn-gibbs4"/> with respect to 'x', 
              we find that <m>R_{p}(x)</m> has maxima or minima at	 
              <me>
                x_{k}=\frac{2\pi k}{2p+1}   \quad (k=0,1,2,\cdots)	
              </me>
              				The value of <m>R_{p}(x)</m> at <m>x_{k}</m> is 
                      <men xml:id="eqn-gibbs6">
                        R_{p}(x)=\frac{\pi}{2}-\int\limits_{0}^{\pi k}\frac{\sin u}{u}\,du + \rho_{p}\left(\frac{2\pi k}{2p+1}\right)
                      </men> 
                      As <m>p\rightarrow \infty</m> for fixed <m>k, \rho_{p}\rightarrow 0.</m> 
              </p> 
              <p>
                Hence the remainder, the deviation of the approximation from <m>(\pi-x)/2</m> 
                at <m>x_{k}</m> which approaches the point of the discontinuity 
                at <m>x=0</m>(end point), tends to the limit 	
                <men xml:id="eqn-gibbs7">
                  \displaystyle{\lim_{p \to \infty}} R_{p}(x_{k}) \rightarrow \frac{\pi}{2}-\int\limits_{0}^{\pi_{k}}\frac{\sin u}{u}\, du
                </men>
                  For <m>k=1</m>, we find that 
                  <me>
                     \displaystyle{\lim_{p \to \infty}} R_{p}(x_{1}) \rightarrow \frac{\pi}{2}-\int\limits_{0}^{\pi}\frac{\sin u}{u}\, du 
                  </me>
                  
                  <men xml:id="eqn-gibbs8">
                   = \frac{\pi}{2}-\frac{\pi}{2}(1.179) = -0.281
                  </men>
                     Hence the negative sign in equation <xref ref="eqn-gibbs8"/> indicates that the 
                     approximate curve for <m>f(x)</m> is overshooted by about m<m>18 \% </m> 
                     at a jump discontinuity (i.e., at <m>x=0</m>), in the Fourier series. 		
                </p>
</subsection>
  </section>

