<?xml version="1.0" encoding="UTF-8"?>

<section xml:id="sec_sixth-Ltrans" xmlns:xi="http://www.w3.org/2001/XInclude">
  <title>Laplace Transforms</title>
  <introduction>
   <p> <idx>Laplace transform</idx>
    The Laplace transform is used to solve differential equations and analyze systems 
    in the field of mathematics and engineering. It transforms a function of time, 
    typically denoted as <m>f(t)</m>, into a function of a complex variable, 
    usually denoted as m<m> F(s)</m>, where 's' is the complex variable. 
    The Laplace transform provides a way to analyze functions in the frequency 
    domain rather than the time domain. Laplace transform helps us in solving the 
    differential equations with boundary values without finding the general 
    solution and the values of the arbitrary constants. It converts differential 
    equation (partial differential equation, PDE or ordinary differential equation, ODE) 
    into algebric equation and hence easy to solve. It transforms a function with 
    continuous time domain to Laplace domain (called s-parameter). 
    Let <m>f(t)</m> be the function defined for all <m>+ ve</m> values of <m>t</m>, 
    then Laplace Transform of <m>f(t)</m>  is denoted as  
<me>
  \mathscr{L}\{f(t)\} = F(s) = \int\limits_{0}^{\infty}e^{-st}f(t)\,dt.
</me>
    </p>
   
      <paragraphs>
    <title>Some useful formulae:</title>
  <p>
    <idx><h>formulae for Laplace's trasnform</h></idx> 
      
      <ol>
        <li>
          <me>
             \mathscr{L}\{1\} = \frac{1}{s}
          </me>
          <proof>
              Since 
              <me>
                \mathscr{L}\{f(t)\} = \int\limits_{0}^{\infty}e^{-st}f(t)\,dt. 
              </me>
              <me>
                \therefore  \mathscr{L}(1) = \int\limits_{0}^{\infty}e^{-st}.1\,dt = \left.\frac{e^{-st}}{-s}\right\vert_{0}^{\infty}  
              </me>
              <me>
                =0+\frac{1}{s}=\frac{1}{s}.
              </me>
          </proof>
        </li>
        <li>
          <me>
            \mathscr{L}\{t^{n}\}=\frac{n!}{s^{n+1}} \quad \text{where}\quad  n=0,1,2,\cdots
          </me>
          <proof>
            <me>
              \mathscr{L}(t^{n})= \int\limits_{0}^{\infty}e^{-st} t^{n}\,dt 
            </me>
            put <m>st=x</m> so that <m>\,dt = \frac{\,dx}{s}</m>. 
            <me>
               \therefore \mathscr{L}(t^{n})= \int\limits_{0}^{\infty}e^{-x} \left(\frac{x}{s}\right)^{n}\frac{\,dx}{s} 
            </me>
            <me>
              = \frac{1}{s^{n+1}}\int\limits_{0}^{\infty}e^{-x} x^{n}\,dx=\frac{n!}{s^{n+1}}
            </me>
          </proof>
          </li>
          <li>
            <me>
              \mathscr{L}\{e^{at}\}=\frac{1}{s-a};  \quad  (s \gt a)
            </me>
            <proof>
              <me>
                \mathscr{L}(e^{at})=\int\limits_{0}^{\infty}e^{-st}e^{at}\,dt= \int\limits_{0}^{\infty}e^{-(s-a)t}\,dt
              </me>
              <me>
                = \left.\frac{e^{-(s-a)t}}{-(s-a)}\right\vert_{0}^{\infty}=\frac{1}{s-a}.
              </me>
            </proof>
            </li>
<li>
  <me>
    \mathscr{L}\{\cosh at\} = \frac{s}{s^{2}-a^{2}};  \quad  (s^{2} \gt a^{2})
  </me>
  <proof>
   <me>
    \mathscr{L}(\cosh at) =L\left[\frac{e^{at}+e^{-at}}{2}\right]= \frac{1}{2}\left[L(e^{at}) +L(e^{-at})\right] 
   </me>
   <me>
    =\frac{1}{2}\left[\frac{1}{s-a}+\frac{1}{s+a}\right] = \frac{s}{s^{2}-a^{2}}.
   </me>
  </proof>
  </li>
  <li><me>
    \mathscr{L}\{\sinh at\} = \frac{a}{s^{2}-a^{2}};  \quad  (s^{2} \gt a^{2})
  </me>
  <proof>
   <me>
    \mathscr{L}(\sinh at)=L\left[\frac{e^{at}-e^{-at}}{2}\right] =\frac{1}{2}\left[L(e^{at}) - L(e^{-at})\right]
   </me>
   <me>
    = \frac{1}{2}\left[\frac{1}{s-a}-\frac{1}{s+a}\right]= \frac{a}{s^{2}-a^{2}}.
   </me>
  </proof>
  </li>
  <li><me>
    \mathscr{L}\{\sin at\} = \frac{a}{s^{2}+a^{2}};  \quad  (s \gt 0)
  </me>
  <proof>
    <me>
      \mathscr{L}(\sin at) =L\left[\frac{e^{iat}-e^{-iat}}{2i}\right] =\frac{1}{2i}\left[L(e^{iat}) - L(e^{-iat})\right] 
    </me>
    <me>
      = \frac{1}{2i}\left[\frac{1}{s-ia}-\frac{1}{s+ia}\right] = \frac{a}{s^{2}+a^{2}}.
    </me>
  </proof>
  </li>
  <li><me>
    \mathscr{L}\{\cos at\} = \frac{s}{s^{2}+a^{2}};  \quad  (s \gt 0)
  </me>
  <proof>
    <me>
      \mathscr{L}(\cos at) =L\left[\frac{e^{iat}+e^{-iat}}{2}\right]=\frac{1}{2}\left[\frac{1}{s-ia}+\frac{1}{s+ia}\right]
    </me>
    <me>
       = \frac{s}{s^{2}+a^{2}}.
    </me>
  </proof>
  </li>
  
  <li>
    <em>(Refer to  <xref ref="subsubsec-Ishift"/> First-shifting property)</em> 
   <me>
    \mathscr{L}\{e^{at}t^{n}\}= \frac{n!}{(s-a)^{n+1}}   \quad  \left[\because L(t^{n}) = \frac{n!}{s^{n+1}}\right]
   </me>
  </li>
  <li><me>
    \mathscr{L}\left\{e^{at}\cosh bt\right\} = \frac{s-a}{(s-a)^{2}-b^{2}}
  </me>
  </li>
  <li><me>
    \mathscr{L}\left\{e^{at}\sinh bt\right\} = \frac{b}{(s-a)^{2}-b^{2}}
  </me>
  </li>
  <li><me>
    \mathscr{L}\left\{e^{at}\sin bt\right\} = \frac{b}{(s-a)^{2}+b^{2}}
  </me>
  </li>
  <li><me>
    \mathscr{L}\left\{e^{at}\cos bt\right\} = \frac{s-a}{(s-a)^{2}+b^{2}}
  </me>
  </li>
  <li> <em>(Refer to <xref ref="subsubsec-Inv_LapTrans"/> Inverse Laplace Transforms)</em>
    <me>
    \mathscr{L}^{-1}\left\{\frac{1}{s}\right\}=1
  </me>
  </li>
  <li><me>
    \mathscr{L}^{-1}\left\{\frac{1}{s^{n}}\right\}=\frac{t^{n-1}}{!(n-1)};\quad\text{here}\quad n=0,1,2,3,\cdots
  </me>
  </li>
  <li><me>
    \mathscr{L}^{-1}\left\{\frac{1}{s-a}\right\} =e^{at}
  </me>
  </li>
  <li><me>
    \mathscr{L}^{-1}\left\{\frac{s}{s^{2}-a^{2}}\right\} =\cosh at 
  </me>
  </li>
  <li><me>
    \mathscr{L}^{-1}\left\{\frac{1}{s^{2}-a^{2}}\right\} =\frac{1}{a}\sinh at
  </me>
  </li>
  <li><me>
    \mathscr{L}^{-1}\left\{\frac{1}{s^{2}+a^{2}}\right\} =\frac{1}{a}\sin at
  </me>
  </li>
  <li><me>
    \mathscr{L}^{-1}\left\{\frac{s}{s^{2}+a^{2}}\right\} =\cos at
  </me>
  </li>
  <li><me>
    \mathscr{L}^{-1}\left\{\frac{1}{(s-a)^{2}+b^{2}}\right\} =\frac{1}{b}e^{at}\sin bt
  </me>
  </li>
  <li><me>
    \mathscr{L}^{-1}\left\{\frac{s-a}{(s-a)^{2}+b^{2}}\right\} =e^{at}\cos bt
  </me>
  </li>
  <li><me>
    \mathscr{L}^{-1}\left\{\frac{1}{(s-a)^{2}-b^{2}}\right\} =\frac{1}{b}e^{at}\sinh bt
  </me>
  </li>
  <li><me>
     \mathscr{L}^{-1}\left\{\frac{s-a}{(s-a)^{2}-b^{2}}\right\} =e^{at}\cosh bt 
  </me>
  </li>
  <li><me>
    \mathscr{L}^{-1}\left\{\frac{1}{(s^{2}+a^{2})^{2}}\right\} =\frac{1}{2a^{3}}(\sin at-at\cos at)
  </me>
  </li>
  <li><me>
    \mathscr{L}^{-1}\left\{\frac{s}{(s^{2}+a^{2})^{2}}\right\} =\frac{1}{2a} t\sin at
  </me>
  </li>
  <li><me>
    \mathscr{L}^{-1}\left\{\frac{s^{2}-a^{2}}{(s^{2}+a^{2})^{2}}\right\} = t\cos at
  </me>
  </li>
      </ol>
    </p>
   </paragraphs>
     </introduction>
 
 <subsection xml:id="subsec-Prop_LapTrans">
  <title>Properties of Laplace Transforms</title>
  <introduction>
    <p>
      The Laplace transform has several properties that make it a powerful tool 
      for solving differential equations and studying linear time-invariant systems. 
      Some of the key properties include: 
      <ol marker="i.">
        <li>
          Linearity: <m>\mathscr{L}\{af(t) + bg(t)\} = aF(s) + bG(s)</m>, where 'a' and 'b' are constants.
        </li>
        <li>Shifting: <m>\mathscr{L}\{f(t - a)\} = e^(-as) * F(s)</m>, which represents a time shift of 'a' units.</li>
          <li>Differentiation: <m>\mathscr{L}\{f'(t)\} = sF(s) - f(0)</m>, where f'(t) represents the derivative of f(t).</li>
            <li>Integration: <m>\mathscr{L}\{ \int^{t}_{0} f(\tau) \,d\tau \} = 1/s * F(s)</m>, where the integral represents the 
            indefinite integral of f(t) with respect to t.</li>
            <li>Convolution: <m>\mathscr{L}{f(t) * g(t)} = F(s) * G(s)</m>, where * denotes convolution.</li>
      </ol>
    </p>
  </introduction>

  <subsubsection xml:id="subsubsec-Lap_linear">
    <title>Linear Property</title>
    <p>
      <me>
         \mathscr{L}\{af_{1}(t)+bf_{2}(t)\} =a \mathscr{L}\{f_{1}(t)\} + b \mathscr{L}\{f_{2}(t)\}
      </me>
      <proof>
        <me>
           \mathscr{L}\{af_{1}(t)+bf_{2}(t)\} = \int\limits_{0}^{\infty}e^{-st}\left[af_{1}(t)+bf_{2}(t)\right]
        </me>
        <me>
           =a\int\limits_{0}^{\infty}e^{-st}f_{1}(t)\,dt+b\int\limits_{0}^{\infty}e^{-st}f_{2}(t)\,dt
        </me>
        <me>
           =a \mathscr{L}\{f_{1}(t)\} + b \mathscr{L}\{f_{2}(t)\}
        </me>
      </proof>
      </p>
  </subsubsection>

<subsubsection xml:id="subsubsec-Ishift">
  <title>First-Shifting Property</title>
  <p>
     If <m>\mathscr{L}\{af(t)\}=F(s),</m> then <m>\mathscr{L}\{e^{at}f(t)\} = F(s-a)</m>.
     <proof>
     <me>
      \mathscr{L}\{e^{at}f(t)\} = \int\limits_{0}^{\infty}e^{-st}e^{at}f(t)\,dt 
     </me>
     <me>
      = \int\limits_{0}^{\infty}e^{-(s-a)t}f(t)\,dt =\int\limits_{0}^{\infty}e^{-rt}f(t)\,dt  =F(r) = F(s-a) 
     </me>
     [<m>\because s-a =r </m>]
     </proof>
    </p>
</subsubsection>

<subsubsection xml:id="subsubsec-Inv_LapTrans">
  <title>Inverse Laplace Transforms</title>
  <p>
    If <m>\mathscr{L}[f(t)] =F(s)</m>  then <m>f(t)</m> is called the inverse 
    Laplace Transform of <m>F(s)</m> and we write <m>f(t) = \mathscr{L}^{-1}F(s)</m>. 
    Here <m>\mathscr{L}^{-1}</m> is called the inverse Laplace Transform operator.
    </p>
</subsubsection>
 </subsection>

<subsection xml:id="subsec-derv_LT">
  <title>Laplace Transform of the Derivative of <m>f(t)</m></title>
  <introduction>
    <p>
    If <m>\mathscr{L}[f(t)] =F(s)</m>  then <me>
      \mathscr{L}[f'(t)] = sL[f(t)]-f(0)
    </me>
     </p>
   <proof>
    <p>
      we have 
      <me>
        \mathscr{L}[f'(t)]=\int\limits_{0}^{\infty}e^{-st}f'(t)\,dt 
      </me>
      <me>
        = \left.e^{-st}f(t)\right\vert_{0}^{\infty}-\int\limits_{0}^{\infty}-se^{-st}f(t)\,dt 
      </me>
      <me>
        =0-f(0)+s\int\limits_{0}^{\infty}e^{-st}f(t)\,dt = sL[f(t)]-f(0) 
      </me>
    </p>
   </proof>
  </introduction>

  <subsubsection xml:id="subsubsec-nderv_LT">
    <title>Laplace Transform of Derivative of order <m>n</m></title>
    <p>
      <me>
        \mathscr{L}[f^{n}(t)] =s^{n}\mathscr{L}[f(t)]-s^{n-1}f(0)-s^{n-2}f' (0)-s^{n-3}f''(0) -\cdots-f^{n-1}(0).
      </me>
      </p>
      <proof>
        <p>
          we have, 
          <men xml:id="eqn-nderv_LT1">
            L[f'(t)]=sL[f(t)]-f(0)
          </men>
          replacing <m>f(t)</m> by <m>f'(t)</m> and <m>f'(t)</m> by <m>f''(t)</m> in 
          equation <xref ref="eqn-nderv_LT1"/>, we get -
          <me>
            L[f''(t)]=sL[f'(t)]-f'(0) = s\{sL[f(t)]-f(0)\}-f'(0) 
          </me>
          <me>
            =s^{2}L[f(t)]-sf(0)-f'(0)
          </me>
  Similarly, <me>
    L[f'''(t)]=s^{3}L[f(t)]-s^{2}f(0)-sf'(0)-f''(0)
  </me>
  <me>
    \therefore  L[f^{n}(t)] =s^{n}L[f(t)]-s^{n-1}f(0)-s^{n-2}f' (0)-s^{n-3}f''(0) -\cdots-f^{n-1}(0).
  </me>
        </p>
      </proof>
  </subsubsection>

<subsubsection xml:id="subsubsec-Int_LT">
  <title>Laplace Transform of Integral of <m>f(t)</m></title>
  <p>
      If <m>\mathscr{L}[f(t)] =F(s)</m>, then 
      <me>
        \mathscr{L}\left[\int\limits_{0}^{t}f(t)\,dt\right]=\frac{1}{s}F(s).
      </me>
    </p>
    <proof>
      <p> Let 
      <me>
        \phi (t) = \int\limits_{0}^{t}f(t)\,dt 
      </me>
      then <me>
        \phi' (t) = \frac{\,d}{\,dt}\left[\int\limits_{0}^{t}f(t)\,dt\right] =f(t) 
      </me>
      and 
       <me>
        \phi (0) =  \int\limits_{0}^{0}f(t)\,dt=0
       </me>
       Now 
       <me>
        \mathscr{L}[\phi' (t)]=s\mathscr{L}[\phi (t)]-\phi (0)=s\mathscr{L}[\phi (t)]
       </me>
 or,
 <me>
  \mathscr{L}[\phi (t)]=\frac{1}{s}\mathscr{L}[\phi' (t)]
 </me>
 or,
 <me>
  \mathscr{L}\left[\int\limits_{0}^{t}f(t)\,dt\right] = \frac{1}{s}\mathscr{L}[f(t)]=\frac{1}{s}F(s)
 </me>
      </p>
    </proof>
</subsubsection>
</subsection>

<subsection xml:id="subsec-Prod_LT">
  <title>Laplace Transform of <m>t^{n}f(t)</m></title>
  <p>
    If <m>\mathscr{L}[f(t)] =F(s)</m>, then <me>
      \mathscr{L}\left[t^{n}f(t)\right]=(-1)^{n}\frac{d^{n}}{\,ds^{n}}[F(s)]=(-1)F^{n}(s)
    </me>
    </p>
    <proof>
      <p>
        <men xml:id="eqn-Prod_LT1">
          \mathscr{L}[f(t)] =F(s)=\int\limits_{0}^{\infty}e^{-st}f(t)\,dt
        </men>
        Differentiating equation <xref ref="eqn-Prod_LT1"/>, w. r. t. 's', we get -
        <me>
          \frac{d}{\,ds}[F(s)] = \frac{d}{\,ds}\left[\int\limits_{0}^{\infty}e^{-st}f(t)\,dt\right]  	= \int\limits_{0}^{\infty}\frac{d}{\,ds}(e^{-st})f(t)\,dt 
        </me>
        <me>
          = \int\limits_{0}^{\infty}(-t e^{-st})f(t)\,dt  =\int\limits_{0}^{\infty}e^{-st}[-tf(t)]\,dt = L[-t f(t)]
        </me>
        or,
        <me>
          L[tf(t)] = (-1)^{1}\frac{d}{\,ds}F(s)
        </me>
        Similarly,
        <me>
          L[t^{2} f(t)] = (-1)^{2}\frac{d^{2}}{\,ds^{2}}F(s)
        </me>
        or,
        <me>
          L[t^{3} f(t)] = (-1)^{3}\frac{d^{3}}{\,ds^{3}}[F(s)]
        </me>
        <me>
          \vdots
        </me>
        <me>
          \mathscr{L}[t^{n} f(t)] = (-1)^{n}\frac{d^{n}}{\,ds^{n}}[F(s)]
        </me>
      </p>
    </proof>
</subsection>

<subsection xml:id="subsec-scale_LT">
  <title>The Change of Scale Property</title>
  <p>
    If <m>\mathscr{L}[f(t)] =F(s),</m>  then <me>
      \mathscr{L}[f(at)] =\frac{1}{a}F\left(\frac{s}{a}\right)
    </me>
    </p>
    <proof>
      <p>
        We have,
        <me>
          \mathscr{L}[f(t)] =\int\limits_{0}^{\infty}e^{-st}f(t)\,dt 
        </me>
        or,
        <me>
          \mathscr{L}[f(at)] = \int\limits_{0}^{\infty}e^{-st}f(at)\,dt 
        </me>
        put <m>at=u</m>  so that <m>\,dt=\frac{1}{a}\,du</m>.
        <me>
          \therefore \quad \mathscr{L}[f(at)]=\int\limits_{0}^{\infty}e^{-su/a}f(u)\,du 
        </me>
        where <me>p=s/a =  \frac{1}{a}F(p) =  \frac{1}{a}F(s/a)</me>.
  </p>
    </proof>
</subsection>

<subsection xml:id="subsec-frac_LT">
  <title>Laplace Transform of <m>\frac{1}{t}f(t)</m></title>
  <p>
    If  <m>\mathscr{L}[f(t)] =F(s)</m>, then <me>
      \mathscr{L}\left[\frac{1}{t}f(t)\right] =\int\limits_{s}^{\infty}F(s)\,ds.
    </me>
     </p>
     <proof>
      <p>
       <men xml:id="eqn-frac_LT1">
          \mathscr{L}[f(t)] =F(s) = \int\limits_{0}^{\infty}e^{-st}f(t)\,dt
       </men>
Integrating equation <xref ref="eqn-frac_LT1"/> w.r.t. 's', we get -
<me>
  \int\limits_{s}^{\infty}F(s)\,ds  = \int\limits_{s}^{\infty}\left[\int\limits_{0}^{\infty}  e^{-st}f(t)\,dt\right]\,ds 
</me>
<me>
  = \int\limits_{0}^{\infty} \left[\int\limits_{s}^{\infty} e^{-st}f(t)\,dt\right]\,ds   = \int\limits_{0}^{\infty}\left[\frac{ e^{-st}f(t)}{-t}\right]_{s}^{\infty} \,dt 
</me>

<me>
  =\int\limits_{0}^{\infty}\frac{f(t)}{-t}\left[e^{-st}\right]_{s}^{\infty}\,dt  = \int\limits_{0}^{\infty}\frac{f(t)}{-t}\left[0-e^{-st}\right]\,dt 
</me>
<me>
 = \int\limits_{0}^{\infty}e^{-st}\{\frac{1}{t}f(t)\}\,dt   = L\left[\frac{1}{t}f(t)\right]
</me>
i.e.,
<me>
  \mathscr{L}\left[\frac{1}{t}f(t)\right] = 	\int\limits_{s}^{\infty}F(s)\,ds
</me>
      </p>
     </proof>
</subsection>
  </section>

