<?xml version="1.0" encoding="UTF-8"?>

<section xml:id="sec_fourth-examplesF" xmlns:xi="http://www.w3.org/2001/XInclude">
  <title>Examples F</title>
 

<paragraphs>
  <title>Laguerre's Function</title>
  <example>
    <statement>
      <p>
         Prove that <me>
          L_{n}(0)=n! 
         </me>
      </p>
    </statement>
    <solution>
      <p>
       We have 
       <me>
        \sum\limits_{n=0}^{\infty}\frac{L_{n}(x)}{n!}t^{n}=\frac{1}{1-t}e^{-xt/(1-t)}
       </me>
       putting <m>x=0</m>, we get -
       <me>
        \sum\limits_{n=0}^{\infty}\frac{L_{n}(0)}{n!}t^{n}=\frac{1}{1-t}=(1-t)^{-1} = 1+t+t^{2}+\cdots+t^{n}+\cdots = \sum\limits_{n=0}^{\infty}t^{n}
       </me>
       <me>
        \therefore L_{n}(0) = n! 
       </me>
      </p>
    </solution>
  </example>

  <example>
    <statement>
      <p>
        Prove that 
        <me>
          xL''_{n}(x) +(1-x)L'_{n}(x)+nL_{n}(x)=0
        </me>
        and hence deduce that <m>L'_{n}(0) =-n(n!)</m>.
      </p>
    </statement>
    <solution>
      <p>
        Since <m> L_{n}(x)</m> satisfies the Laguerre's equation, 
        <m>xy''+(1-x)y'+ny =0</m>  [for <m>\lambda =n</m>]. 
        <me>
          \therefore, \quad	xL''_{n}(x) +(1-x)L'_{n}(x)+nL_{n}(x)=0 
        </me>
          putting <m>x=0</m>, we have <m>L'_{n}(0)=-n L_{n}(0)</m>
          <me>
             \therefore L'_{n}(0) =-n(n!).
          </me>
      </p>
    </solution>
  </example>

  <example>
    <statement>
      <p>
         Evaluate	
         <me>
          \int\limits_{0}^{\infty}e^{-x}[L_{n}(x)]^{2}\,dx.
         </me>
      </p>
    </statement>
    <solution>
      <p>
       We may have	
       <me>
        \int\limits_{0}^{\infty}e^{-x}\sum\limits_{m,n =0}^{\infty}L_{m}(x)L_{n}(x)\frac{s^{m}t^{n}}{m!n!}\,dx
       </me>
       <me>
        =(1-s)^{-1}(1-t)^{-1}\int\limits_{0}^{\infty}exp\left[-x\frac{(1-st)}{(1-s)(1-t)}\right]\,dx
       </me>
       <me>
        =(1-st)^{-1}=\sum\limits_{n}(st)^{n}  \hspace{1cm} \left[\because \int\limits_{0}^{\infty}e^{-\alpha x}\,dx=\frac{1}{\alpha}\right]
       </me> 
        put <m>m=n</m> and equate the coefficients of <m>(st)^{n}</m> on both sides, we get -
        <me>
          \int\limits_{0}^{\infty}e^{-x}[L_{n}(x)]^{2}\,dx =(n!)^{2}.
        </me>			
      </p>
      <p>
        <term>Alternative:</term>
        In case of <m>r=n</m> in eqn. <xref ref="eqn-laguer_eq8"/>, we have	
        <me>
          L_{n}(x) =(-1)^{n}x^{n} 
        </me>
        	<me>
             \therefore \int\limits_{0}^{\infty}e^{-x}[L_{n}(x)]^{2}\,dx =(-1)^{n}\int\limits_{0}^{\infty}e^{-x}x^{n}L_{n}(x)\,dx 
          </me>
          <me>
            =(-1)^{n}\int\limits_{0}^{\infty}e^{-x}x^{n}e^{x}\frac{d^{n}}{dx^{n}}(x^{n}e^{-x})\,dx
          </me>
          
          <me>
             =(-1)^{n}\int\limits_{0}^{\infty}x^{n}\frac{d^{n}}{dx^{n}}(x^{n}e^{-x})\,dx
          </me>
              Integrating by parts <m>n</m> times, 
              <me>
                =(-1)^{n}n!\int\limits_{0}^{\infty}\frac{d^{n-m}}{dx^{n-m}}(x^{n}e^{-x})\,dx = (-1)^{n}n!\int\limits_{0}^{\infty}x^{n}e^{-x}\,dx=(n!)^{2}.
              </me>
        </p>
    </solution>
  </example>

  <example>
    <statement>
      <p>
        Show that
        <me>
          L_{2n}(x) = n!\sum\limits_{m=0}^{n}\frac{2^{n-m}(-1)^{m}}{m!(n-m)!}L_{n-m}(x), \hspace{1cm} n \gt m.
        </me>
      </p>
    </statement>
    <solution>
      <p>
        We have	
        <me>
          L_{n}(x)=\frac{1}{n!}e^{x}\frac{d^{n}}{dx^{n}}(x^{n}e^{-x})
        </me>
        Therefore
        <me>
          L_{o}(x)=1, \hspace{1cm} L_{1}(x)=\frac{1}{1!}(1-x) =1-x.
        </me>
          Replacing <m>x</m> by <m>2x</m>, we get - 
          <me>
            L_{1}(2x)=1-2x =2(1-x)-1=2L_{1}(x)-2\frac{1}{1!}L_{o}(x) 
          </me>
          <me>
            = 1!\sum\limits_{m=0}^{1}\frac{2^{1-m}(-1)^{m}}{m!(1-m)!}L_{1-m}(x)
          </me>
          
          Also,
          	<me>
              L_{2}(2x)=\frac{1}{2!}(2-8x+4x^{2}) = 1-4x+2x^{2}
            </me>
            <me>
              =4(1-2x+\frac{x^{2}}{2})-4(1-x)+1
            </me>
            
            	<me>
                =2^{2}L_{2}(x)-2\frac{2!}{1!1!}L_{1}(x)+\frac{2!}{0!2!}L_{o}(x)
              </me>
              <me>
                =2!\sum\limits_{m=0}^{2}\frac{2^{2-m}(-1)^{m}}{m!(2-m)!}L_{2-m}(x)
              </me>
              
              similarly,
              <me>
                L_{3}(2x)=3!\sum\limits_{m=0}^{3}\frac{2^{3-m}(-1)^{m}}{m!(3-m)!}L_{3-m}(x)
              </me>
              and in general,
              <me>
                L_{n}(2x)=3!\sum\limits_{m=0}^{n}\frac{2^{n-m}(-1)^{m}}{m!(n-m)!}L_{n-m}(x) 
              </me>
      </p>
    </solution>
  </example>

  <example>
    <statement>
      <p>
        Show that	if 
        <me>
          \int\limits_{0}^{\infty}e^{-x}x^{m}L_{n}(x)\,dx =0 \quad \text{if} \quad n \gt m. 
        </me>
      </p>
    </statement>
    <solution>
      <p>
       <me>
        \int\limits_{0}^{\infty}e^{-x}x^{m}L_{n}(x)\,dx= \int\limits_{0}^{\infty}x^{m}e^{-x}e^{x}\frac{d^{n}}{dx^{n}}(x^{n}e^{-x})\,dx 
       </me>
       Rodrigue's formula for <m>L_{n}(x)</m> is 
       <me>
        e^{x}\frac{d^{n}}{dx^{n}}(x^{n}e^{-x})  =\int\limits_{0}^{\infty}x^{m}\frac{d^{n}}{dx^{n}}(x^{n}e^{-x})\,dx
       </me>
      
       <me>
        =\left.x^{m}\frac{d^{n-1}}{dx^{n-1}}(x^{n}e^{-x})\right\vert_{0}^{\infty}-\int\limits_{0}^{\infty}mx^{m-1}\frac{d^{n-1}}{dx^{n-1}}(x^{n}e^{-x})\,dx
       </me>
       
       <me>
         =0+(-1)m\int\limits_{0}^{\infty}x^{m-1}\frac{d^{n-1}}{dx^{n-1}}(x^{n}e^{-x})\,dx
       </me>
       <me>
        =(-1)^{2}m(m-1)\int\limits_{0}^{\infty}x^{m-2}\frac{d^{n-2}}{dx^{n-2}}(x^{n}e^{-x})\,dx
       </me>
       <me>
        =(-1)^{m}m!\int\limits_{0}^{\infty}\frac{d^{n-m}}{dx^{n-m}}(x^{n}e^{-x})\,dx =0. \quad if \quad  n \gt m.
       </me>	 
      </p>
    </solution>
  </example>
</paragraphs>
   
</section>
