<?xml version="1.0" encoding="UTF-8"?>

<section xml:id="sec_fourth-power" xmlns:xi="http://www.w3.org/2001/XInclude">
  <title>Power Series Method</title>
  <introduction>
  <p>
    It is a method to find the solution of homogeneous linear differential equation of second order 
    in the form of series. We know that the solution of differential equations
     </p>
    <ol>
      <li>
        <p>
          <me>
            y''-y=0 
          </me>
          <me>
            C_{1}e^{x}+C_{2}e^{-x}
          </me>
          where,
          <me>
           e^{x}=1+\frac{x}{1!}+ \frac{x^{2}}{2!}+\frac{x^{3}}{3!}+\cdots 
          </me>
          and 
          <me>
             e^{-x}= 1-\frac{x}{1!}+ \frac{x^{2}}{2!}-\frac{x^{3}}{3!}+\cdots 
          </me>
          <me>
            \therefore y = C_{1}\left\{1+\frac{x}{1!}+ \frac{x^{2}}{2!}+\frac{x^{3}}{3!}+\cdots \right\}
          </me>
          <me>
            +C_{2}\left\{1-\frac{x}{1!}+ \frac{x^{2}}{2!}-\frac{x^{3}}{3!}+\cdots \right\}
          </me>
          
          It is a power series solution of the given differential equation.
        </p>
      </li>
      <li>
        <p>
          If <m>y''+y=0</m> then <m>y=A\cos x+B\sin x </m> is the solution of a given equation. 
          where,  
          <me>
            \cos x= 1-\frac{x^{2}}{2!}+\frac{x^{4}}{4!}-\frac{x^{6}}{6!}+\cdots
          </me>
          and 
          <me>
             \sin x=x-\frac{x^{3}}{3!}+\frac{x^{5}}{5!}-\frac{x^{7}}{7!}+\cdots
          </me>
          <me>
            \therefore y = A\left\{1-\frac{x^{2}}{2!}+\frac{x^{4}}{4!}-\frac{x^{6}}{6!}+\cdots  \right\}
          </me> 
          <me>
            +B\left\{x-\frac{x^{3}}{3!}+\frac{x^{5}}{5!}-\frac{x^{7}}{7!}+\cdots \right\}
          </me>
          
          is the power series solution of the given equation.
        </p>
        </li>
    </ol>
   <p>
    Let us consider the second order homogeneous linear differential equation 
    <me>
      f_{o}(x)\frac{\,d^{2}y}{\,dx^{2}}+f_{1}(x)\frac{\,dy}{\,dx}+f_{2}(x)y=0
    </me>
    <men xml:id="eqn-powers1">
      \frac{\,d^{2}y}{\,dx^{2}}+q_{1}(x)\frac{\,dy}{\,dx}+q_{2}(x)y=0
    </men>
    where,
    <me>
       q_{1}(x)=\frac{f_{1}(x)}{f_{o}(x)}, \quad \text{and} \quad q_{2}(x)=\frac{f_{2}(x)}{f_{o}(x)}.
    </me>
    and suppose it has no solution expressible as a finite linear combination of elementary function. 
    <term>Algebric, trigonomertric, logerithmic, and exponential functions are elementary functions</term>. 
    Then, we can find that it has a solution which can be expressable in the form of infinite series. 
    Let us assume such a solution of equation <xref ref="eqn-powers1"/> is 
    <men xml:id="eqn-powers2">
      y=\sum\limits_{\lambda =0}^{\infty}a_{\lambda}x^{\lambda}
    </men>
    is called a power series in <m>x</m>. Where <m>a_{o}{,}a_{1}{,}a_{2}{,} \cdots</m> are constants. 
    In the expression <xref ref="eqn-powers2"/> at least one <m>a's</m> is not zero. 
    But in case when <m>a_{o}=a_{1}=a_{2}= \cdots =0</m> then there is no series satisfying the 
    given differential equation. Hence the power series solution method is not valid 
    for such an equation. Some important terms are defining here helps us in establishing 
    the validity of series solution method.
    </p>

      <ol>
        <li>
          <p>
             <term> Ordinary Point:</term> <m>x=0</m> (or origin) is called an ordinary point 
          of the differential equation <xref ref="eqn-powers1"/> if <m>q_{1}(x)</m> and 
          <m>q_{2}(x)</m> are finite or regular at <m> x=0</m> and these can be expressed 
          as power series given by 
          <me>
            f(x) = \sum\limits_{k =0}^{\infty}a_{k}x^{k}.
          </me>
          e.g., in
          <me>
            y'' -\frac{2x}{1-x^{2}}y'+\frac{2}{1-x^{2}}y =0
          </me>
          where 
          <me>
            q_{1}(x)=-\frac{2x}{1-x^{2}}=-2x(1-x^{2})^{-1}=-2x(1+x^{2}+x^{4}+\cdots)
          </me>
          and 
          <me>
            q_{2}(x)=\frac{2}{1-x^{2}}=2(1-x^{2})^{-1} =2(1+x^{2}+x^{4}+\cdots)
          </me>
          and are finite at <m>x=0</m>.	
          </p>
         
          <p>
            Thus <m>x=0</m> is an ordinary point of the given diffn. eqn. 
            We assume the solution of this equation as 
            <me>
              y = \sum\limits_{\lambda =0}^{\infty}a_{\lambda}x^{\lambda}.
            </me>
          </p>
        </li>
        <li>
          <p>
            <term>Singular Point:</term>
            When <m>q_{1}(x)</m> and <m>q_{2}(x)</m> are not finite at <m>x=0 </m>, then <m>x=0</m> 
            is called a singular point of the diffn. eqn. If <m>xq_{1}(x)</m> and <m>x^{2}q_{2}(x)</m> 
            tend to finite values at <m>x=0</m> then the equation has a regular singularity at the origin. 
            But if <m>xq_{1}(x)</m> and <m>x^{2}q_{2}(x)</m>  one or both not finite at <m>x=0</m> then 
            <m>x=0</m> is called an irregular singular points. For example in an equation 
            <me>
              y''-\frac{x}{2x^{2}}y' +\frac{(x^{2}+1)}{2x^{2}}y =0
            </me>
             has rugular singularity at <m>x=0</m> and 
             <me>
              y''+\frac{4}{x}y' +\frac{5}{x^{3}}y=0
             </me>
                has a singularity at <m>x=0</m> but not regular, i.e., it has an irregular singularity 
                at <m>x=0</m>. Hence such type of equation has no series solution because on solving 
                such equation we find all the constants <m> a_{o}{,}a_{1}{,}a_{2}{,}\cdots</m> are zero.
          </p>
          <p>
            The solution of a equation having <m>x=0</m> is a singular points is assumed in the form 
            <me>
              y = \sum\limits_{\lambda =0}^{\infty}a_{\lambda}x^{\lambda+k}.
            </me>
            where <m>k</m> may be positive or negative integer or fraction. 
            Since many equations in physics fall to second category and equations under first category are 
            just the special cases of second category, we concentrate here only on second category. 
            This method of finding the solution of equation in power series is developed by 
            Frobenius and Fuchs.
          </p>
          </li>
      </ol>  
     </introduction>
 
 <subsection xml:id="subsec-reg_sing">
  <title>When <m>x=0</m> is a Regular Singular Point of the Equation</title>
  <p>
    In this case, the solution is 
    <me>
      y = \sum\limits_{\lambda =0}^{\infty}a_{\lambda}x^{\lambda+k} 
    </me>
    and on substituting of <m>y{,}y'</m> and <m>y"</m> in the given differential equation 
    we get the identity. The index <m>k</m> will be determined by the quadratic equation 
    obtained by equating the coefficient of lowest power of <m>x</m> to zero. 
    The quadratic equation in <m>k</m> is called the <term>Indicial equation</term>. 
    Thus, we will get two values of <m>k</m>. The series solution of equation <xref ref="eqn-powers1"/>
    will depend upon the nature of the roots of the indicial equation.
    </p>
    <p>
     <alert>Case I.</alert> When roots (<m> k_{1}{,}k_{2}</m>) are distinct and not differing 
     by an integer, then the complete solution is 
     <me>
      y=C_{1}(y)_{k_{1}}+C_{2}(y)_{k_{2}} 
     </me>
    <alert>Case II.</alert> When roots are equal (<m>k_{1}=k_{2}</m>), then 
    <me>
      y=C_{1}(y)_{k_{1}}+C_{2}(\frac{dy}{dk})_{k_{1}}.
    </me>
    <alert>Case III.</alert> When roots are distinct and differ by an integer, then 
    there arise two possibilities 
    <ol marker="i.">
      <li>
        If some of the coefficients of y series become infinite at <m>k=k_{2} </m>, 
        then replace <m>a_{o}</m> by <m>b_{o}(k-k_{2})</m>. The complete solution is then 
        <me>
          y=C_{1}(y)_{k_{1}}+C_{2}(\frac{dy}{dk})_{k_{2}} 
        </me>
        [on taking <m>k=k_{1}</m>, we obtain a solution which is a constant multiple of 
        that obtained for <m>k_{1}</m>.] 
      </li>
      <li>
         When the coefficient of y series does not become infinite for any <m>k</m>, 
         then the complete solution is 
         <me>
          y=C_{1}(y)_{k_{1}}+C_{2}(y)_{k_{2}} 
         </me>
        </li>
    </ol>
      </p>
 </subsection>
 


  </section>

