<?xml version="1.0" encoding="UTF-8"?>

<section xml:id="sec_sixth-examplesB" xmlns:xi="http://www.w3.org/2001/XInclude">
  <title>ExamplesB</title>
 
<example xml:id="Lap_Q1">
  <statement>
    <p>
       Find the Laplace transform of <m>(1+\cos2t)</m>.
    </p>
  </statement>
  <solution>
    <p>
      <me>
        \mathscr{L}(1+\cos2t)=\int\limits_{0}^{\infty}e^{-st}(1+\cos2t)\,dt 
      </me>
      <me>
        = \int\limits_{0}^{\infty}e^{-st}.1\,dt + \int\limits_{0}^{\infty}e^{-st}\cos at\,dt
      </me>
      
      <me>
         =\frac{1}{s}+ \frac{s}{s^{2}+2^{2}} = \frac{1}{s}+ \frac{s}{s^{2}+4}
      </me>
    </p>
  </solution>
</example>

<example>
  <statement>
    <p>
      Find the Laplace transform of <m>\cos^{2}t</m>.	
    </p>
  </statement>
  <solution>
    <p>
      <me>
        \because \quad \cos2t = 2\cos^{2}t-1; \quad  \therefore \cos^{2}t= \frac{1}{2}[\cos 2t+1]
      </me>
      Now,
      <me>
        \mathscr{L}[\cos^{2}t]= \int\limits_{0}^{\infty}e^{-st}\cos^{2}t\,dt 
      </me>
      <me>
        = \frac{1}{2}\int\limits_{0}^{\infty}e^{-st}[\cos 2t+1] =\frac{1}{2}[ \frac{1}{s}+ \frac{s}{s^{2}+4}].
      </me>
      (see problem <xref ref="Lap_Q1"/>)
    </p>
  </solution>
</example>

<example>
  <statement>
    <p>
      Find the Laplace transform of <m>t\sin at</m>.
    </p>
  </statement>
  <solution>
    <p>
      <me>
        \mathscr{L}[t\sin at] = \mathscr{L}\left[t\{\frac{e^{iat}-e^{-iat}}{2i}\}\right] =\frac{1}{2i}[\mathscr{L}(te^{iat})-\mathscr{L}(te^{-iat})]
      </me>
      <me>
        =\frac{1}{2i}\left[\frac{1}{(s-ia)^{2}}-\frac{1}{(s+ia)^{2}}\right]. 
      </me>
     (see formula 8 in <xref ref="sec_sixth-Ltrans"/>) 
      <me>
         =\frac{1}{2i}\left[\frac{s^{2}+2ias-a^{2}-s^{2}+2ias+a^{2}}{(s^{2}+a^{2})^{2}}\right]
      </me>
      <me>
         = \frac{1}{2i}\left[\frac{4ias}{(s^{2}+a^{2})^{2}}\right]= \frac{2as}{(s^{2}+a^{2})^{2}} 
      </me>  
    </p>
  </solution>
</example>
    
    <example>
      <statement>
        <p>
           Find the Laplace Transform of <m>\cos at \sinh at</m>.
        </p>
      </statement>
      <solution>
        <p>
<me>
  \mathscr{L}[\cos at \sinh at] = \mathscr{L}\left[\cos at\{\frac{e^{at}-e^{-at}}{2}\}\right]
</me>
<me>
  =\frac{1}{2}[\mathscr{L}(\cos at e^{at})-\mathscr{L}(\cos at e^{-at})]
</me>
<me>
  = \frac{1}{2}\left[\frac{s-a}{(s-a)^{2}+a^{2}}-\frac{s+a}{(s+a)^{2}+a^{2}}\right]
</me>
        </p>
      </solution>
    </example>

    <example>
      <statement>
        <p>
           Find <m>\mathscr{L}[\sin (\omega t + \theta)]</m>.   
        </p>
      </statement>
      <solution>
        <p>
          <me>
            \mathscr{L}[\sin (\omega t + \theta)] = \mathscr{L}[\sin \omega t \cos \theta +\cos \omega t \sin \theta]
          </me>
          <me>
             = \cos \theta \mathscr{L}[\sin \omega t] +\sin \theta \mathscr{L}[\cos \omega t] 
          </me>
          <me>    
 = \cos \theta \left[\frac{\omega}{s^{2}+\omega ^{2}}\right] +  \sin \theta \left[\frac{s}{s^{2}+\omega ^{2}}\right].
          </me>
        </p>
      </solution>
    </example>

    <example>
      <statement>
        <p>
           Find the inverse transform of <m>\frac{1}{s^{2}-5s+6}</m>.
        </p>
      </statement>
      <solution>
        <p>
      Let us convert the given function into partial fractions. 
      <me>
        \mathscr{L}^{-1}\left(\frac{1}{s^{2}-5s+6}\right) = \mathscr{L}^{-1}\left(\frac{1}{s-3}\right)-L^{-1}\left(\frac{1}{s-2}\right) 
      </me>
      <me>
        = e^{3t}-e^{2t}
      </me>
        </p>
      </solution>
    </example>

    <example>
      <statement>
        <p>
           Find <me>
            \mathscr{L}^{-1}\left(\frac{s-1}{s^{2}-6s+25}\right).
           </me>
        </p>
      </statement>
      <solution>
        <p>
        </p>
         <hint>
            <p>
            <me>
               \frac{s-1}{s^{2}-6s+25} = \frac{s-1}{(s-3)^{2}+4^{2}} 
            </me>
            
             <me>
              =\frac{s-3+2}{(s-3)^{2}+4^{2}} =\frac{s-3}{(s-3)^{2}+4^{2}}+\frac{1}{2} \frac{4}{(s-3)^{2}+4^{2}} 
             </me>
            </p>
          </hint>
      </solution>
    </example>

    <example>
      <statement>
        <p>
          Find <me>
            \mathscr{L}^{-1}\left(\frac{s+4}{s(s-1)(s^{2}+4)}\right).
          </me>
        </p>
      </statement>
       <hint>
          <p>
            <me>
              \frac{s+4}{s(s-1)(s^{2}+4)} =\frac{A}{s}+\frac{B}{s-1}+\frac{Cs+D}{s^{2}+4}
            </me>
            or,
            <me>
               s+4 
            </me>
            
            <men xml:id="eqn-Inv_LT1">
             = A(s-1)(s^{2}+4) +Bs(s^{2}+4) +(Cs +D) -s(s-1)
            </men> 
          </p>
        </hint>
      <solution>
        <p>
          putting, <m>s=1</m>, we get - <m>4=-4A; \quad \therefore A = -1</m>, 
          again, put <m>s=1</m>, we get -  <m>5=B.5;  \quad    \therefore B = 1</m>,   
          equating the coefficient of <m>s^{3}</m> on both sides of equation <xref ref="eqn-Inv_LT1"/>, we have, 
          <m>0=A+B+C</m>      or, 
          <me>
            0=-1+1+C; \quad    \therefore C = 0
          </me>
          equating the coefficient of <m>s</m> on both sides of equation <xref ref="eqn-Inv_LT1"/>, we get- 
          <m>1=4A+4B-D =-4+4-D</m>	 	or, <m>D=-1</m>. 
          On putting  <m>A,B,C,D</m> in equation <xref ref="eqn-Inv_LT1"/>, we get - 
          <me>
            \frac{s+4}{s(s-1)(s^{2}+4)} =-\frac{1}{s}+\frac{1}{s-1}-\frac{1}{s^{2}+4}
          </me>
        </p>
      </solution>
    </example>

    <example>
      <statement>
        <p>
           Find 
           <me>
             \mathscr{L}^{-1}\left(\frac{s^{2}}{(s^{2}+a^{2})(s^{2}+b^{2})}\right).
           </me>
        </p>
      </statement>
      <solution>
        <p> Here,
          <me>
            \left(\frac{s^{2}}{(s^{2}+a^{2})(s^{2}+b^{2})}\right) =\frac{A}{(s^{2}+a^{2})}+ \frac{B}{(s^{2}+b^{2})}
          </me>
          or,
          <me>
             s^{2}=A(s^{2}+b^{2})+B(s^{2}+a^{2}) =s^{2}(A+B)+Ab^{2}+Ba^{2}
          </me>
          now,
          <m> A+B=1  </m> and <m>Ab^{2}+Ba^{2}=0 \quad \Rightarrow Ab^{2}=-Ba^{2}</m>

 <me>
  \therefore \quad -\frac{Ba^{2}}{b^{2}}+B=1
 </me>
 or,
 <me>
  B\left(1-\frac{a^{2}}{b^{2}}\right)=1 
 </me>
 or,
 <me>
  B\left(\frac{b^{2}-a^{2}}{b2}\right)=1
 </me>
 <me>
   \therefore \quad B= \frac{b2}{b^{2}-a^{2}}
 </me>

   again,
   <me>
     Ab^{2}=-	\left(\frac{b2}{b^{2}-a^{2}}\right)a^{2}
   </me>
   or,
   <me>
     A=\frac{a2}{a^{2}-b^{2}}
   </me>
   <me>
     \therefore  \quad \frac{s^{2}}{(s^{2}+a^{2})(s^{2}+b^{2})} = \frac{a2}{a^{2}-b^{2}}\frac{1}{s^{2}+a^{2}}-\frac{b2}{a^{2}-b^{2}}\frac{1}{s^{2}+b^{2}}
   </me>
   <me>
    = \frac{1}{a^{2}-b^{2}}\left[\frac{a^{2}}{s^{2}+a^{2}}-\frac{b^{2}}{s^{2}+b^{2}}\right]
   </me>
   Hence,
   <me>
    \mathscr{L}^{-1}\left(\frac{s^{2}}{(s^{2}+a^{2})(s^{2}+b^{2})}\right)
   </me>
   <me>
    = \frac{1}{a^{2}-b^{2}}\left[a^{2}\left(\frac{1}{a}\sin at\right)-b^{2}\left(\frac{1}{b}\sin bt\right)\right]
   </me>
   
   <me>
     =\frac{1}{a^{2}-b^{2}}[a\sin at-b\sin bt]
   </me>
        </p>
      </solution>
    </example>

    <example>
      <statement>
        <p>
          Find the inverse Laplace Transform of <m>\frac{1}{s(s^{2}+1)}</m>.
        </p>
      </statement>
      <solution>
        <p>
          We have 	
          <me>
            \mathscr{L}^{-1}\left[\frac{1}{(s^{2}+1)}\right] = \sin t
          </me>
          or,
          <me>
           \mathscr{L}^{-1}\left[\frac{1}{s(s^{2}+1)}\right] = \int\limits_{0}^{t}1.\sin t\,dt 
          </me>
          or,
          <me>
            [-\cos t]_{0}^{t} = (-\cos t +1)
          </me>
          i.e., 
          <me>
            \mathscr{L}^{-1}\left[\frac{1}{s(s^{2}+1)}\right] = 1-\cos t
          </me>
        </p>
      </solution>
    </example>

    <example>
      <statement>
        <p>
          Find the inverse Laplace transform of <m>\frac{1}{s^{2}(s^{2}+a^{2})}</m>.
        </p>
      </statement>
      <solution>
        <p>
          We have <me>
            \mathscr{L}^{-1}\left[\frac{1}{(s^{2}+a^{2})}\right] = \frac{1}{a}\sin at 
          </me>
          or,
          <me>
            \mathscr{L}^{-1}\left[\frac{1}{s(s^{2}+a^{2})}\right]  =\frac{1}{a}\int\limits_{0}^{t}\sin at\,dt 
          </me>
          <me>
            = \frac{1}{a}\left[\frac{-\cos at}{a}\right]_{0}^{t}
          </me>
          <me>
            =\frac{1}{a^{2}}[1-\cos at +1] = \frac{1}{a^{2}}[1-\cos at]
          </me>
          or,
          <me>
            \mathscr{L}^{-1}\left[\frac{1}{s^{2}(s^{2}+a^{2})}\right] =  \frac{1}{a^{2}}\int\limits_{0}^{t}(1-\cos at)\,dt
          </me>
          <me>
             = \frac{1}{a^{2}}\left[\left.t\right\vert_{0}^{t}-\left(\frac{\sin at}{a}\right)_{0}^{t}\right] 
          </me>
          <me>
            =  \frac{1}{a^{2}}\left[t-\frac{1}{a}\sin at\right]
          </me>
        </p>
      </solution>
    </example>

    <example>
      <statement>
        <p>
          Find <me>
            \mathscr{L}^{-1}\left[\frac{1}{s^{2}+4s}\right]
          </me>
        </p>
      </statement>
      <hint>
          <p>
            Find 
            <me>
              \mathscr{L}^{-1}\left[\frac{1}{s(s^{2}+2^{2})}\right]
            </me>
          </p>
         </hint>
      <solution>
        <p>
          <me>
            \frac{1}{4}(1-\cos 2t)
          </me>
        </p>
      </solution>
    </example>

    <example>
      <statement>
        <p>
          Find the Laplace Transform of <m>t\sinh at</m>.  
          </p>
      </statement>
      <solution>
        <p>
          <me>
            \mathscr{L}[\sinh at] = \frac{a}{s^{2}-a^{2}} 
          </me>
          or,
          <me>
            \mathscr{L}[t\sinh at] =-\frac{d}{\,ds}\left[\frac{a}{s^{2}-a^{2}}\right]   =  \frac{2as}{(s^{2}-a^{2})^{2}}
          </me>
        </p>
      </solution>
    </example>

    <example>
      <statement>
        <p>
          Find <m>\mathscr{L}[t^{2}e^{t}\sin 4t]</m>. 
        </p>
      </statement>
      <solution>
        <p>
          <me>
            \mathscr{L}[\sin 4t] = \frac{4}{s^{2}+16}
          </me>
          or,
          <me>
            \mathscr{L}[e^{t}\sin 4t] = \frac{4}{(s-1)^{2}+16}
          </me>
          or,
          <me>
            \mathscr{L}[t^{2}e^{t}\sin 4t] =(-1)^{2}\frac{\,d^{2}}{\,ds^{2}}\left[ \frac{4}{(s-1)^{2}+16}\right]
          </me>
          <me>
            = \frac{\,d^{2}}{\,ds^{2}}\left[\frac{4}{s^{2}-2s+17}\right] 
          </me>
          <me>
            =\frac{\,d}{\,ds}\left[\frac{-4(2s-2)}{(s^{2}-2s +17)^{2}}\right]
          </me>
          <me>
            =-4\left[\frac{(s^{2}-2s +17)^{2}\{2s^{2}-4s+34-8s^{2}+16s-8\}}{(s^{2}-2s +17)^{4}}\right]  
          </me>
          <me>
             = \frac{-4\{-6s^{2}+12s+26\}}{(s^{2}-2s +17)^{3}}
          </me>
        </p>
      </solution>
    </example>

    <example>
      <statement>
        <p>
           Find the inverse Laplace Transfoem of the function, 
           <me>
            \log \left(1+\frac{\omega^{2}}{s^{2}}\right).
           </me>
        </p>
      </statement>
      <solution>
        <p>
          Let 
          <me>
            F(s)= \log (1+\frac{\omega^{2}}{s^{2}})  
          </me>
          we know that, 
          <me>
            -\frac{\,d}{\,ds}\log \left(\frac{s^{2}+\omega^{2}}{s^{2}}\right) =-\frac{\,d}{\,ds}[\log (s^{2}+\omega^{2}) -\log s^{2}]
          </me>
          <me>
            =-\left[\frac{1\cdot2s}{s^{2}+\omega^{2}}-\frac{2s}{s^{2}}\right] = \left[\frac{2}{s}-\frac{2s}{s^{2}+\omega^{2}}\right]
          </me>
          or,
          <me>
            tf(t)   =\mathscr{L}^{-1}\left[\frac{2}{s}-\frac{2s}{s^{2}+\omega^{2}}\right] = 2-2\cos \omega t
          </me>
          or,
          <me>
            f(t)=\frac{2}{t}[1-\cos \omega t] 
          </me>
        </p>
      </solution>
    </example>
    <example>
      <statement>
        <p>
           Find <m>\mathscr{L}^{-1}[\cot^{-1}(1+s)]</m>.
        </p>
      </statement>
      <solution>
        <p>
         Let <m>F(s) = \cot^{-1}(1+s)</m>
         we know that 
         <me>
          \mathscr{L}[tf(t)] =-\frac{\,d}{\,ds}F(s)=-\frac{\,d}{\,ds}\left[\cot^{-1}(1+s)\right] 
         </me>
         <me>
          = -\left[\frac{-1}{1+(1+s)^{2}}\right] = \frac{1}{(s+1)^{2}+1}
         </me>
         or,
         <me>
          tf(t) = \mathscr{L}^{-1}\left[\frac{1}{(s+1)^{2}+1}\right] =e^{-t}\sin t
         </me>
         <me>
          \therefore f(t) = \frac{1}{t}\left[e^{-t}\sin t\right].
         </me>
        </p>
      </solution>
    </example>
    <example>
      <statement>
        <p>
          Find the Laplace Transform of <m>\frac{\sin 2t}{t}</m>.
        </p>
      </statement>
      <solution>
        <p>
          <me>
            \mathscr{L}[\sin 2t] = \frac{2}{s^{2}+4} 
          </me>
          Now,
          <me>
            \mathscr{L}\left[\frac{\sin2t}{t}\right] = 	\int\limits_{s}^{\infty}\frac{2}{s^{2}+4}\,ds
          </me>
          <me>
            =2.\frac{1}{2}\left[\tan^{-1}\frac{s}{2}\right]_{s}^{\infty} = \left[\tan^{-1}\infty -\tan^{-1}\frac{s}{2}\right]
          </me>
          <me>
             = \frac{\pi}{2}-\tan^{-1}\frac{s}{2} = \cot^{-1}\frac{s}{2}.
          </me>
        </p>
      </solution>
    </example>

    <example>
      <statement>
        <p>
          Find the Laplace Transform of <m>\frac{1-\cos t}{t^{2}}</m>.
        </p>
      </statement>
      <solution>
        <p>
          <me>
             \mathscr{L}[1-\cos t] = L[1]-L[\cos t] = \frac{1}{s}-\frac{s}{s^{2}+1}
          </me>
          or,
          <me>
           \mathscr{L}\left[\frac{1-\cos t}{t}\right] = \int\limits_{s}^{\infty}\left(\frac{1}{s}-\frac{s}{s^{2}+1}\right)\,ds 
          </me>
          <me>
            = \left[\log s-\frac{1}{2}\log (s^{2}+1)\right]_{s}^{\infty}  =\frac{1}{2}\left[\log s^{2}-\log (s^{2}+1)\right]_{s}^{\infty}  
          </me>
          <me>
           =\frac{1}{2}\left[\log \frac{s^{2}}{s^{2}+1}\right]_{s}^{\infty} =\frac{1}{2}\left[\log \frac{s^{2}}{s^{2}(1+1/s^{2})}\right]_{s}^{\infty} 
          </me>
          <me>
            = \frac{1}{2}\left[0-\log \frac{s^{2}}{s^{2}+1}\right] = -\frac{1}{2}\left[\log \frac{s^{2}}{s^{2}+1}\right]
          </me>
          
          again
          <me>
            \mathscr{L}\left[\frac{1-\cos t}{t^{2}}\right]  =- \frac{1}{2} \int\limits_{s}^{\infty}\log  \frac{s^{2}}{s^{2}+1} \,ds 
          </me>
          <me>
            	= - \frac{1}{2} \int\limits_{s}^{\infty}\log - \frac{1}{2} \int\limits_{s}^{\infty}\log \left(\frac{s^{2}}{s^{2}+1}.1\right)\,ds
          </me>
        </p>
        <p>
          Integrating by parts, we have 
          <me>
            =-	\frac{1}{2}\left[\log \frac{s^{2}}{s^{2}+1}.s-\int\limits_{s}^{\infty}\frac{s^{2}+1}{s^{2}}.\frac{(s^{2}+1).2s -s^{2}(2s)s}{(s^{2}+1)^{2}}	\,ds\right]_{s}^{\infty}
          </me>
        <me>
          =-\frac{1}{2}\left[s \log \frac{s^{2}}{s^{2}+1}-2\int\limits_{s}^{\infty}\frac{1}{s^{2}+1}\,ds\right]_{s}^{\infty} 
        </me>
        <me>
          = -\frac{1}{2}\left[s \log \frac{s^{2}}{s^{2}+1}-2\tan ^{-1}s\right]_{s}^{\infty}
        </me>
        
          <me>
            =-\frac{1}{2}\left[0-2(\pi/2) -s \log \frac{s^{2}}{s^{2}+1}+2\tan ^{-1}s\right]
          </me>
          <me>
             = -\frac{1}{2}\left[-\pi-s \log \frac{s^{2}}{s^{2}+1}+2\tan ^{-1}s\right]	
          </me>
          <me>
            = \frac{\pi}{2}+\frac{s}{2} \log \frac{s^{2}}{s^{2}+1}-\tan^{-1}s
          </me>
          <me>
             = \left(\frac{\pi}{2}-\tan^{-1}s \right) +\frac{s}{2} \log \frac{s^{2}}{s^{2}+1}
          </me>
          <me>
            =\cot^{-1}s + \frac{s}{2} \log \frac{s^{2}}{s^{2}+1}.
          </me>
          </p>
      </solution>
    </example>
</section>
