<?xml version="1.0" encoding="UTF-8"?>

<section xml:id="sec_fourth-examplesA" xmlns:xi="http://www.w3.org/2001/XInclude">
  <title>ExamplesA</title>
 
<example>
  <statement>
    <p>
      The current in a circuit, containing a resistance <m>R</m>, an induction <m>L</m>, and 
      a constant e.m.f. <m>E</m>, at time <m>t</m>, is given by <m>i=\frac{E}{R}\left(1-e^{-\frac{Rt}{L}}\right)</m>. 
      Obtain a suitable approximation to <m>i</m> when <m>t</m> is very small.
    </p>
  </statement>
  <solution>
    <p>
       From a circuit <image source="fig41.png" width="30%"/>, we have potential drop across resistance <m> =iR</m> and	voltage induced at 
       inductance <m>=-L\frac{\,di}{\,dt} </m>. Using Kirchoff's Voltage law, 
       </p>
       <p>
       <me>
        E-L\frac{\,di}{\,dt} = iR
       </me>    
       or,
       <me>
         \frac{\,di}{\,dt}+\frac{Ri}{L}=\frac{E}{L}
       </me>
        or,
        <me>
          I.F. = e^{\int \frac{R}{L}\,dt}=e^{\frac{Rt}{L}}
        </me>
        Its solution is 	
        <me>
           i\cdot e^{\frac{Rt}{L}} = \int \frac{E}{L}e^{\frac{Rt}{L}}\,dt+C =\frac{E}{L}\cdot\frac{L}{R}e^{\frac{Rt}{L}}+C
        </me>
        <men xml:id="eqn-diffex1">
           \therefore \quad i=\frac{E}{R}+Ce^{-\frac{Rt}{L}}  
        </men>
        when  <m>t=0,\quad i=0 </m> then, <m>0=\frac{E}{R}+C</m>	 or, <m>C=-\frac{E}{R}</m>. 
        Therefore, expression <xref ref="eqn-diffex1"/> becomes 
        <me>
          i=\frac{E}{R}-\frac{E}{R}e^{-\frac{Rt}{L}} = \frac{E}{R}\left(1-e^{-\frac{Rt}{L}}\right) 
        </me>
        but,  when <m>t = \infty,</m>  
        <me>
          i=\frac{E}{R}. \qquad \text{ans.}
        </me>
           </p>
  </solution>
</example>
    
    <example>
      <statement>
        <p>
          Find the solution for the equation of motion when a mass <m>m</m> attached to a spring with 
          spring constant <m>k</m> is pulled and then released, as shown in 
          figure <image source="fig42.png" width="20%"/>
        </p>
      </statement>
      <solution>
        <p>
         The motion executed by a spring is simple harmonic motion, therefore, <m>F=-ky</m> (where <m>y</m> 
         is the displacement of mass <m>m</m> at any time, <m>t</m>.) 
         <me>
           m\frac{\,d^{2}y}{\,dt^{2}}=-ky
         </me>
         or,
         <me>
           \frac{\,d^{2}y}{\,dt^{2}}+\frac{k}{m}y=0 
         </me>
         or,
         <men xml:id="eqn-diffex2">
          \frac{\,d^{2}y}{\,dt^{2}}+\omega^{2}y=0
         </men>
         where <m>\omega^{2} = \frac{k}{m}</m>. The eqn. <xref ref="eqn-diffex2"/> is the equation of motion.
         <me>
           A.E. = m^{2}+\omega^{2}=0 \hspace{0.5cm}  \text{or,} \quad m=\pm i\omega
         </me>
         The general solution of eqn. <xref ref="eqn-diffex2"/> is then
         <men xml:id="eqn-diffeq3">
          y(t) =C_{1}e^{i\omega}t+C_{2}e^{-i\omega}t = A\cos\omega t+B\sin\omega t
         </men>
         If <m>T</m> be the period of motion, then <m>y(t)=y(t+T)</m>.
         <me>
           \therefore A \cos\omega t +B\sin\omega t =A\cos(\omega t+\omega T)+B\sin(\omega t+\omega t)
         </me>
         <me>
          = A\left[\cos\omega t\cdot\cos\omega T-\sin\omega t\cdot\sin\omega T\right] 
          + B\left[\sin\omega t\cdot\cos\omega T+\cos\omega t\cdot\sin\omega T\right]
         </me>
         <me>
          =\left(A\cos\omega T+B\sin\omega T\right)\cos\omega t+\left(B\cos\omega T-A\sin\omega T\right)\sin\omega t
         </me>
         equating on both sides, we get -
         <me>
          A\cos\omega T+B\sin\omega T = A 
         </me>
         <me>
          \Rightarrow \cos\omega T =1 \hspace{1cm} \text{and} \quad  \sin\omega T =0.
         </me>
         i.e.,
         <me>
           \cos\omega T =1=\cos 2n\pi  
         </me>
         or,
         <me>
         \omega T = 2n\pi
         </me>
         <me>
          \therefore  T = \frac{2n\pi}{\omega} = 2n\pi\sqrt{\frac{m}{k}} 
         </me>
        </p>
      </solution>
    </example>

    <example>
      <statement>
        <p>
          Solve 
          <me>
            \frac{\,d^{2}y}{\,dx^{2}}+a^{2}y=\sec ax.
          </me>
        </p>
      </statement>
      <solution>
        <p>
           A.E. is  <m>D^{2}+a^{2}=0</m> or, <m>D=\pm ai</m>.	
           <me>
            C.F. = C_{1}\cos ax+C_{2}\sin ax
           </me>
           <me>
            P.I. = \frac{1}{D^{2}+a^{2}}\cdot \sec ax = \frac{1}{(D+ai)(D-ai)}\cdot \sec ax
           </me>
           <me>
            = \frac{1}{2ai}\left[\frac{1}{(D-ai)}-\frac{1}{(D+ai)}\right]\sec ax
           </me>
           Therefore,
           <men xml:id="eqn-diffeq4">
            P.I. = \frac{1}{2ai}\frac{1}{(D-ai)}\sec ax-\frac{1}{2ai}\frac{1}{(D+ai)}\sec ax 
           </men>
           Now,
           <men xml:id="eqn-diffeq5">
             \frac{1}{(D-ai)}\sec ax = e^{aix}\int e^{-aix}\sec ax\,dx
           </men>
           [using eqns. <xref ref="eqn-pisol3"/>, and <xref ref="eqn-pisol4"/>]
           <me>
            =e^{aix}\int\frac{\cos ax-i\sin ax}{\cos ax}\,dx =e^{aix}\int(1-i\tan ax)\,dx 
           </me>
           <me>
             = e^{aix}(x+\frac{i}{a}\log\cos ax)
           </me>
            changing <m>i</m> to <m>-i</m>, we have 
           <me>
            \frac{1}{(D+ai)}\sec ax =e^{-aix}(x-\frac{i}{a}\log\cos ax)
           </me>
           putting these values in eqn. <xref ref="eqn-diffeq4"/>, we get - 
           <me>
            P.I. = \frac{1}{2ai}\left[e^{aix}\left(x+\frac{i}{a}\log\cos ax\right)-e^{-aix}\left(x-\frac{i}{a}\log\cos ax\right)\right]
           </me>
           <me>
            =\frac{x}{2ai}e^{aix}-\frac{x}{2ai}e^{-aix}+\frac{e^{aix}\log\cos ax}{2a^{2}}+\frac{e^{-aix}\log\cos ax}{2a^{2}}
           </me>
           <me>
            =\frac{x}{a}\frac{e^{aix}-e^{-aix}}{2i}+\frac{1}{a^{2}}\frac{e^{aix}+e^{-aix}}{2}\log\cos ax
           </me>
           <me>
             =\frac{x}{a}\sin ax +\frac{1}{a^{2}}\cos ax\cdot\log\cos ax
           </me>
           <me>
             \therefore  y= C_{1}\cos ax+C_{2}\sin ax+\frac{x}{a}\sin ax+\frac{1}{a^{2}}\cos ax\cdot\log\cos ax.
           </me>  
        </p>
      </solution>
    </example>

    <example>
      <statement>
        <p>
          Solve
          <me>
            \frac{\,d^{2}y}{\,dx^{2}}-2\frac{\,dy}{\,dx}+y=2\cos x.
          </me>
        </p>
      </statement>
      <solution>
        <p>
          <men xml:id="eqn-diffeq6">
            (D^{2}-2D+1)y =2\cos x 
          </men>
          <me>
            \text{A.E.,} \quad m^{2}-2m+1=0 
          </me>
          or,
          <me>
             (m-1)^{2}=0 \quad \Rightarrow  m=1,1
          </me>
          <men xml:id="eqn-diffeq7">
            \therefore \quad C.F. = y_{c}  = (C_{1}+C_{2}x)e^{x}  
          </men>
          <men xml:id="eqn-diffeq8">
            \text{P.I.} = y_{p} \quad \text{(By inspection method)}
          </men>
          Let, <m>y_{p} =-\sin x,</m> <m>Dy_{p}=-\cos x</m>,	and, <m>D^{2} y_{p} =\sin x</m>. 
          Therefore, <m>y=y_{p}</m> is a P.I. of eqn. <xref ref="eqn-diffeq6"/>, becouse it satisfies the equation.
          <men xml:id="eqn-diffeq9">
            y=y_{c}+y_{p}=(C_{1}+C_{2}x)e^{x}-\sin x 
          </men>
          It is a general solution of eqn. <xref ref="eqn-diffeq6"/>.
        </p>
        <p>
          <term>The solution of eqn. <xref ref="eqn-diffeq6"/> by successive integration method.</term>
          The roots of A.E. are real and equal, i.e., <m>m=1,1</m>. Hence, from eqn. <xref ref="eqn-pisol5"/>
          <men xml:id="eqn-diffeq10">
            y= e^{x}\int \bar{Q}(x)e^{-x}\,dx +C_{2}e^{x}  
          </men>
          where,
          <men xml:id="eqn-diffeq11">
          \bar{Q}(x) =2e^{x}\int e^{-x}\cos x\,dx+C_{1}e^{x} 
          </men>
          using <xref ref="eqn-pisol6"/>. Hence,
          <me>
            \int e^{-x}\cos x\,dx=\frac{e^{-x}(\sin x-\cos x)}{1+1}=\frac{e^{-x}(\sin x-\cos x)}{2}
          </me>
          <me>
            \because \quad \int e^{mx}\cos nx\,dx=\frac{e^{mx}(n\sin nx+m\cos nx)}{m^{2}+n^{2}}
          </me>
          and 
          <me>
            \int e^{mx}\sin nx\,dx=\frac{e^{mx}(m\sin nx-n\cos nx)}{m^{2}+n^{2}}
          </me>
          or,
          <me>
            \bar{Q}(x)=e^{x}.e^{-x}(\sin x-\cos x)+C_{1}e^{x}
          </me>
          <me>
            \therefore y=e^{x}\int \left\{\left(\sin x-\cos x\right)+C_{1}e^{x}\right\}e^{-x}\,dx +C_{2}e^{x}
          </me>
          <me>
            =e^{x}\left[\int e^{-x}\sin x\,dx-\int e^{-x}\cos x\,dx+C_{1}\int\,dx\right]+C_{2}e^{x}
          </me>
          <me>
            =e^{x}\left[\frac{e^{-x}(-\sin x-\cos x)}{2}-\frac{e^{-x}(\sin x-\cos x)}{2}+C_{1}x\right]+C_{2}e^{x}
          </me>
          <me>
            =\frac{(-\sin x-\cos x)}{2}-\frac{(\sin x-\cos x)}{2}+C_{1}xe^{x}+C_{2}e^{x}
          </me>
          <me>
            =(C_{1}x+C_{2})e^{x}-\sin x.   \qquad \text{ans}.
          </me>
          </p>
      </solution>
    </example>

<paragraphs>
  <title>Python Code for Differential Equation</title>
  <ol marker="1.">
    <li> 
      <p> For equation 
         <me>
         \frac{\,di}{\,dt}+\frac{Ri}{L}=\frac{E}{L}
       </me>
      <term>the Python code is</term>  <image source="odeQ1.png" width="60%"/> 
      </p>
       <p>
        from sympy.interactive import printing 
       </p>
       <p>
       printing.init_printing(use_latex=True) 
       </p>
<p>
  from sympy import * 
</p>
<p>
  import sympy as sp 
</p>
       <p>
        t=sp.Symbol('t', real=True) 
       </p>
<p>
   I=sp.Function('I')(t) 
</p>
<p>
  R, L, E=sp.symbols('R, L, E', real=True)
</p>
       <p>
        diffeq=Eq(I.diff(t)+R/L*I,E/L) 
       </p>
       <p>
         display(diffeq)
       </p>
       <p>
         dsolve(diffeq,I)
       </p>
       <p>
        import numpy as np 
       </p>
        <p>
           from scipy.integrate import odeint 
        </p>
        <p>
          import matplotlib.pyplot as plt
        </p>
<p>
  E=5 
</p>
       <p>
         R=5 
       </p> 
       <p>
         L=0.02 
       </p>
       <p>
         Io=0 
       </p>
       <p>
        t=np.arange(0,0.025,0.001)
       </p>

        <p>
          def f(I,t,E,L,R): 
        </p>
        <p>
           dIdt =-(R/L)*I+(E/L) 
        </p>
        <p>
           return dIdt
        </p>

 <p>
  Is=odeint(f,Io,t,args=(E,L,R))
 </p>
 <p>
   plt.plot(t,Is, '-') 
 </p>
 <p>
  plt.plot(t,Is, 'ro') 
 </p>
 <p>
  plt.title('DI(t)+RI(t)/L=E/L') 
 </p>
 <p>
  plt.xlabel('t(s)') 
 </p>
 <p>
  plt.ylabel('I(A)') 
 </p>
 <p>
   plt.show()
 </p>

       <p>
        Since <m> e^{RC_{1}}</m> is a constant, the general solution of this equation is 
     <m>I(t) = \left[\frac{E}{R}+Ce^{-Rt/L}\right]</m>. 
       </p>
    </li>
    <li>
      <p>
        <m>y"+a^2*y=0</m>
        <image source="odeQ2.png" width="60%"/> 
      </p>
      <p> 
        from sympy.interactive import printing
      </p>
      <p>
        printing.init_printing(use_latex=True) 
      </p>
      <p>
         from sympy import * 
      </p>
      <p>
        import sympy as sp 
      </p>

      <p>
        t,y =sp.symbols('t,y') 
      </p>
      <p>
         a=sp.Symbol('a',positive=True) 
      </p>
      <p>
          y=sp.Function('y')(t) 
      </p>
      <p>
         diffeq=Eq(y.diff(t,2)+a**2*y,0) 
      </p>
      <p>
         display(diffeq)
      </p>
      <p>
         dsolve(diffeq,y)
      </p>
<p>
  import numpy as np
</p>
<p>
  from scipy.integrate import odeint
</p>
<p>
  import matplotlib.pyplot as plt
</p>
<p>
  def f(u,t):
    return (u[1], -5*u[0])
</p>
<p>
   yo=[0,4]
</p>
<p>
   xs=np.arange(0,5,0.1)
</p>

<p>
  us=odeint(f,yo,xs)
</p>
<p>
  ys=us[:,0]
</p>


  <p>
    plt.plot(xs,ys, '-')
  </p>
<p>
  plt.plot(xs,ys, 'ro')
</p>
<p>
  plt.title('(D**2+5)y=0')
</p>
<p>
  plt.xlabel('t values')
</p>
<p>
  plt.ylabel('y values')
</p>
<p>
  plt.show()
</p>
</li>
<li>
  <p> 
    <m>y"+a^2*y=\sec(ax)</m>
     <image source="odeQ3.png" width="60%"/> 
  </p>
  </li>
  <li>
  <p>
    <m>y"-2y'+y=2*\cos(x)</m>
     <image source="odeQ4.png" width="60%"/> 
  </p>
  </li>
  </ol>
  
</paragraphs>
  
  <example>
    <statement>
      <p>
        Solve <me>x^{2}y''-(x^{2}+2x)y'+(x+2)y=x^{3}</me>.
        </p>
    </statement>
    <solution>
      <p>
        The equation in standard form is 
        <men xml:id="eqn-vcoef1">
          y''-\left(1+\frac{2}{x}\right)y' +\left(\frac{1}{x}+\frac{2}{x^{2}}\right)y=x  
        </men>
        Here, <m>P=-\left(1+\frac{2}{x}\right) </m>	and <m>Q= \left(\frac{1}{x}+\frac{2}{x^{2}}\right)</m>. 
        Since, <m>P+Qx=0</m>, we have <m>y_{1} =x </m> is a known integral of C.F. 
        So we find C.F. of the given differential eqn. <xref ref="eqn-vcoef1"/> by putting <m>y=vx</m>  in 
        <men xml:id="eqn-vcoef2">
          y''-\left(1+\frac{2}{x}\right)y' +\left(\frac{1}{x}+\frac{2}{x^{2}}\right)y=0  
        </men>
        or,
        <me>
          \frac{d^{2}v}{dx^{2}}-\frac{dv}{dx}=0
        </me>
        or,
        <me>
          [D^{2}-D]v =0,
        </me>
        <me>
          \therefore \quad D =0,1.
        </me>
        Hence, <m>v=C_{1}+C_{2}e^{x}</m>	[<m>\because C.F.= C_{1}e^{m_{1}x}+C_{2}e^{m_{2}x}</m>].  
        Therefore the C.F. of eqn. <xref ref="eqn-vcoef2"/> is <m>y=vx=C_{1}x+C_{2}xe^{x} </m>, 
        where, <m>y_{1} =x {,} y_{2}=xe^{x}</m>,  and <m>|W| =y_{1}y'_{2} -y'_{1} y_{2} =x^{2}e^{x}</m>. 
        Now, let <m>y=v_{1}y_{1}+v_{2}y_{2} = v_{1}x+v_{2}xe^{x}</m> be the solution of eqn. <xref ref="eqn-vcoef1"/>.
        Where,
        <me>
           v_{1}=-\int \frac{Xy_{2}}{|W|}\,dx+C_{1} =-x+C_{1}
        </me>
        and 
        <me>
           v_{2}=\int \frac{Xy_{1}}{|W|}\,dx+C_{2} =-e^{-x}+C_{2}
        </me>
        Therefore the complete solution is 
        <me>
          y=(-x+C_{1})x+(-e^{-x}+C_{2})xe^{x}=(C_{1}x+C_{2}xe^{x})-(x^{2}+x).
        </me> 
      </p>
    </solution>
  </example>

  <example>
    <statement>
      <p>
        Solve  <me>x^{2}y''-2xy'+2y=x\ln{x}</me>.
      </p>
    </statement>
    <solution>
      <p>
        The equation in standard form is 
        <men xml:id="eqn-vcoef3">
          y''-\frac{2}{x}y' +\frac{2}{x^{2}}y =\frac{\ln{x}}{x}
        </men>
        Since <m>P+Qx=0</m> and <m>2+2Px+Qx^{2} =0 </m> we assume <m>y_{1}=x</m> 
        and <m>y_{2}=x^{2}</m> to be the two independent solutions of eqn. <xref ref="eqn-vcoef3"/>. 
        Hence  we have <m>|W|=x^{2}</m>. Therefore the complete solution of eqn. <xref ref="eqn-vcoef3"/> is 
		     [see eqn. <xref ref="eqn-varcoef13"/>]	
         <me>
          y=x\left[-\int\frac{x^{2}\left(\frac{\ln{x}}{x}\right)}{x^{2}}\,dx+C_{1}\right]+x^{2}\left[\int\frac{x\left(\frac{\ln{x}}{x}\right)}{x^{2}}\,dx+C_{2}\right]
         </me>
         <me>
          =-x\int\left(\frac{\ln{x}}{x}\right)\,dx+C_{1}x+x^{2}\int\left(\frac{\ln{x}}{x^{2}}\right)\,dx+C_{2}x^{2}
         </me>
         <me>
          =-x\left\{\frac{1}{2}(\ln x)^{2}\right\}+x^{2}\left\{-\frac{\ln x}{x}-\frac{1}{x}\right\}+(C_{1}x+C_{2}x^{2})
         </me>
         <me>
          =-x\left\{\frac{1}{2}(\ln x)^{2}+\ln x+1\right\}+(C_{1}x+C_{2}x^{2}).
         </me>
      </p>
    </solution>
  </example>

  <example>
    <statement>
      <p> Solve 
        <me>
          x^{2}y''+xy' - y=x^{2}e^{x}.
        </me>
      </p>
    </statement>
    <solution>
      <p>
        <men xml:id="eqn-vcoef4">
           x^{2}y''+xy' - y=x^{2}e^{x} 
        </men>
        This is the equation with decreasing power of x. Hence put <m>x=e^{z}</m> and <m>\frac{d}{dz}\equiv D</m>. 
       We have	
       <me>
        D(D-1)y+Dy-y=e^{2z}e^{e^{z}}
       </me>
       or,
       <men xml:id="eqn-vcoef5">
        (D^{2}-1)y=e^{2z}e^{e^{z}}
       </men>
       A.E. is 
       <me>
        D^{2}-1 =0 
       </me>
       or,
       <me>
        D=+1,-1
       </me>
       <men xml:id="eqn-vcoef6">
         \text{C.F.} = C_{1}e^{z}+C_{2}e^{-z} = C_{1}x+\frac{C_{2}}{x} 
       </men>
       where <m>y_{1}=x</m> and <m>y_{2}=\frac{1}{x}</m> also 
       <me>
        |W| =y_{1}y'_{2} -y'_{1}y_{2} = x(-\frac{1}{x^{2}})-1.\frac{1}{x} =-\frac{2}{x}
       </me>
        The standard form of eqn. <xref ref="eqn-vcoef4"/> is  
       <men xml:id="eqn-vcoef7">
        y'' +\frac{1}{x}y'-\frac{1}{x^{2}}y = e^{x} 
       </men>
       Now the complete solution of eqn. <xref ref="eqn-vcoef7"/> is 
       <me>
        y=x\left[-\int\frac{e^{x}.\frac{1}{x}}{-\frac{2}{x}}\,dx +C_{1}\right]+\frac{1}{x}\left[\int\frac{e^{x}.x}{-\frac{2}{x}}\,dx+C_{2}\right]
       </me>
       <fn> 
       If <m>x=e^{z}</m> then <m>z=\log x</m> and  <m>\frac{\,dz}{\,dx}=\frac{1}{x} </m>  
       hence, 
       <me>
        \frac{\,dy}{\,dx} =\frac{\,dy}{\,dz}\cdot \frac{\,dz}{\,dx} =\frac{1}{x}\cdot \frac{\,dy}{\,dz} 
        </me>
        or,
        <me>
          x\frac{\,dy}{\,dx}=\frac{\,dy}{\,dz}=Dy   
        </me>
        also,
        <me>
          x^{2}\frac{\,d^{2}y}{\,dx^{2}}
        </me>
        <me>
          = \frac{\,d^{2}y}{\,dz^{2}}-\frac{\,dy}{\,dz}=D^{2}y-Dy =D(D-1)y
        </me>
       </fn>
       <me>
         =x\left[\frac{e^{x}}{2}+C_{1}\right]+\frac{1}{x}\left[-\frac{1}{2}e^{x}x^{2}+xe^{x}-e^{x}+C_{2}\right] 
       </me>
       <me>
        = (C_{1}x+\frac{C_{2}}{x})+(e^{x}-\frac{e^{x}}{x})
       </me>
      </p>
    </solution>
  </example>

  <example>
    <statement>
      <p>
         Solve <me>
           y''-2y' - 3y=\sin(2x)
         </me> 
      </p>
    </statement>
    <solution>
      <p>
       It has <m>1-P+Q=0</m> type auxiliary equaion, hence <m>y_{1} =e^{-x}</m> be the known integral of C.F. 
       Select <m>y=vy_{1}</m> be the solutioin of corresponding differential equation. 
       (read page <xref ref="subsubsec-var_coef"/> for details). We may get a homogeneous equation like <m>v''-2v'=0</m> which gives, 
       <m>D=\pm\sqrt{2}.</m> This corresponds to <m>C.F. = C_{1}e^{m_{1}x}+C_{2}e^{m_{2}x}.</m> 
       Use Wronskian to find  the complete solution of the differential equation.  
      </p>
    </solution>
  </example>
</section>
