<?xml version="1.0" encoding="UTF-8"?>

<section xml:id="sec_fifth-examplesA" xmlns:xi="http://www.w3.org/2001/XInclude">
  <title>Examples A</title>
 
<example>
  <statement>
    <p>
      Find the Fourier series expansion of <m>f(x) =x</m>,  where 
      <m>0\lt x \lt 2\pi</m>, 	and sketch its graph from <m>x=-4\pi</m> to <m>4\pi</m>.
    </p>
  </statement>
  <solution>
    <p>
      Let 
      <me>
         f(x) = x = 	\frac{a_{o}}{2} + \sum\limits_{n=1}^{\infty}\left[a_{n}\cos nx + b_{n}\sin nx\right]
      </me>
      where 
      <me>
        a_{o} = \frac{1}{\pi}\int\limits_{0}^{2\pi}f(x)\,dx = \frac{1}{\pi}\int\limits_{0}^{2\pi}x\,dx =  \frac{1}{\pi}\left[\frac{x^{2}}{2}\right]^{2\pi}_{0} = 2\pi.
      </me>
      <me>
        a_{n}= \frac{1}{\pi}\int\limits_{0}^{2\pi} f(x)\cos nx \,dx = \frac{1}{\pi}\int\limits_{0}^{2\pi} x\cos nx \,dx 
      </me>
      <me>
        = \frac{1}{\pi}\left[x.\frac{\sin nx}{n}-1.\frac{\cos nx}{-n^{2}}\right]_{0}^{2\pi}
      </me>
      
      <me>
        =\frac{1}{\pi}\left[0+\frac{1}{n^{2}}(\cos 2n\pi-\cos 0)\right]= \frac{1}{\pi}\left[\frac{1}{n^{2}}(1-1)\right] = 0.
      </me>
      and 
      <me>
        b_{n}= \frac{1}{\pi}\int\limits_{0}^{2\pi} f(x)\sin nx \,dx = \frac{1}{\pi}\int\limits_{0}^{2\pi} x\sin nx \,dx 
      </me>
      <me>
        = \frac{1}{\pi}\left[x.\frac{\cos nx}{-n}-1.\frac{\sin nx}{-n^{2}}\right]_{0}^{2\pi}
      </me>
      
      <me>
        =\frac{1}{\pi}\left[\frac{2\pi \cos 2n \pi}{-n}+\frac{1}{n^{2}}\left(\sin nx\right)_{0}^{2\pi}\right]= -\frac{2}{n}.
      </me>
      Substituting these values in expression <m>f(x)</m>, we get -
      <me>
        x=\pi - 2\left[\sin x+\frac{\sin 2x}{2}+\frac{\sin 3x}{3}+\cdots\right]
      </me>
			The graphical representation of the given function is shown in 
      figure below. <image source="fig51.png" width ="45%"/>
    </p>
  </solution>
</example>

<example>
  <statement>
    <p>
      Obtain the Fourier series for <m>f(x) = e^{-x}</m> in the interval <m>0 \lt x\lt 2\pi</m>.
    </p>
  </statement>
  <solution>
    <p>
      Let
      <me>
        f(x) =e^{-x} = 	\frac{a_{o}}{2} + \sum\limits_{n=1}^{\infty}\left[a_{n}\cos nx + b_{n}\sin nx\right]
      </me>
      where 
      <me>
        a_{o} = \frac{1}{\pi}\int\limits_{0}^{2\pi}f(x)\,dx = \frac{1}{\pi}\int\limits_{0}^{2\pi}e^{-x}\,dx =  \frac{1}{\pi}\left[\frac{e^{-x}}{-1}\right]^{2\pi}_{0} 
      </me>
      <me>
        = \frac{1}{\pi}\left[-e^{-2\pi}+1\right] = \frac{1-e^{-2\pi}}{\pi}.
      </me>
      
      <me>
         a_{n} = \frac{1}{\pi}\int\limits_{0}^{2\pi} f(x)\cos nx \,dx = \frac{1}{\pi}\int\limits_{0}^{2\pi} e^{-x}\cos nx \,dx 
      </me>
      <me>
        = \frac{1}{\pi}\left[\frac{e^{-x}}{1+n^{2}}(-\cos nx +n \sin nx)\right]_{0}^{2\pi}
      </me>
      
      <me>
        =\frac{1}{\pi(1+n^{2})}\left[e^{-x}(-\cos 2n\pi+n\sin 2n\pi) - e^{0}(-\cos 0+n\sin 0)\right]
      </me>
      <me>
        =\frac{1}{\pi(1+n^{2})}\left[1-e^{-2\pi}\right].
      </me>
      <me>
        b_{n} = \frac{1}{\pi}\int\limits_{0}^{2\pi} f(x)\sin nx \,dx = \frac{1}{\pi}\int\limits_{0}^{2\pi} e^{-x}\sin nx \,dx 
      </me>
      <me>
        = \frac{1}{\pi}\left[\frac{e^{-x}}{1+n^{2}}(-\sin nx +n \cos nx)\right]_{0}^{2\pi}
      </me>
      
      <me>
        =\frac{1}{\pi (1+n^{2})}\left[e^{-2\pi}(-\sin 2n\pi - n \cos 2n \pi) - e^{0}(-\sin 0 - n\cos 0)\right]
      </me>
      <me>
        =\frac{n}{\pi (1+n^{2})}\left[e^{-2\pi}(-n) - e^{0}(-n)\right].
      </me>
      From expression <m>f(x)</m>, we get -
      <me>
        e^{-x} = \frac{1-e^{-2\pi}}{\pi} + \sum\limits_{n=1}^{\infty}\left[\frac{1-e^{-2\pi}}{\pi (1+n^{2})} \cos nx + \frac{1-e^{-2\pi}}{\pi (1+n^{2})}n \sin nx\right]
      </me>
      <me>
        =\frac{1-e^{-2\pi}}{\pi}\left[\frac{1}{2}+\left\{\frac{\cos x}{2}+\frac{\cos 2x}{5}+\cdots + \right\} \right.
      </me>
      <me>
       \left. + \left\{\frac{\sin x}{2}+\frac{2\sin 2x}{5}+\cdots + \right\}\right].
      </me>
        which is the required Fourier series.
    </p>
  </solution>
</example>

<example>
  <statement>
    <p>
      Find the Fourier series of the function
      <me>
         f(x) = \begin{cases} 
             -1, &amp; \text{for } -\pi \lt x \lt -\frac{\pi}{2}\\ 
                 0,       &amp; \text{for} -\frac{\pi}{2} \lt x \lt \frac{\pi}{2}\\ 
                     +1,  &amp; \text{for}  +\frac{\pi}{2} \lt x \lt \pi. 
                     \end{cases}
      </me>
    </p>
  </statement>
  <solution>
    <p>
      Let
      <me>
        f(x) =	\frac{a_{o}}{2} + \sum\limits_{n=1}^{\infty}\left[a_{n}\cos nx + b_{n}\sin nx\right]
      </me>
      where 
      <me>
        a_{o} = \frac{1}{\pi}\int\limits_{-\pi}^{\pi}f(x)\,dx = \frac{1}{\pi}\left[\int\limits_{-\pi}^{-\pi/2}(-1)\,dx + \int\limits_{-\pi/2}^{\pi/2} 0. \,dx + \int\limits_{\pi/2}^{\pi}(+1)\,dx\right]
      </me>
      <me>
        =\frac{1}{\pi}\left[-\left(x\right)_{-\pi}^{-\pi/2}+\left(x\right)_{\pi/2}^{\pi}\right]
      </me>
      <me>
         = \frac{1}{\pi}\left[-\left\{-\frac{\pi}{2}+\pi \right\} + \left\{\pi -\frac{\pi}{2} \right\}\right] = \frac{1}{\pi}\left[-\left\{-\frac{\pi}{2} +\frac{\pi}{2} \right\}\right] = 0.
      </me>
      <me>
        a_{n} = \frac{1}{\pi}\int\limits_{-\pi}^{\pi} f(x)\cos nx \,dx 
      </me>
      <me>
        = \frac{1}{\pi}\left[\int\limits_{-\pi}^{-\pi/2} (-1)\cos nx \,dx + \int\limits_{-\pi/2}^{\pi/2} 0.\cos nx \,dx + \int\limits_{\pi/2}^{\pi} (+1)\cos nx \,dx\right]
      </me>
      
      <me>
        =\frac{1}{\pi}\left[-\left(\frac{\sin nx}{n}\right)_{-\pi}^{-\pi/2}+\left(\frac{\sin nx}{n}\right)_{\pi/2}^{\pi}\right]
      </me>
        <me>
          =\frac{1}{\pi}\left[-\left(-\frac{\sin n\pi/2}{n}+	\frac{\sin n\pi}{n}\right)+\left(\frac{\sin n\pi}{n} -	\frac{\sin n\pi/2}{n}\right)\right] = 0.
        </me>
        <me>
          b_{n} = \frac{1}{\pi}\int\limits_{-\pi}^{\pi} f(x)\sin nx \,dx 
        </me>
        <me>
          = \frac{1}{\pi}\left[\int\limits_{-\pi}^{-\pi/2} (-1)\sin nx \,dx + \int\limits_{-\pi/2}^{\pi/2} 0.\sin nx \,dx + \int\limits_{\pi/2}^{\pi} (+1)\sin nx \,dx\right]
        </me>
        
        <me>
          =\frac{1}{\pi}\left[+\left(\frac{\cos nx}{n}\right)_{-\pi}^{-\pi/2}+\left(\frac{\cos nx}{-n}\right)_{\pi/2}^{\pi}\right]
        </me>
          now, from expression <m>f(x)</m>, we get -
          <me>
            f(x)=\sum\limits_{n=1}^{\infty} \left[+\frac{2}{n\pi}\left(\cos \frac{n\pi}{2}-\cos n\pi\right)\sin nx\right]
          </me>
          <me>
            = +\frac{2}{\pi}\left[\frac{\sin x}{1}-\frac{2\sin 2x}{2}+\frac{\sin 3x}{3}-\cdots\right]
          </me>
          <me>
            = +\frac{2}{\pi}\left[\sin x-\frac{2\sin 2x}{2}+\frac{\sin 3x}{3}-\cdots\right].
          </me>
            which is the required Fourier series expansion.
    </p>
  </solution>
</example>
</section>
